@prefix : <https://w3id.org/pmd/co#> .
@prefix owl: <http://www.w3.org/2002/07/owl#> .
@prefix rdf: <http://www.w3.org/1999/02/22-rdf-syntax-ns#> .
@prefix xml: <http://www.w3.org/XML/1998/namespace> .
@prefix xsd: <http://www.w3.org/2001/XMLSchema#> .
@prefix rdfs: <http://www.w3.org/2000/01/rdf-schema#> .
@base <https://w3id.org/pmd/co> .

<https://w3id.org/pmd/co> rdf:type owl:Ontology .

#################################################################
#    Annotation properties
#################################################################

###  http://purl.obolibrary.org/obo/IAO_0000111
<http://purl.obolibrary.org/obo/IAO_0000111> rdf:type owl:AnnotationProperty ;
                                             rdfs:isDefinedBy <http://purl.obolibrary.org/obo/iao.owl> .


###  http://purl.obolibrary.org/obo/IAO_0000114
<http://purl.obolibrary.org/obo/IAO_0000114> rdf:type owl:AnnotationProperty ;
                                             rdfs:isDefinedBy <http://purl.obolibrary.org/obo/iao.owl> .


###  http://purl.obolibrary.org/obo/IAO_0000115
<http://purl.obolibrary.org/obo/IAO_0000115> rdf:type owl:AnnotationProperty ;
                                             rdfs:isDefinedBy <http://purl.obolibrary.org/obo/iao.owl> .


###  http://purl.obolibrary.org/obo/IAO_0000117
<http://purl.obolibrary.org/obo/IAO_0000117> rdf:type owl:AnnotationProperty ;
                                             rdfs:isDefinedBy <http://purl.obolibrary.org/obo/iao.owl> .


###  http://purl.obolibrary.org/obo/IAO_0000119
<http://purl.obolibrary.org/obo/IAO_0000119> rdf:type owl:AnnotationProperty ;
                                             rdfs:isDefinedBy <http://purl.obolibrary.org/obo/iao.owl> .


###  http://swrl.stanford.edu/ontologies/3.3/swrla.owl#isRuleEnabled
<http://swrl.stanford.edu/ontologies/3.3/swrla.owl#isRuleEnabled> rdf:type owl:AnnotationProperty ;
                                                                  rdfs:isDefinedBy <http://swrl.stanford.edu/ontologies/3.3/swrla.owl> .


###  http://www.w3.org/2000/01/rdf-schema#comment
rdfs:comment rdfs:isDefinedBy <http://www.w3.org/2000/01/rdf-schema.owl> .


###  http://www.w3.org/2000/01/rdf-schema#isDefinedBy
rdfs:isDefinedBy rdfs:isDefinedBy <http://www.w3.org/2000/01/rdf-schema.owl> .


###  http://www.w3.org/2000/01/rdf-schema#label
rdfs:label rdfs:isDefinedBy <http://www.w3.org/2000/01/rdf-schema.owl> .


###  http://www.w3.org/2004/02/skos/core#altLabel
<http://www.w3.org/2004/02/skos/core#altLabel> rdf:type owl:AnnotationProperty ;
                                               rdfs:isDefinedBy <http://www.w3.org/2004/02/skos/core.owl> .


###  http://www.w3.org/2004/02/skos/core#definition
<http://www.w3.org/2004/02/skos/core#definition> rdf:type owl:AnnotationProperty ;
                                                 rdfs:isDefinedBy <http://www.w3.org/2004/02/skos/core.owl> .


###  https://w3id.org/pmd/co/definitionSource
<https://w3id.org/pmd/co/definitionSource> rdf:type owl:AnnotationProperty ;
                                           rdfs:isDefinedBy <https://w3id.org/pmd/co.owl> .


#################################################################
#    Datatypes
#################################################################

###  http://www.w3.org/1999/02/22-rdf-syntax-ns#PlainLiteral
rdf:PlainLiteral rdfs:isDefinedBy <http://www.w3.org/1999/02/22-rdf-syntax-ns.owl> .


###  http://www.w3.org/2001/XMLSchema#boolean
xsd:boolean rdfs:isDefinedBy <http://www.w3.org/2001/xmlschema.owl> .


###  http://www.w3.org/2001/XMLSchema#string
xsd:string rdfs:isDefinedBy <http://www.w3.org/2001/xmlschema.owl> .


#################################################################
#    Object Properties
#################################################################

###  http://purl.obolibrary.org/obo/RO_0000087
<http://purl.obolibrary.org/obo/RO_0000087> rdf:type owl:ObjectProperty ;
                                            rdfs:isDefinedBy <http://purl.obolibrary.org/obo/ro.owl> ;
                                            rdfs:label "has role"@en .


###  http://www.w3.org/ns/prov#wasDerivedFrom
<http://www.w3.org/ns/prov#wasDerivedFrom> rdf:type owl:ObjectProperty ;
                                           rdfs:isDefinedBy <http://www.w3.org/ns/prov.owl> .


###  https://w3id.org/pmd/co/belongsToProject
<https://w3id.org/pmd/co/belongsToProject> rdf:type owl:ObjectProperty ;
                                           owl:inverseOf <https://w3id.org/pmd/co/process> ;
                                           rdfs:domain <https://w3id.org/pmd/co/Process> ;
                                           rdfs:range <https://w3id.org/pmd/co/Project> ;
                                           rdfs:isDefinedBy <https://w3id.org/pmd/co.owl> ;
                                           <http://www.w3.org/2004/02/skos/core#definition> "Association between a process and a project."@en ,
                                                                                            "belongs to process"@en .


###  https://w3id.org/pmd/co/characteristic
<https://w3id.org/pmd/co/characteristic> rdf:type owl:ObjectProperty ;
                                         owl:inverseOf <https://w3id.org/pmd/co/characteristicOf> ;
                                         rdfs:isDefinedBy <https://w3id.org/pmd/co> ;
                                         rdfs:label "characteristic"@en ;
                                         <http://www.w3.org/2004/02/skos/core#altLabel> "has characteristic"@en ;
                                         <http://www.w3.org/2004/02/skos/core#definition> "Die Objekteigenschaft characterisitc, wird in Verbindung mit ProzessKnoten, Prozess und Objekt verwendet und dient zur Herstellung einer Verbindung mit dem WerteObjekt. Diese Eigenschaft ermöglicht die Abbildung von Beziehungen zwischen ProzessKnoten, Prozessen und Objekten und den dazugehörigen Werten oder Attributen (Metadaten), die in WerteObjekt ausgedrückt sind."@de ,
                                                                                          "The object property characteristic, in conjunction with ProcessingNode, Process and Object, is used to establish a connection with ValueObjects. This property enables the representation of relationships between ProcessingNodes, Processes and Objects and the associated values or attributes (metadata) that are stored in ValueObjects."@en .


###  https://w3id.org/pmd/co/characteristicOf
<https://w3id.org/pmd/co/characteristicOf> rdf:type owl:ObjectProperty ;
                                           rdfs:isDefinedBy <https://w3id.org/pmd/co> ;
                                           rdfs:label "characteristic of"@en ;
                                           <http://www.w3.org/2004/02/skos/core#altLabel> "is characteristic of" .


###  https://w3id.org/pmd/co/input
<https://w3id.org/pmd/co/input> rdf:type owl:ObjectProperty ;
                                rdfs:subPropertyOf <https://w3id.org/pmd/co/participant> ;
                                owl:inverseOf <https://w3id.org/pmd/co/inputOf> ;
                                rdfs:isDefinedBy <https://w3id.org/pmd/co> ;
                                rdfs:label "input"@en ;
                                <http://www.w3.org/2004/02/skos/core#altLabel> "has input" ;
                                <http://www.w3.org/2004/02/skos/core#definition> "This property is used to link the processes to their input objects."@en .


###  https://w3id.org/pmd/co/inputOf
<https://w3id.org/pmd/co/inputOf> rdf:type owl:ObjectProperty ;
                                  rdfs:subPropertyOf <https://w3id.org/pmd/co/participantOf> ;
                                  rdfs:isDefinedBy <https://w3id.org/pmd/co> ;
                                  rdfs:label "input of"@en ;
                                  <http://www.w3.org/2004/02/skos/core#altLabel> "is input of" .


###  https://w3id.org/pmd/co/output
<https://w3id.org/pmd/co/output> rdf:type owl:ObjectProperty ;
                                 rdfs:subPropertyOf <https://w3id.org/pmd/co/participant> ;
                                 owl:inverseOf <https://w3id.org/pmd/co/outputOf> ;
                                 rdfs:isDefinedBy <https://w3id.org/pmd/co> ;
                                 rdfs:label "output"@en ;
                                 <http://www.w3.org/2004/02/skos/core#altLabel> "has output" ;
                                 <http://www.w3.org/2004/02/skos/core#definition> "This property is used to link the processes to their output objects"@en .


###  https://w3id.org/pmd/co/outputOf
<https://w3id.org/pmd/co/outputOf> rdf:type owl:ObjectProperty ;
                                   rdfs:subPropertyOf <https://w3id.org/pmd/co/participantOf> ;
                                   rdfs:isDefinedBy <https://w3id.org/pmd/co> ;
                                   rdfs:label "output of"@en ;
                                   <http://www.w3.org/2004/02/skos/core#altLabel> "is output of"@en .


###  https://w3id.org/pmd/co/participant
<https://w3id.org/pmd/co/participant> rdf:type owl:ObjectProperty ;
                                      owl:inverseOf <https://w3id.org/pmd/co/participantOf> ;
                                      rdfs:domain <https://w3id.org/pmd/co/Process> ;
                                      rdfs:isDefinedBy <https://w3id.org/pmd/co> ;
                                      rdfs:label "participant"@en ;
                                      <http://www.w3.org/2004/02/skos/core#altLabel> "has participant" ;
                                      <http://www.w3.org/2004/02/skos/core#definition> "A relation between a process and an object, in which the objects is somehow involved in the process."@en .


###  https://w3id.org/pmd/co/participantOf
<https://w3id.org/pmd/co/participantOf> rdf:type owl:ObjectProperty ;
                                        rdfs:isDefinedBy <https://w3id.org/pmd/co> ;
                                        rdfs:label "participant of"@en ;
                                        <http://www.w3.org/2004/02/skos/core#altLabel> "is participant of"@en .


###  https://w3id.org/pmd/co/process
<https://w3id.org/pmd/co/process> rdf:type owl:ObjectProperty ;
                                  rdfs:domain <https://w3id.org/pmd/co/Project> ;
                                  rdfs:range <https://w3id.org/pmd/co/Process> ;
                                  rdfs:isDefinedBy <https://w3id.org/pmd/co> ;
                                  rdfs:label "process"@en ;
                                  <http://www.w3.org/2004/02/skos/core#altLabel> "has process"@en ;
                                  <http://www.w3.org/2004/02/skos/core#definition> "Describes that a process is associated with a project."@en .


#################################################################
#    Data properties
#################################################################

###  https://w3id.org/pmd/co/value
<https://w3id.org/pmd/co/value> rdf:type owl:DatatypeProperty ;
                                rdfs:isDefinedBy <https://w3id.org/pmd/co> ;
                                rdfs:label "hat Wert"@de ,
                                           "value"@en ;
                                <http://www.w3.org/2004/02/skos/core#definition> "Provides the actual value a value object is referring to."@en .


#################################################################
#    Classes
#################################################################

###  http://purl.obolibrary.org/obo/IAO_0000078
<http://purl.obolibrary.org/obo/IAO_0000078> rdf:type owl:Class ;
                                             owl:equivalentClass [ rdf:type owl:Class ;
                                                                   owl:oneOf ( <http://purl.obolibrary.org/obo/IAO_0000002>
                                                                               <http://purl.obolibrary.org/obo/IAO_0000120>
                                                                               <http://purl.obolibrary.org/obo/IAO_0000121>
                                                                               <http://purl.obolibrary.org/obo/IAO_0000122>
                                                                               <http://purl.obolibrary.org/obo/IAO_0000123>
                                                                               <http://purl.obolibrary.org/obo/IAO_0000124>
                                                                               <http://purl.obolibrary.org/obo/IAO_0000125>
                                                                               <http://purl.obolibrary.org/obo/IAO_0000423>
                                                                               <http://purl.obolibrary.org/obo/IAO_0000428>
                                                                             )
                                                                 ] ;
                                             <http://purl.obolibrary.org/obo/IAO_0000111> "curation status specification"@en ;
                                             <http://purl.obolibrary.org/obo/IAO_0000114> <http://purl.obolibrary.org/obo/IAO_0000125> ;
                                             <http://purl.obolibrary.org/obo/IAO_0000115> "The curation status of the term. The allowed values come from an enumerated list of predefined terms. See the specification of these instances for more detailed definitions of each enumerated value."@en ;
                                             rdfs:isDefinedBy <http://purl.obolibrary.org/obo/iao.owl> ;
                                             rdfs:label "curation status specification"@en .


###  http://www.w3.org/ns/prov#Organization
<http://www.w3.org/ns/prov#Organization> rdf:type owl:Class ;
                                         rdfs:isDefinedBy <http://www.w3.org/ns/prov.owl> .


###  https://w3id.org/pmd/co/AnalysingProcess
<https://w3id.org/pmd/co/AnalysingProcess> rdf:type owl:Class ;
                                           rdfs:subClassOf <https://w3id.org/pmd/co/Process> ;
                                           rdfs:isDefinedBy <https://w3id.org/pmd/co> ;
                                           rdfs:label "Analyseprozess"@de ,
                                                      "Analysing Process"@en ;
                                           <http://www.w3.org/2004/02/skos/core#definition> "A process that is driven by the primary intent to gain new measurements."@en .


###  https://w3id.org/pmd/co/ClassificationDocument
<https://w3id.org/pmd/co/ClassificationDocument> rdf:type owl:Class ;
                                                 rdfs:subClassOf <https://w3id.org/pmd/co/Document> ;
                                                 rdfs:isDefinedBy <https://w3id.org/pmd/co> ;
                                                 rdfs:label "Classification Document"@en ,
                                                            "Klassifzierungsdokument"@de ;
                                                 <http://www.w3.org/2004/02/skos/core#definition> "Diese Entität beschreibt ein Dokument, das dazu dient, den Arbeits- oder Anwendungsbereich eines Prozessknotens in Übereinstimmung mit genormten Abstufungen zu definieren."@de ,
                                                                                                  "This entity describes a document used to define the working or application range of a process node in accordance with standardized graduations."@en .


###  https://w3id.org/pmd/co/DepartmentRole
<https://w3id.org/pmd/co/DepartmentRole> rdf:type owl:Class ;
                                         rdfs:subClassOf [ rdf:type owl:Restriction ;
                                                           owl:onProperty [ owl:inverseOf <http://purl.obolibrary.org/obo/RO_0000087>
                                                                          ] ;
                                                           owl:someValuesFrom <http://www.w3.org/ns/prov#Organization>
                                                         ] ;
                                         rdfs:isDefinedBy <https://w3id.org/pmd/co.owl> ;
                                         rdfs:label "Department Role"@en ,
                                                    "A role indication that an organization is a sub section of another organization." .


###  https://w3id.org/pmd/co/Description
<https://w3id.org/pmd/co/Description> rdf:type owl:Class ;
                                      rdfs:isDefinedBy <https://w3id.org/pmd/co> ;
                                      rdfs:label "Beschreibung"@de ,
                                                 "Description"@en ;
                                      <http://www.w3.org/2004/02/skos/core#definition> "Ein beschreibender Text, der die Natur / Beschaffenheit / Informationen zu einer Entität qualifiziert (z.B. Aktivitäten, Entitäten, Objekten, ...)."@de ,
                                                                                       "A descriptive text qualifying the nature of a thing (e.g. agent, activity, entity, object, ...)." .


###  https://w3id.org/pmd/co/Document
<https://w3id.org/pmd/co/Document> rdf:type owl:Class ;
                                   rdfs:isDefinedBy <https://w3id.org/pmd/co> ;
                                   rdfs:label "Document"@en ,
                                              "Dokument"@de ;
                                   <http://www.w3.org/2004/02/skos/core#definition> "An original or official paper relied on as the basis, proof, or support of something"@en ,
                                                                                    "Ein Original oder offizielles Papier, auf das man sich als Grundlage, Beweis oder Unterstützung von etwas stützt."@de ;
                                   <https://w3id.org/pmd/co/definitionSource> "“Document.” Merriam-Webster.com Dictionary, Merriam-Webster, https://www.merriam-webster.com/dictionary/document. Accessed 16 Jan. 2023."@en .


###  https://w3id.org/pmd/co/Identifier
<https://w3id.org/pmd/co/Identifier> rdf:type owl:Class ;
                                     rdfs:isDefinedBy <https://w3id.org/pmd/co> ;
                                     rdfs:label "Identifier"@en ,
                                                "Identifikator"@de ;
                                     <http://www.w3.org/2004/02/skos/core#definition> "A named value intended to distinguish between entities."@en .


###  https://w3id.org/pmd/co/Image
<https://w3id.org/pmd/co/Image> rdf:type owl:Class ;
                                rdfs:isDefinedBy <https://w3id.org/pmd/co> ;
                                rdfs:label "Bild"@de ,
                                           "Image"@en ;
                                <http://www.w3.org/2004/02/skos/core#definition> "A visual representation of something"@en ;
                                <https://w3id.org/pmd/co/definitionSource> "“Image.” Merriam-Webster.com Dictionary, Merriam-Webster, https://www.merriam-webster.com/dictionary/image. Accessed 25 Nov. 2022."@en .


###  https://w3id.org/pmd/co/InitiatorRole
<https://w3id.org/pmd/co/InitiatorRole> rdf:type owl:Class ;
                                        rdfs:isDefinedBy <https://w3id.org/pmd/co.owl> ;
                                        <http://www.w3.org/2004/02/skos/core#definition> "A role indicating that its bearer has inititated a process."@en ,
                                                                                         "Initiator Role"@en .


###  https://w3id.org/pmd/co/LaboratoryRole
<https://w3id.org/pmd/co/LaboratoryRole> rdf:type owl:Class ;
                                         rdfs:subClassOf [ rdf:type owl:Restriction ;
                                                           owl:onProperty [ owl:inverseOf <http://purl.obolibrary.org/obo/RO_0000087>
                                                                          ] ;
                                                           owl:someValuesFrom <http://www.w3.org/ns/prov#Organization>
                                                         ] ;
                                         rdfs:isDefinedBy <https://w3id.org/pmd/co.owl> ;
                                         rdfs:label "Laboratory Role"@en ;
                                         <http://www.w3.org/2004/02/skos/core#definition> "A role indicating that an organization participates in a process as laboratory."@de .


###  https://w3id.org/pmd/co/Object
<https://w3id.org/pmd/co/Object> rdf:type owl:Class ;
                                 rdfs:isDefinedBy <https://w3id.org/pmd/co> ;
                                 rdfs:label "Object"@en ,
                                            "Objekt"@de ;
                                 <http://www.w3.org/2004/02/skos/core#definition> "A discernable, tangible or simulated entity that is processed in a process by a processing node."@en .


###  https://w3id.org/pmd/co/OperatorRole
<https://w3id.org/pmd/co/OperatorRole> rdf:type owl:Class ;
                                       rdfs:isDefinedBy <https://w3id.org/pmd/co.owl> ;
                                       rdfs:label "Operator Role"@en ;
                                       <http://www.w3.org/2004/02/skos/core#definition> "A role indicating that its bearer participates a process as operator."@en .


###  https://w3id.org/pmd/co/Process
<https://w3id.org/pmd/co/Process> rdf:type owl:Class ;
                                  <http://purl.obolibrary.org/obo/IAO_0000117> "A process is an activity comprising a series of actions or operations conducing to an end. In PMD, a process is conducted via processing nodes and has a discernable duration as part of a workflow. A process consumes objects and parameters. A process potentially generates new objects and measurements."@en ;
                                  rdfs:isDefinedBy <https://w3id.org/pmd/co> ;
                                  rdfs:label "Process"@en ,
                                             "Prozess"@de ;
                                  <http://www.w3.org/2004/02/skos/core#definition> "A process is an activity including a series of actions or operations conducing to an end. In PMD, a process is conducted via processing nodes and has a discernable duration as part of a workflow. A process consumes objects and parameters. A process potentially generates new objects and measurements."@en .


###  https://w3id.org/pmd/co/ProcessDescription
<https://w3id.org/pmd/co/ProcessDescription> rdf:type owl:Class ;
                                             owl:equivalentClass [ owl:intersectionOf ( <https://w3id.org/pmd/co/Description>
                                                                                        [ rdf:type owl:Restriction ;
                                                                                          owl:onProperty <https://w3id.org/pmd/co/characteristicOf> ;
                                                                                          owl:someValuesFrom <https://w3id.org/pmd/co/Process>
                                                                                        ]
                                                                                      ) ;
                                                                   rdf:type owl:Class
                                                                 ] ;
                                             rdfs:subClassOf <https://w3id.org/pmd/co/Description> ;
                                             rdfs:isDefinedBy <https://w3id.org/pmd/co> ;
                                             rdfs:label "Process Description"@en ,
                                                        "Prozessbeschreibung"@de ;
                                             <http://www.w3.org/2004/02/skos/core#definition> "A descriptive text qualifying the nature of a process instance used as an identifier that is not strictly intended to be unique, e.g. \"1050°C30 840°C10/ÖL\"."@en ,
                                                                                              "A human readable order of steps. Might include additional information that likes sketches and notes."@en .


###  https://w3id.org/pmd/co/Project
<https://w3id.org/pmd/co/Project> rdf:type owl:Class ;
                                  rdfs:isDefinedBy <https://w3id.org/pmd/co> ;
                                  rdfs:label "Project"@en ,
                                             "Projekt"@de ;
                                  <http://www.w3.org/2004/02/skos/core#definition> "A series of goal-orientated (intent) activities and interactions to achieve a specific outcome."@en ,
                                                                                   "Eine Reihe von zielorientierten (absichtlichen) Aktivitäten und Interaktionen, um ein bestimmtes Ergebnis zu erzielen."@de .


###  https://w3id.org/pmd/co/ProjectIdentifier
<https://w3id.org/pmd/co/ProjectIdentifier> rdf:type owl:Class ;
                                            owl:equivalentClass [ owl:intersectionOf ( <https://w3id.org/pmd/co/Identifier>
                                                                                       [ rdf:type owl:Restriction ;
                                                                                         owl:onProperty <https://w3id.org/pmd/co/characteristicOf> ;
                                                                                         owl:someValuesFrom <https://w3id.org/pmd/co/Project>
                                                                                       ]
                                                                                     ) ;
                                                                  rdf:type owl:Class
                                                                ] ;
                                            rdfs:subClassOf <https://w3id.org/pmd/co/Identifier> ;
                                            rdfs:isDefinedBy <https://w3id.org/pmd/co> ;
                                            rdfs:label "Project Identifier"@en ,
                                                       "Projektidentifikator"@de ;
                                            <http://www.w3.org/2004/02/skos/core#definition> "A colloquial, human-generated, descriptive text qualifying the nature of a project."@en ,
                                                                                             "Ein umgangssprachlicher, von Menschen erstellter, beschreibender Text, der die Art eines Projekts qualifiziert."@de .


###  https://w3id.org/pmd/co/RelatedProjectIdentifier
<https://w3id.org/pmd/co/RelatedProjectIdentifier> rdf:type owl:Class ;
                                                   rdfs:subClassOf <https://w3id.org/pmd/co/Identifier> ;
                                                   rdfs:isDefinedBy <https://w3id.org/pmd/co> ;
                                                   rdfs:label "Identifikation Eines Verbundenen Projektes"@de ,
                                                              "Related Project Identifier"@en ;
                                                   <http://www.w3.org/2004/02/skos/core#definition> "Diese Eigenschaft beschreibt einen benannten Wert, der dazu dient, zwischen Projekten zu unterscheiden, die mit dem betrachteten Projekt in Relation stehen. Zwei in Relation stehende Projekte könnten zum Beispiel ein Messprojekt sein, das Teil eines Projekts mit einem breiteren Betrachtungsbereich ist."@de ,
                                                                                                    "This property describes a named value intended to distinguish between projects that are related to the project considered. For instance, two related projects could be a measurement project that is part of project with a broader scope."@en .


###  https://w3id.org/pmd/co/SimulationProcess
<https://w3id.org/pmd/co/SimulationProcess> rdf:type owl:Class ;
                                            rdfs:subClassOf <https://w3id.org/pmd/co/Process> ;
                                            rdfs:isDefinedBy <https://w3id.org/pmd/co> ;
                                            rdfs:label "Simulation Process"@en ,
                                                       "Simulationsprozess"@de ;
                                            <http://www.w3.org/2004/02/skos/core#definition> "A process that is used for a simulation." .


###  https://w3id.org/pmd/co/TransformativeAnalysisProcess
<https://w3id.org/pmd/co/TransformativeAnalysisProcess> rdf:type owl:Class ;
                                                        rdfs:subClassOf <https://w3id.org/pmd/co/AnalysingProcess> ;
                                                        rdfs:isDefinedBy <https://w3id.org/pmd/co> ;
                                                        rdfs:label "Transformative Analysis Process"@en ,
                                                                   "Transformativer Analyseprozess"@de ;
                                                        <http://www.w3.org/2004/02/skos/core#definition> "An analysis process that is transformative."@en .


#################################################################
#    Individuals
#################################################################

###  http://purl.obolibrary.org/obo/IAO_0000002
<http://purl.obolibrary.org/obo/IAO_0000002> rdf:type owl:NamedIndividual ;
                                             <http://purl.obolibrary.org/obo/IAO_0000111> "example to be eventually removed"@en ;
                                             rdfs:isDefinedBy <http://purl.obolibrary.org/obo/iao.owl> ;
                                             rdfs:label "example to be eventually removed"@en .


###  http://purl.obolibrary.org/obo/IAO_0000120
<http://purl.obolibrary.org/obo/IAO_0000120> rdf:type owl:NamedIndividual ;
                                             <http://purl.obolibrary.org/obo/IAO_0000111> "metadata complete"@en ;
                                             <http://purl.obolibrary.org/obo/IAO_0000115> "Class has all its metadata, but is either not guaranteed to be in its final location in the asserted IS_A hierarchy or refers to another class that is not complete."@en ;
                                             rdfs:isDefinedBy <http://purl.obolibrary.org/obo/iao.owl> ;
                                             rdfs:label "metadata complete"@en .


###  http://purl.obolibrary.org/obo/IAO_0000121
<http://purl.obolibrary.org/obo/IAO_0000121> rdf:type owl:NamedIndividual ;
                                             <http://purl.obolibrary.org/obo/IAO_0000111> "organizational term"@en ;
                                             <http://purl.obolibrary.org/obo/IAO_0000115> "Term created to ease viewing/sort terms for development purpose, and will not be included in a release"@en ;
                                             rdfs:isDefinedBy <http://purl.obolibrary.org/obo/iao.owl> ;
                                             rdfs:label "organizational term"@en .


###  http://purl.obolibrary.org/obo/IAO_0000122
<http://purl.obolibrary.org/obo/IAO_0000122> rdf:type owl:NamedIndividual ;
                                             <http://purl.obolibrary.org/obo/IAO_0000111> "ready for release"@en ;
                                             <http://purl.obolibrary.org/obo/IAO_0000115> "Class has undergone final review, is ready for use, and will be included in the next release. Any class lacking \"ready_for_release\" should be considered likely to change place in hierarchy, have its definition refined, or be obsoleted in the next release.  Those classes deemed \"ready_for_release\" will also derived from a chain of ancestor classes that are also \"ready_for_release.\""@en ;
                                             rdfs:isDefinedBy <http://purl.obolibrary.org/obo/iao.owl> ;
                                             rdfs:label "ready for release"@en .


###  http://purl.obolibrary.org/obo/IAO_0000123
<http://purl.obolibrary.org/obo/IAO_0000123> rdf:type owl:NamedIndividual ;
                                             <http://purl.obolibrary.org/obo/IAO_0000111> "metadata incomplete"@en ;
                                             <http://purl.obolibrary.org/obo/IAO_0000115> "Class is being worked on; however, the metadata (including definition) are not complete or sufficiently clear to the branch editors."@en ;
                                             rdfs:isDefinedBy <http://purl.obolibrary.org/obo/iao.owl> ;
                                             rdfs:label "metadata incomplete"@en .


###  http://purl.obolibrary.org/obo/IAO_0000124
<http://purl.obolibrary.org/obo/IAO_0000124> rdf:type owl:NamedIndividual ;
                                             <http://purl.obolibrary.org/obo/IAO_0000111> "uncurated"@en ;
                                             <http://purl.obolibrary.org/obo/IAO_0000115> "Nothing done yet beyond assigning a unique class ID and proposing a preferred term."@en ;
                                             rdfs:isDefinedBy <http://purl.obolibrary.org/obo/iao.owl> ;
                                             rdfs:label "uncurated"@en .


###  http://purl.obolibrary.org/obo/IAO_0000125
<http://purl.obolibrary.org/obo/IAO_0000125> rdf:type owl:NamedIndividual ;
                                             <http://purl.obolibrary.org/obo/IAO_0000111> "pending final vetting"@en ;
                                             <http://purl.obolibrary.org/obo/IAO_0000115> "All definitions, placement in the asserted IS_A hierarchy and required minimal metadata are complete. The class is awaiting a final review by someone other than the term editor."@en ;
                                             rdfs:isDefinedBy <http://purl.obolibrary.org/obo/iao.owl> ;
                                             rdfs:label "pending final vetting"@en .


###  http://purl.obolibrary.org/obo/IAO_0000423
<http://purl.obolibrary.org/obo/IAO_0000423> rdf:type owl:NamedIndividual ;
                                             <http://purl.obolibrary.org/obo/IAO_0000111> "to be replaced with external ontology term"@en ;
                                             <http://purl.obolibrary.org/obo/IAO_0000115> "Terms with this status should eventually replaced with a term from another ontology."@en ;
                                             <http://purl.obolibrary.org/obo/IAO_0000117> "Alan Ruttenberg"@en ;
                                             <http://purl.obolibrary.org/obo/IAO_0000119> "group:OBI"@en ;
                                             rdfs:isDefinedBy <http://purl.obolibrary.org/obo/iao.owl> ;
                                             rdfs:label "to be replaced with external ontology term"@en .


###  http://purl.obolibrary.org/obo/IAO_0000428
<http://purl.obolibrary.org/obo/IAO_0000428> rdf:type owl:NamedIndividual ;
                                             <http://purl.obolibrary.org/obo/IAO_0000115> "A term that is metadata complete, has been reviewed, and problems have been identified that require discussion before release. Such a term requires editor note(s) to identify the outstanding issues."@en ;
                                             rdfs:isDefinedBy <http://purl.obolibrary.org/obo/iao.owl> ;
                                             rdfs:label "requires discussion"@en .


#################################################################
#    Annotations
#################################################################

<http://www.w3.org/2004/02/skos/core#example> rdfs:isDefinedBy <http://www.w3.org/2004/02/skos/core.owl> .


#################################################################
#    Rules
#################################################################

<https://w3id.org/pmd/co/p1> rdf:type <http://www.w3.org/2003/11/swrl#Variable> .

<https://w3id.org/pmd/co/o2> rdf:type <http://www.w3.org/2003/11/swrl#Variable> .

<https://w3id.org/pmd/co/o1> rdf:type <http://www.w3.org/2003/11/swrl#Variable> .

[ <http://swrl.stanford.edu/ontologies/3.3/swrla.owl#isRuleEnabled> "true"^^xsd:boolean ;
   rdfs:comment "" ;
   rdfs:label "S2" ;
   rdf:type <http://www.w3.org/2003/11/swrl#Imp> ;
   <http://www.w3.org/2003/11/swrl#body> [ rdf:type <http://www.w3.org/2003/11/swrl#AtomList> ;
                                           rdf:first [ rdf:type <http://www.w3.org/2003/11/swrl#IndividualPropertyAtom> ;
                                                       <http://www.w3.org/2003/11/swrl#propertyPredicate> <https://w3id.org/pmd/co/output> ;
                                                       <http://www.w3.org/2003/11/swrl#argument1> <https://w3id.org/pmd/co/p1> ;
                                                       <http://www.w3.org/2003/11/swrl#argument2> <https://w3id.org/pmd/co/o2>
                                                     ] ;
                                           rdf:rest [ rdf:type <http://www.w3.org/2003/11/swrl#AtomList> ;
                                                      rdf:first [ rdf:type <http://www.w3.org/2003/11/swrl#IndividualPropertyAtom> ;
                                                                  <http://www.w3.org/2003/11/swrl#propertyPredicate> <https://w3id.org/pmd/co/input> ;
                                                                  <http://www.w3.org/2003/11/swrl#argument1> <https://w3id.org/pmd/co/p1> ;
                                                                  <http://www.w3.org/2003/11/swrl#argument2> <https://w3id.org/pmd/co/o1>
                                                                ] ;
                                                      rdf:rest [ rdf:type <http://www.w3.org/2003/11/swrl#AtomList> ;
                                                                 rdf:first [ rdf:type <http://www.w3.org/2003/11/swrl#ClassAtom> ;
                                                                             <http://www.w3.org/2003/11/swrl#classPredicate> <https://w3id.org/pmd/co/Process> ;
                                                                             <http://www.w3.org/2003/11/swrl#argument1> <https://w3id.org/pmd/co/p1>
                                                                           ] ;
                                                                 rdf:rest rdf:nil
                                                               ]
                                                    ]
                                         ] ;
   <http://www.w3.org/2003/11/swrl#head> [ rdf:type <http://www.w3.org/2003/11/swrl#AtomList> ;
                                           rdf:first [ rdf:type <http://www.w3.org/2003/11/swrl#IndividualPropertyAtom> ;
                                                       <http://www.w3.org/2003/11/swrl#propertyPredicate> <http://www.w3.org/ns/prov#wasDerivedFrom> ;
                                                       <http://www.w3.org/2003/11/swrl#argument1> <https://w3id.org/pmd/co/o2> ;
                                                       <http://www.w3.org/2003/11/swrl#argument2> <https://w3id.org/pmd/co/o1>
                                                     ] ;
                                           rdf:rest rdf:nil
                                         ]
 ] .

###  Generated by the OWL API (version 4.5.29) https://github.com/owlcs/owlapi
