<?xml version="1.0"?>
<rdf:RDF xmlns="https://w3id.org/pmd/co#"
     xml:base="https://w3id.org/pmd/co"
     xmlns:obo="http://purl.obolibrary.org/obo/"
     xmlns:owl="http://www.w3.org/2002/07/owl#"
     xmlns:rdf="http://www.w3.org/1999/02/22-rdf-syntax-ns#"
     xmlns:xml="http://www.w3.org/XML/1998/namespace"
     xmlns:xsd="http://www.w3.org/2001/XMLSchema#"
     xmlns:rdfs="http://www.w3.org/2000/01/rdf-schema#"
     xmlns:skos="http://www.w3.org/2004/02/skos/core#"
     xmlns:swrl="http://www.w3.org/2003/11/swrl#"
     xmlns:swrla="http://swrl.stanford.edu/ontologies/3.3/swrla.owl#"
     xmlns:swrlb="http://www.w3.org/2003/11/swrlb#">
    <owl:Ontology rdf:about="https://w3id.org/pmd/co"/>
    


    <!-- 
    ///////////////////////////////////////////////////////////////////////////////////////
    //
    // Annotation properties
    //
    ///////////////////////////////////////////////////////////////////////////////////////
     -->

    


    <!-- http://purl.obolibrary.org/obo/IAO_0000111 -->

    <owl:AnnotationProperty rdf:about="http://purl.obolibrary.org/obo/IAO_0000111">
        <rdfs:isDefinedBy rdf:resource="http://purl.obolibrary.org/obo/iao.owl"/>
    </owl:AnnotationProperty>
    


    <!-- http://purl.obolibrary.org/obo/IAO_0000115 -->

    <owl:AnnotationProperty rdf:about="http://purl.obolibrary.org/obo/IAO_0000115">
        <rdfs:isDefinedBy rdf:resource="http://purl.obolibrary.org/obo/iao.owl"/>
    </owl:AnnotationProperty>
    


    <!-- http://purl.obolibrary.org/obo/IAO_0000117 -->

    <owl:AnnotationProperty rdf:about="http://purl.obolibrary.org/obo/IAO_0000117">
        <rdfs:isDefinedBy rdf:resource="http://purl.obolibrary.org/obo/iao.owl"/>
    </owl:AnnotationProperty>
    


    <!-- http://purl.obolibrary.org/obo/IAO_0000119 -->

    <owl:AnnotationProperty rdf:about="http://purl.obolibrary.org/obo/IAO_0000119">
        <rdfs:isDefinedBy rdf:resource="http://purl.obolibrary.org/obo/iao.owl"/>
    </owl:AnnotationProperty>
    


    <!-- http://swrl.stanford.edu/ontologies/3.3/swrla.owl#isRuleEnabled -->

    <owl:AnnotationProperty rdf:about="http://swrl.stanford.edu/ontologies/3.3/swrla.owl#isRuleEnabled">
        <rdfs:isDefinedBy rdf:resource="http://swrl.stanford.edu/ontologies/3.3/swrla.owl"/>
    </owl:AnnotationProperty>
    


    <!-- http://www.w3.org/2000/01/rdf-schema#comment -->

    <rdf:Description rdf:about="http://www.w3.org/2000/01/rdf-schema#comment">
        <rdfs:isDefinedBy rdf:resource="http://www.w3.org/2000/01/rdf-schema.owl"/>
    </rdf:Description>
    


    <!-- http://www.w3.org/2000/01/rdf-schema#isDefinedBy -->

    <rdf:Description rdf:about="http://www.w3.org/2000/01/rdf-schema#isDefinedBy">
        <rdfs:isDefinedBy rdf:resource="http://www.w3.org/2000/01/rdf-schema.owl"/>
    </rdf:Description>
    


    <!-- http://www.w3.org/2000/01/rdf-schema#label -->

    <rdf:Description rdf:about="http://www.w3.org/2000/01/rdf-schema#label">
        <rdfs:isDefinedBy rdf:resource="http://www.w3.org/2000/01/rdf-schema.owl"/>
    </rdf:Description>
    


    <!-- http://www.w3.org/2004/02/skos/core#altLabel -->

    <owl:AnnotationProperty rdf:about="http://www.w3.org/2004/02/skos/core#altLabel">
        <rdfs:isDefinedBy rdf:resource="http://www.w3.org/2004/02/skos/core.owl"/>
    </owl:AnnotationProperty>
    


    <!-- http://www.w3.org/2004/02/skos/core#definition -->

    <owl:AnnotationProperty rdf:about="http://www.w3.org/2004/02/skos/core#definition">
        <rdfs:isDefinedBy rdf:resource="http://www.w3.org/2004/02/skos/core.owl"/>
    </owl:AnnotationProperty>
    


    <!-- 
    ///////////////////////////////////////////////////////////////////////////////////////
    //
    // Datatypes
    //
    ///////////////////////////////////////////////////////////////////////////////////////
     -->

    


    <!-- http://www.w3.org/1999/02/22-rdf-syntax-ns#PlainLiteral -->

    <rdf:Description rdf:about="http://www.w3.org/1999/02/22-rdf-syntax-ns#PlainLiteral">
        <rdfs:isDefinedBy rdf:resource="http://www.w3.org/1999/02/22-rdf-syntax-ns.owl"/>
    </rdf:Description>
    


    <!-- http://www.w3.org/2001/XMLSchema#boolean -->

    <rdf:Description rdf:about="http://www.w3.org/2001/XMLSchema#boolean">
        <rdfs:isDefinedBy rdf:resource="http://www.w3.org/2001/xmlschema.owl"/>
    </rdf:Description>
    


    <!-- 
    ///////////////////////////////////////////////////////////////////////////////////////
    //
    // Object Properties
    //
    ///////////////////////////////////////////////////////////////////////////////////////
     -->

    


    <!-- http://www.w3.org/ns/prov#wasDerivedFrom -->

    <owl:ObjectProperty rdf:about="http://www.w3.org/ns/prov#wasDerivedFrom">
        <rdfs:isDefinedBy rdf:resource="http://www.w3.org/ns/prov.owl"/>
    </owl:ObjectProperty>
    


    <!-- https://w3id.org/pmd/co/characteristic -->

    <owl:ObjectProperty rdf:about="https://w3id.org/pmd/co/characteristic">
        <owl:inverseOf rdf:resource="https://w3id.org/pmd/co/characteristicOf"/>
        <rdfs:isDefinedBy rdf:resource="https://w3id.org/pmd/co"/>
        <rdfs:label xml:lang="en">characteristic</rdfs:label>
        <skos:altLabel xml:lang="en">has characteristic</skos:altLabel>
        <skos:definition xml:lang="de">Die Objekteigenschaft characterisitc, wird in Verbindung mit ProzessKnoten, Prozess und Objekt verwendet und dient zur Herstellung einer Verbindung mit dem WerteObjekt. Diese Eigenschaft ermöglicht die Abbildung von Beziehungen zwischen ProzessKnoten, Prozessen und Objekten und den dazugehörigen Werten oder Attributen (Metadaten), die in WerteObjekt ausgedrückt sind.</skos:definition>
        <skos:definition xml:lang="en">The object property characteristic, in conjunction with ProcessingNode, Process and Object, is used to establish a connection with ValueObjects. This property enables the representation of relationships between ProcessingNodes, Processes and Objects and the associated values or attributes (metadata) that are stored in ValueObjects.</skos:definition>
    </owl:ObjectProperty>
    


    <!-- https://w3id.org/pmd/co/characteristicOf -->

    <owl:ObjectProperty rdf:about="https://w3id.org/pmd/co/characteristicOf">
        <rdfs:isDefinedBy rdf:resource="https://w3id.org/pmd/co"/>
        <rdfs:label xml:lang="en">characteristic of</rdfs:label>
        <skos:altLabel>is characteristic of</skos:altLabel>
    </owl:ObjectProperty>
    


    <!-- https://w3id.org/pmd/co/component -->

    <owl:ObjectProperty rdf:about="https://w3id.org/pmd/co/component">
        <rdfs:domain rdf:resource="https://w3id.org/pmd/co/ProcessingNode"/>
        <rdfs:isDefinedBy rdf:resource="https://w3id.org/pmd/co"/>
        <rdfs:label xml:lang="en">component</rdfs:label>
        <skos:altLabel xml:lang="en">has component</skos:altLabel>
        <skos:definition xml:lang="de">Die Objekt-Eigenschaft Komponente, die in Verbindung mit ProzessKnoten und seinen (modularen) Elementen verwendet wird. Sie ermöglicht die Darstellung der einzelnen, unterschiedlichen Teile von ProzessKnoten. Im Wesentlichen ist die  &quot;Komponenten-Eigenschaft&quot; eine Möglichkeit, ein komplexes System in überschaubare und eindeutige Teile zu zerlegen, um die Rolle der einzelnen Teile innerhalb des Gesamtsystems zu verstehen und zu verwalten.</skos:definition>
        <skos:definition xml:lang="en">The object property component, which is used in connection with ProcessingNode and its (modular) elements. It enables the representation of the individual, different parts of processing nodes. Essentially, the &apos;component property&apos; is a way of breaking down a complex system into manageable and distinct parts in order to understand and manage the role of each part within the overall system.</skos:definition>
    </owl:ObjectProperty>
    


    <!-- https://w3id.org/pmd/co/executedBy -->

    <owl:ObjectProperty rdf:about="https://w3id.org/pmd/co/executedBy">
        <owl:inverseOf rdf:resource="https://w3id.org/pmd/co/executes"/>
        <rdfs:domain rdf:resource="https://w3id.org/pmd/co/Process"/>
        <rdfs:range rdf:resource="https://w3id.org/pmd/co/ProcessingNode"/>
        <rdfs:isDefinedBy rdf:resource="https://w3id.org/pmd/co"/>
        <rdfs:label xml:lang="en">executed by</rdfs:label>
        <skos:definition xml:lang="en">This property represents which process is executed by which process node.</skos:definition>
    </owl:ObjectProperty>
    


    <!-- https://w3id.org/pmd/co/executes -->

    <owl:ObjectProperty rdf:about="https://w3id.org/pmd/co/executes">
        <rdfs:domain rdf:resource="https://w3id.org/pmd/co/ProcessingNode"/>
        <rdfs:range rdf:resource="https://w3id.org/pmd/co/Process"/>
        <rdfs:isDefinedBy rdf:resource="https://w3id.org/pmd/co"/>
        <rdfs:label xml:lang="en">executes</rdfs:label>
        <skos:definition xml:lang="en">This property represents which ProcessingNode executes a Process.</skos:definition>
    </owl:ObjectProperty>
    


    <!-- https://w3id.org/pmd/co/input -->

    <owl:ObjectProperty rdf:about="https://w3id.org/pmd/co/input">
        <rdfs:subPropertyOf rdf:resource="https://w3id.org/pmd/co/participant"/>
        <owl:inverseOf rdf:resource="https://w3id.org/pmd/co/inputOf"/>
        <rdfs:isDefinedBy rdf:resource="https://w3id.org/pmd/co"/>
        <rdfs:label xml:lang="en">input</rdfs:label>
        <skos:altLabel>has input</skos:altLabel>
        <skos:definition xml:lang="en">This property is used to link the processes to their input objects.</skos:definition>
    </owl:ObjectProperty>
    


    <!-- https://w3id.org/pmd/co/inputOf -->

    <owl:ObjectProperty rdf:about="https://w3id.org/pmd/co/inputOf">
        <rdfs:subPropertyOf rdf:resource="https://w3id.org/pmd/co/participantOf"/>
        <rdfs:isDefinedBy rdf:resource="https://w3id.org/pmd/co"/>
        <rdfs:label xml:lang="en">input of</rdfs:label>
        <skos:altLabel>is input of</skos:altLabel>
    </owl:ObjectProperty>
    


    <!-- https://w3id.org/pmd/co/nextProcess -->

    <owl:ObjectProperty rdf:about="https://w3id.org/pmd/co/nextProcess">
        <owl:inverseOf rdf:resource="https://w3id.org/pmd/co/previousProcess"/>
        <rdfs:domain rdf:resource="https://w3id.org/pmd/co/Process"/>
        <rdfs:range rdf:resource="https://w3id.org/pmd/co/Process"/>
        <rdfs:isDefinedBy rdf:resource="https://w3id.org/pmd/co"/>
        <rdfs:label xml:lang="en">next process</rdfs:label>
        <skos:altLabel xml:lang="en">has next process</skos:altLabel>
        <skos:definition xml:lang="en">This property is used to indicate the process that was run after the current process.</skos:definition>
    </owl:ObjectProperty>
    


    <!-- https://w3id.org/pmd/co/output -->

    <owl:ObjectProperty rdf:about="https://w3id.org/pmd/co/output">
        <rdfs:subPropertyOf rdf:resource="https://w3id.org/pmd/co/participant"/>
        <owl:inverseOf rdf:resource="https://w3id.org/pmd/co/outputOf"/>
        <rdfs:isDefinedBy rdf:resource="https://w3id.org/pmd/co"/>
        <rdfs:label xml:lang="en">output</rdfs:label>
        <skos:altLabel>has output</skos:altLabel>
        <skos:definition xml:lang="en">This property is used to link the processes to their output objects</skos:definition>
    </owl:ObjectProperty>
    


    <!-- https://w3id.org/pmd/co/outputOf -->

    <owl:ObjectProperty rdf:about="https://w3id.org/pmd/co/outputOf">
        <rdfs:subPropertyOf rdf:resource="https://w3id.org/pmd/co/participantOf"/>
        <rdfs:isDefinedBy rdf:resource="https://w3id.org/pmd/co"/>
        <rdfs:label xml:lang="en">output of</rdfs:label>
        <skos:altLabel xml:lang="en">is output of</skos:altLabel>
    </owl:ObjectProperty>
    


    <!-- https://w3id.org/pmd/co/participant -->

    <owl:ObjectProperty rdf:about="https://w3id.org/pmd/co/participant">
        <owl:inverseOf rdf:resource="https://w3id.org/pmd/co/participantOf"/>
        <rdfs:domain rdf:resource="https://w3id.org/pmd/co/Process"/>
        <rdfs:isDefinedBy rdf:resource="https://w3id.org/pmd/co"/>
        <rdfs:label xml:lang="en">participant</rdfs:label>
        <skos:altLabel>has participant</skos:altLabel>
        <skos:definition xml:lang="en">A relation between a process and an object, in which the objects is somehow involved in the process.</skos:definition>
    </owl:ObjectProperty>
    


    <!-- https://w3id.org/pmd/co/participantOf -->

    <owl:ObjectProperty rdf:about="https://w3id.org/pmd/co/participantOf">
        <rdfs:isDefinedBy rdf:resource="https://w3id.org/pmd/co"/>
        <rdfs:label xml:lang="en">participant of</rdfs:label>
        <skos:altLabel xml:lang="en">is participant of</skos:altLabel>
    </owl:ObjectProperty>
    


    <!-- https://w3id.org/pmd/co/previousProcess -->

    <owl:ObjectProperty rdf:about="https://w3id.org/pmd/co/previousProcess">
        <rdfs:domain rdf:resource="https://w3id.org/pmd/co/Process"/>
        <rdfs:range rdf:resource="https://w3id.org/pmd/co/Process"/>
        <rdfs:isDefinedBy rdf:resource="https://w3id.org/pmd/co"/>
        <rdfs:label xml:lang="en">previous process</rdfs:label>
        <skos:altLabel>has previous process</skos:altLabel>
        <skos:definition xml:lang="en">This property is used to indicate that which process was previously run.</skos:definition>
    </owl:ObjectProperty>
    


    <!-- https://w3id.org/pmd/co/subordinateProcess -->

    <owl:ObjectProperty rdf:about="https://w3id.org/pmd/co/subordinateProcess">
        <owl:inverseOf rdf:resource="https://w3id.org/pmd/co/superordinateProcess"/>
        <rdfs:domain rdf:resource="https://w3id.org/pmd/co/Process"/>
        <rdfs:range rdf:resource="https://w3id.org/pmd/co/Process"/>
        <rdfs:isDefinedBy rdf:resource="https://w3id.org/pmd/co"/>
        <rdfs:label xml:lang="en">subordinate process</rdfs:label>
        <skos:altLabel>has subordinate process</skos:altLabel>
        <skos:definition xml:lang="en">This property is used to link a process to its subordinate processes.</skos:definition>
    </owl:ObjectProperty>
    


    <!-- https://w3id.org/pmd/co/superordinateProcess -->

    <owl:ObjectProperty rdf:about="https://w3id.org/pmd/co/superordinateProcess">
        <rdfs:isDefinedBy rdf:resource="https://w3id.org/pmd/co"/>
        <rdfs:label xml:lang="en">superordinate process</rdfs:label>
        <skos:altLabel xml:lang="en">has superordinate process</skos:altLabel>
        <skos:definition xml:lang="en">This property is used to link a process to its super ordinated processes.</skos:definition>
    </owl:ObjectProperty>
    


    <!-- 
    ///////////////////////////////////////////////////////////////////////////////////////
    //
    // Data properties
    //
    ///////////////////////////////////////////////////////////////////////////////////////
     -->

    


    <!-- https://w3id.org/pmd/co/value -->

    <owl:DatatypeProperty rdf:about="https://w3id.org/pmd/co/value">
        <rdfs:isDefinedBy rdf:resource="https://w3id.org/pmd/co"/>
        <rdfs:label xml:lang="de">hat Wert</rdfs:label>
        <rdfs:label xml:lang="en">value</rdfs:label>
        <skos:definition xml:lang="en">Provides the actual value a value object is referring to.</skos:definition>
    </owl:DatatypeProperty>
    


    <!-- 
    ///////////////////////////////////////////////////////////////////////////////////////
    //
    // Classes
    //
    ///////////////////////////////////////////////////////////////////////////////////////
     -->

    


    <!-- https://w3id.org/pmd/co/Process -->

    <owl:Class rdf:about="https://w3id.org/pmd/co/Process">
        <obo:IAO_0000117 xml:lang="en">A process is an activity comprising a series of actions or operations conducing to an end. In PMD, a process is conducted via processing nodes and has a discernable duration as part of a workflow. A process consumes objects and parameters. A process potentially generates new objects and measurements.</obo:IAO_0000117>
        <rdfs:isDefinedBy rdf:resource="https://w3id.org/pmd/co"/>
        <rdfs:label xml:lang="en">Process</rdfs:label>
        <rdfs:label xml:lang="de">Prozess</rdfs:label>
        <skos:definition xml:lang="en">A process is an activity including a series of actions or operations conducing to an end. In PMD, a process is conducted via processing nodes and has a discernable duration as part of a workflow. A process consumes objects and parameters. A process potentially generates new objects and measurements.</skos:definition>
    </owl:Class>
    


    <!-- https://w3id.org/pmd/co/ProcessingNode -->

    <owl:Class rdf:about="https://w3id.org/pmd/co/ProcessingNode">
        <rdfs:isDefinedBy rdf:resource="https://w3id.org/pmd/co"/>
        <rdfs:label xml:lang="en">Processing Node</rdfs:label>
        <rdfs:label xml:lang="de">Prozessknoten</rdfs:label>
        <skos:definition xml:lang="en">Processing nodes are tools, equipment and accessories as well as software that are relevant for the performance of processes, such as e.g. mechanical and chemical test as well as simulation, prediction, and machine learning. Accordingly, processing nodes may be machines, parts of machines, and software applications.</skos:definition>
        <skos:definition xml:lang="de">Prozessknoten sind Werkzeuge, Geräte und Zubehör sowie Software, die für die Durchführung von Prozessen relevant sind, wie z. B. mechanische und chemische Tests sowie Simulationen, Vorhersagen und maschinelles Lernen. Dementsprechend können Prozessknoten Maschinen, Teile von Maschinen und Softwareanwendungen sein.</skos:definition>
    </owl:Class>
    


    <!-- 
    ///////////////////////////////////////////////////////////////////////////////////////
    //
    // Annotations
    //
    ///////////////////////////////////////////////////////////////////////////////////////
     -->

    <rdf:Description rdf:about="http://purl.obolibrary.org/obo/IAO_0000002">
        <obo:IAO_0000111 xml:lang="en">example to be eventually removed</obo:IAO_0000111>
        <rdfs:isDefinedBy rdf:resource="http://purl.obolibrary.org/obo/iao.owl"/>
        <rdfs:label xml:lang="en">example to be eventually removed</rdfs:label>
    </rdf:Description>
    <rdf:Description rdf:about="http://purl.obolibrary.org/obo/IAO_0000114">
        <rdfs:isDefinedBy rdf:resource="http://purl.obolibrary.org/obo/iao.owl"/>
    </rdf:Description>
    <rdf:Description rdf:about="http://purl.obolibrary.org/obo/IAO_0000120">
        <obo:IAO_0000111 xml:lang="en">metadata complete</obo:IAO_0000111>
        <obo:IAO_0000115 xml:lang="en">Class has all its metadata, but is either not guaranteed to be in its final location in the asserted IS_A hierarchy or refers to another class that is not complete.</obo:IAO_0000115>
        <rdfs:isDefinedBy rdf:resource="http://purl.obolibrary.org/obo/iao.owl"/>
        <rdfs:label xml:lang="en">metadata complete</rdfs:label>
    </rdf:Description>
    <rdf:Description rdf:about="http://purl.obolibrary.org/obo/IAO_0000121">
        <obo:IAO_0000111 xml:lang="en">organizational term</obo:IAO_0000111>
        <obo:IAO_0000115 xml:lang="en">Term created to ease viewing/sort terms for development purpose, and will not be included in a release</obo:IAO_0000115>
        <rdfs:isDefinedBy rdf:resource="http://purl.obolibrary.org/obo/iao.owl"/>
        <rdfs:label xml:lang="en">organizational term</rdfs:label>
    </rdf:Description>
    <rdf:Description rdf:about="http://purl.obolibrary.org/obo/IAO_0000122">
        <obo:IAO_0000111 xml:lang="en">ready for release</obo:IAO_0000111>
        <obo:IAO_0000115 xml:lang="en">Class has undergone final review, is ready for use, and will be included in the next release. Any class lacking &quot;ready_for_release&quot; should be considered likely to change place in hierarchy, have its definition refined, or be obsoleted in the next release.  Those classes deemed &quot;ready_for_release&quot; will also derived from a chain of ancestor classes that are also &quot;ready_for_release.&quot;</obo:IAO_0000115>
        <rdfs:isDefinedBy rdf:resource="http://purl.obolibrary.org/obo/iao.owl"/>
        <rdfs:label xml:lang="en">ready for release</rdfs:label>
    </rdf:Description>
    <rdf:Description rdf:about="http://purl.obolibrary.org/obo/IAO_0000123">
        <obo:IAO_0000111 xml:lang="en">metadata incomplete</obo:IAO_0000111>
        <obo:IAO_0000115 xml:lang="en">Class is being worked on; however, the metadata (including definition) are not complete or sufficiently clear to the branch editors.</obo:IAO_0000115>
        <rdfs:isDefinedBy rdf:resource="http://purl.obolibrary.org/obo/iao.owl"/>
        <rdfs:label xml:lang="en">metadata incomplete</rdfs:label>
    </rdf:Description>
    <rdf:Description rdf:about="http://purl.obolibrary.org/obo/IAO_0000124">
        <obo:IAO_0000111 xml:lang="en">uncurated</obo:IAO_0000111>
        <obo:IAO_0000115 xml:lang="en">Nothing done yet beyond assigning a unique class ID and proposing a preferred term.</obo:IAO_0000115>
        <rdfs:isDefinedBy rdf:resource="http://purl.obolibrary.org/obo/iao.owl"/>
        <rdfs:label xml:lang="en">uncurated</rdfs:label>
    </rdf:Description>
    <rdf:Description rdf:about="http://purl.obolibrary.org/obo/IAO_0000125">
        <obo:IAO_0000111 xml:lang="en">pending final vetting</obo:IAO_0000111>
        <obo:IAO_0000115 xml:lang="en">All definitions, placement in the asserted IS_A hierarchy and required minimal metadata are complete. The class is awaiting a final review by someone other than the term editor.</obo:IAO_0000115>
        <rdfs:isDefinedBy rdf:resource="http://purl.obolibrary.org/obo/iao.owl"/>
        <rdfs:label xml:lang="en">pending final vetting</rdfs:label>
    </rdf:Description>
    <rdf:Description rdf:about="http://purl.obolibrary.org/obo/IAO_0000423">
        <obo:IAO_0000111 xml:lang="en">to be replaced with external ontology term</obo:IAO_0000111>
        <obo:IAO_0000115 xml:lang="en">Terms with this status should eventually replaced with a term from another ontology.</obo:IAO_0000115>
        <obo:IAO_0000117 xml:lang="en">Alan Ruttenberg</obo:IAO_0000117>
        <obo:IAO_0000119 xml:lang="en">group:OBI</obo:IAO_0000119>
        <rdfs:isDefinedBy rdf:resource="http://purl.obolibrary.org/obo/iao.owl"/>
        <rdfs:label xml:lang="en">to be replaced with external ontology term</rdfs:label>
    </rdf:Description>
    <rdf:Description rdf:about="http://purl.obolibrary.org/obo/IAO_0000428">
        <obo:IAO_0000115 xml:lang="en">A term that is metadata complete, has been reviewed, and problems have been identified that require discussion before release. Such a term requires editor note(s) to identify the outstanding issues.</obo:IAO_0000115>
        <rdfs:isDefinedBy rdf:resource="http://purl.obolibrary.org/obo/iao.owl"/>
        <rdfs:label xml:lang="en">requires discussion</rdfs:label>
    </rdf:Description>
    <rdf:Description rdf:about="http://www.w3.org/2001/XMLSchema#string">
        <rdfs:isDefinedBy rdf:resource="http://www.w3.org/2001/xmlschema.owl"/>
    </rdf:Description>
    <rdf:Description rdf:about="http://www.w3.org/2004/02/skos/core#example">
        <rdfs:isDefinedBy rdf:resource="http://www.w3.org/2004/02/skos/core.owl"/>
    </rdf:Description>
    <rdf:Description rdf:about="https://w3id.org/pmd/co/definitionSource">
        <rdfs:isDefinedBy rdf:resource="https://w3id.org/pmd/co.owl"/>
    </rdf:Description>
    


    <!-- 
    ///////////////////////////////////////////////////////////////////////////////////////
    //
    // Rules
    //
    ///////////////////////////////////////////////////////////////////////////////////////
     -->

    <rdf:Description rdf:about="https://w3id.org/pmd/co/p1">
        <rdf:type rdf:resource="http://www.w3.org/2003/11/swrl#Variable"/>
    </rdf:Description>
    <rdf:Description rdf:about="https://w3id.org/pmd/co/o2">
        <rdf:type rdf:resource="http://www.w3.org/2003/11/swrl#Variable"/>
    </rdf:Description>
    <rdf:Description rdf:about="https://w3id.org/pmd/co/o1">
        <rdf:type rdf:resource="http://www.w3.org/2003/11/swrl#Variable"/>
    </rdf:Description>
    <rdf:Description>
        <swrla:isRuleEnabled rdf:datatype="http://www.w3.org/2001/XMLSchema#boolean">true</swrla:isRuleEnabled>
        <rdfs:comment></rdfs:comment>
        <rdfs:label>S2</rdfs:label>
        <rdf:type rdf:resource="http://www.w3.org/2003/11/swrl#Imp"/>
        <swrl:body>
            <rdf:Description>
                <rdf:type rdf:resource="http://www.w3.org/2003/11/swrl#AtomList"/>
                <rdf:first>
                    <rdf:Description>
                        <rdf:type rdf:resource="http://www.w3.org/2003/11/swrl#IndividualPropertyAtom"/>
                        <swrl:propertyPredicate rdf:resource="https://w3id.org/pmd/co/output"/>
                        <swrl:argument1 rdf:resource="https://w3id.org/pmd/co/p1"/>
                        <swrl:argument2 rdf:resource="https://w3id.org/pmd/co/o2"/>
                    </rdf:Description>
                </rdf:first>
                <rdf:rest>
                    <rdf:Description>
                        <rdf:type rdf:resource="http://www.w3.org/2003/11/swrl#AtomList"/>
                        <rdf:first>
                            <rdf:Description>
                                <rdf:type rdf:resource="http://www.w3.org/2003/11/swrl#IndividualPropertyAtom"/>
                                <swrl:propertyPredicate rdf:resource="https://w3id.org/pmd/co/input"/>
                                <swrl:argument1 rdf:resource="https://w3id.org/pmd/co/p1"/>
                                <swrl:argument2 rdf:resource="https://w3id.org/pmd/co/o1"/>
                            </rdf:Description>
                        </rdf:first>
                        <rdf:rest>
                            <rdf:Description>
                                <rdf:type rdf:resource="http://www.w3.org/2003/11/swrl#AtomList"/>
                                <rdf:first>
                                    <rdf:Description>
                                        <rdf:type rdf:resource="http://www.w3.org/2003/11/swrl#ClassAtom"/>
                                        <swrl:classPredicate rdf:resource="https://w3id.org/pmd/co/Process"/>
                                        <swrl:argument1 rdf:resource="https://w3id.org/pmd/co/p1"/>
                                    </rdf:Description>
                                </rdf:first>
                                <rdf:rest rdf:resource="http://www.w3.org/1999/02/22-rdf-syntax-ns#nil"/>
                            </rdf:Description>
                        </rdf:rest>
                    </rdf:Description>
                </rdf:rest>
            </rdf:Description>
        </swrl:body>
        <swrl:head>
            <rdf:Description>
                <rdf:type rdf:resource="http://www.w3.org/2003/11/swrl#AtomList"/>
                <rdf:first>
                    <rdf:Description>
                        <rdf:type rdf:resource="http://www.w3.org/2003/11/swrl#IndividualPropertyAtom"/>
                        <swrl:propertyPredicate rdf:resource="http://www.w3.org/ns/prov#wasDerivedFrom"/>
                        <swrl:argument1 rdf:resource="https://w3id.org/pmd/co/o2"/>
                        <swrl:argument2 rdf:resource="https://w3id.org/pmd/co/o1"/>
                    </rdf:Description>
                </rdf:first>
                <rdf:rest rdf:resource="http://www.w3.org/1999/02/22-rdf-syntax-ns#nil"/>
            </rdf:Description>
        </swrl:head>
    </rdf:Description>
</rdf:RDF>



<!-- Generated by the OWL API (version 4.5.29) https://github.com/owlcs/owlapi -->

