@prefix : <https://w3id.org/pmd/co#> .
@prefix owl: <http://www.w3.org/2002/07/owl#> .
@prefix rdf: <http://www.w3.org/1999/02/22-rdf-syntax-ns#> .
@prefix xml: <http://www.w3.org/XML/1998/namespace> .
@prefix xsd: <http://www.w3.org/2001/XMLSchema#> .
@prefix rdfs: <http://www.w3.org/2000/01/rdf-schema#> .
@base <https://w3id.org/pmd/co> .

<https://w3id.org/pmd/co> rdf:type owl:Ontology .

#################################################################
#    Annotation properties
#################################################################

###  http://purl.obolibrary.org/obo/IAO_0000111
<http://purl.obolibrary.org/obo/IAO_0000111> rdf:type owl:AnnotationProperty ;
                                             rdfs:isDefinedBy <http://purl.obolibrary.org/obo/iao.owl> .


###  http://purl.obolibrary.org/obo/IAO_0000115
<http://purl.obolibrary.org/obo/IAO_0000115> rdf:type owl:AnnotationProperty ;
                                             rdfs:isDefinedBy <http://purl.obolibrary.org/obo/iao.owl> .


###  http://purl.obolibrary.org/obo/IAO_0000117
<http://purl.obolibrary.org/obo/IAO_0000117> rdf:type owl:AnnotationProperty ;
                                             rdfs:isDefinedBy <http://purl.obolibrary.org/obo/iao.owl> .


###  http://purl.obolibrary.org/obo/IAO_0000119
<http://purl.obolibrary.org/obo/IAO_0000119> rdf:type owl:AnnotationProperty ;
                                             rdfs:isDefinedBy <http://purl.obolibrary.org/obo/iao.owl> .


###  http://swrl.stanford.edu/ontologies/3.3/swrla.owl#isRuleEnabled
<http://swrl.stanford.edu/ontologies/3.3/swrla.owl#isRuleEnabled> rdf:type owl:AnnotationProperty ;
                                                                  rdfs:isDefinedBy <http://swrl.stanford.edu/ontologies/3.3/swrla.owl> .


###  http://www.w3.org/2000/01/rdf-schema#comment
rdfs:comment rdfs:isDefinedBy <http://www.w3.org/2000/01/rdf-schema.owl> .


###  http://www.w3.org/2000/01/rdf-schema#isDefinedBy
rdfs:isDefinedBy rdfs:isDefinedBy <http://www.w3.org/2000/01/rdf-schema.owl> .


###  http://www.w3.org/2000/01/rdf-schema#label
rdfs:label rdfs:isDefinedBy <http://www.w3.org/2000/01/rdf-schema.owl> .


###  http://www.w3.org/2004/02/skos/core#altLabel
<http://www.w3.org/2004/02/skos/core#altLabel> rdf:type owl:AnnotationProperty ;
                                               rdfs:isDefinedBy <http://www.w3.org/2004/02/skos/core.owl> .


###  http://www.w3.org/2004/02/skos/core#definition
<http://www.w3.org/2004/02/skos/core#definition> rdf:type owl:AnnotationProperty ;
                                                 rdfs:isDefinedBy <http://www.w3.org/2004/02/skos/core.owl> .


###  http://www.w3.org/2004/02/skos/core#example
<http://www.w3.org/2004/02/skos/core#example> rdf:type owl:AnnotationProperty ;
                                              rdfs:isDefinedBy <http://www.w3.org/2004/02/skos/core.owl> .


###  https://w3id.org/pmd/co/definitionSource
<https://w3id.org/pmd/co/definitionSource> rdf:type owl:AnnotationProperty ;
                                           rdfs:isDefinedBy <https://w3id.org/pmd/co.owl> .


#################################################################
#    Datatypes
#################################################################

###  http://www.w3.org/1999/02/22-rdf-syntax-ns#PlainLiteral
rdf:PlainLiteral rdfs:isDefinedBy <http://www.w3.org/1999/02/22-rdf-syntax-ns.owl> .


###  http://www.w3.org/2001/XMLSchema#string
xsd:string rdfs:isDefinedBy <http://www.w3.org/2001/xmlschema.owl> .


#################################################################
#    Object Properties
#################################################################

###  http://purl.org/dc/terms/isPartOf
<http://purl.org/dc/terms/isPartOf> rdf:type owl:ObjectProperty ;
                                    rdfs:isDefinedBy <http://purl.org/dc/terms.owl> .


###  http://purl.org/spar/datacite/hasIdentifier
<http://purl.org/spar/datacite/hasIdentifier> rdf:type owl:ObjectProperty ;
                                              rdfs:isDefinedBy <http://purl.org/spar/datacite.owl> .


###  http://www.w3.org/ns/prov#wasDerivedFrom
<http://www.w3.org/ns/prov#wasDerivedFrom> rdf:type owl:ObjectProperty ;
                                           rdfs:isDefinedBy <http://www.w3.org/ns/prov.owl> .


###  https://w3id.org/pmd/co/belongsToProject
<https://w3id.org/pmd/co/belongsToProject> rdf:type owl:ObjectProperty ;
                                           owl:inverseOf <https://w3id.org/pmd/co/process> ;
                                           rdfs:isDefinedBy <https://w3id.org/pmd/co.owl> ;
                                           <http://www.w3.org/2004/02/skos/core#definition> "Association between a process and a project."@en ,
                                                                                            "belongs to process"@en .


###  https://w3id.org/pmd/co/characteristic
<https://w3id.org/pmd/co/characteristic> rdf:type owl:ObjectProperty ;
                                         owl:inverseOf <https://w3id.org/pmd/co/characteristicOf> ;
                                         rdfs:range <https://w3id.org/pmd/co/ValueObject> ;
                                         rdfs:isDefinedBy <https://w3id.org/pmd/co> ;
                                         rdfs:label "characteristic"@en ;
                                         <http://www.w3.org/2004/02/skos/core#altLabel> "has characteristic"@en ;
                                         <http://www.w3.org/2004/02/skos/core#definition> "Die Objekteigenschaft characterisitc, wird in Verbindung mit ProzessKnoten, Prozess und Objekt verwendet und dient zur Herstellung einer Verbindung mit dem WerteObjekt. Diese Eigenschaft ermöglicht die Abbildung von Beziehungen zwischen ProzessKnoten, Prozessen und Objekten und den dazugehörigen Werten oder Attributen (Metadaten), die in WerteObjekt ausgedrückt sind."@de ,
                                                                                          "The object property characteristic, in conjunction with ProcessingNode, Process and Object, is used to establish a connection with ValueObjects. This property enables the representation of relationships between ProcessingNodes, Processes and Objects and the associated values or attributes (metadata) that are stored in ValueObjects."@en .


###  https://w3id.org/pmd/co/characteristicOf
<https://w3id.org/pmd/co/characteristicOf> rdf:type owl:ObjectProperty ;
                                           rdfs:isDefinedBy <https://w3id.org/pmd/co> ;
                                           rdfs:label "characteristic of"@en ;
                                           <http://www.w3.org/2004/02/skos/core#altLabel> "is characteristic of" .


###  https://w3id.org/pmd/co/composedOf
<https://w3id.org/pmd/co/composedOf> rdf:type owl:ObjectProperty ;
                                     owl:inverseOf <https://w3id.org/pmd/co/composes> ;
                                     rdfs:isDefinedBy <https://w3id.org/pmd/co> ;
                                     rdfs:label "composed of"@en ;
                                     <http://www.w3.org/2004/02/skos/core#definition> """This property is used to describe the fact that and which objects are composed of other objects, i.e. it is used to describe the specific constituents or ingredients that form a particular entity or object. 
As a prepositional phrase, it indicates the elements, parts, or components that make up a whole."""@en ,
                                                                                      "This property is used to describe which voxels and materials an object is composed of."@en .


###  https://w3id.org/pmd/co/composes
<https://w3id.org/pmd/co/composes> rdf:type owl:ObjectProperty ;
                                   rdfs:domain <https://w3id.org/pmd/co/Object> ;
                                   rdfs:range <https://w3id.org/pmd/co/Object> ;
                                   rdfs:isDefinedBy <https://w3id.org/pmd/co> ;
                                   rdfs:label "composes"@en ;
                                   <http://www.w3.org/2004/02/skos/core#definition> """Diese Eigenschaft wird verwendet, um die Tatsache zu beschreiben, dass und welche Objekte andere Objekte zusammensetzen, d. h. sie wird verwendet, um die spezifischen Bestandteile oder Zutaten zu beschreiben, aus denen ein bestimmtes Gebilde oder Objekt besteht. 
Als Präpositionalphrase bezeichnet sie die Elemente, Teile oder Komponenten, aus denen sich ein anderes Objekt zusammensetzt."""@de ,
                                                                                    """This property is used to describe the fact that and which objects compose other objects, i.e. it is used to describe the specific constituents or ingredients forming a particular entity or object. 
As a prepositional phrase, it indicates the elements, parts, or components that make up a whole of another object."""@en ,
                                                                                    "This property is used to describe which objects a voxel or a material contributes to compose."@en .


###  https://w3id.org/pmd/co/executedBy
<https://w3id.org/pmd/co/executedBy> rdf:type owl:ObjectProperty ;
                                     owl:inverseOf <https://w3id.org/pmd/co/executes> ;
                                     rdfs:isDefinedBy <https://w3id.org/pmd/co> ;
                                     rdfs:label "executed by"@en ;
                                     <http://www.w3.org/2004/02/skos/core#definition> "This property represents which process is executed by which process node."@en .


###  https://w3id.org/pmd/co/executes
<https://w3id.org/pmd/co/executes> rdf:type owl:ObjectProperty ;
                                   rdfs:isDefinedBy <https://w3id.org/pmd/co> ;
                                   rdfs:label "executes"@en ;
                                   <http://www.w3.org/2004/02/skos/core#definition> "This property represents which ProcessingNode executes a Process."@en .


###  https://w3id.org/pmd/co/input
<https://w3id.org/pmd/co/input> rdf:type owl:ObjectProperty ;
                                rdfs:subPropertyOf <https://w3id.org/pmd/co/participant> ;
                                owl:inverseOf <https://w3id.org/pmd/co/inputOf> ;
                                rdfs:isDefinedBy <https://w3id.org/pmd/co> ;
                                rdfs:label "input"@en ;
                                <http://www.w3.org/2004/02/skos/core#altLabel> "has input" ;
                                <http://www.w3.org/2004/02/skos/core#definition> "This property is used to link the processes to their input objects."@en .


###  https://w3id.org/pmd/co/inputOf
<https://w3id.org/pmd/co/inputOf> rdf:type owl:ObjectProperty ;
                                  rdfs:subPropertyOf <https://w3id.org/pmd/co/participantOf> ;
                                  rdfs:isDefinedBy <https://w3id.org/pmd/co> ;
                                  rdfs:label "input of"@en ;
                                  <http://www.w3.org/2004/02/skos/core#altLabel> "is input of" .


###  https://w3id.org/pmd/co/isResourceOf
<https://w3id.org/pmd/co/isResourceOf> rdf:type owl:ObjectProperty ;
                                       owl:inverseOf <https://w3id.org/pmd/co/resource> ;
                                       rdfs:isDefinedBy <https://w3id.org/pmd/co> ;
                                       rdfs:label "is resource of" .


###  https://w3id.org/pmd/co/nextProcess
<https://w3id.org/pmd/co/nextProcess> rdf:type owl:ObjectProperty ;
                                      owl:inverseOf <https://w3id.org/pmd/co/previousProcess> ;
                                      rdfs:isDefinedBy <https://w3id.org/pmd/co> ;
                                      rdfs:label "next process"@en ;
                                      <http://www.w3.org/2004/02/skos/core#altLabel> "has next process"@en ;
                                      <http://www.w3.org/2004/02/skos/core#definition> "This property is used to indicate the process that was run after the current process."@en .


###  https://w3id.org/pmd/co/output
<https://w3id.org/pmd/co/output> rdf:type owl:ObjectProperty ;
                                 rdfs:subPropertyOf <https://w3id.org/pmd/co/participant> ;
                                 owl:inverseOf <https://w3id.org/pmd/co/outputOf> ;
                                 rdfs:isDefinedBy <https://w3id.org/pmd/co> ;
                                 rdfs:label "output"@en ;
                                 <http://www.w3.org/2004/02/skos/core#altLabel> "has output" ;
                                 <http://www.w3.org/2004/02/skos/core#definition> "This property is used to link the processes to their output objects"@en .


###  https://w3id.org/pmd/co/outputOf
<https://w3id.org/pmd/co/outputOf> rdf:type owl:ObjectProperty ;
                                   rdfs:subPropertyOf <https://w3id.org/pmd/co/participantOf> ;
                                   rdfs:isDefinedBy <https://w3id.org/pmd/co> ;
                                   rdfs:label "output of"@en ;
                                   <http://www.w3.org/2004/02/skos/core#altLabel> "is output of"@en .


###  https://w3id.org/pmd/co/participant
<https://w3id.org/pmd/co/participant> rdf:type owl:ObjectProperty ;
                                      owl:inverseOf <https://w3id.org/pmd/co/participantOf> ;
                                      rdfs:isDefinedBy <https://w3id.org/pmd/co> ;
                                      rdfs:label "participant"@en ;
                                      <http://www.w3.org/2004/02/skos/core#altLabel> "has participant" ;
                                      <http://www.w3.org/2004/02/skos/core#definition> "A relation between a process and an object, in which the objects is somehow involved in the process."@en .


###  https://w3id.org/pmd/co/participantOf
<https://w3id.org/pmd/co/participantOf> rdf:type owl:ObjectProperty ;
                                        rdfs:isDefinedBy <https://w3id.org/pmd/co> ;
                                        rdfs:label "participant of"@en ;
                                        <http://www.w3.org/2004/02/skos/core#altLabel> "is participant of"@en .


###  https://w3id.org/pmd/co/previousProcess
<https://w3id.org/pmd/co/previousProcess> rdf:type owl:ObjectProperty ;
                                          rdfs:isDefinedBy <https://w3id.org/pmd/co> ;
                                          rdfs:label "previous process"@en ;
                                          <http://www.w3.org/2004/02/skos/core#altLabel> "has previous process" ;
                                          <http://www.w3.org/2004/02/skos/core#definition> "This property is used to indicate that which process was previously run."@en .


###  https://w3id.org/pmd/co/process
<https://w3id.org/pmd/co/process> rdf:type owl:ObjectProperty ;
                                  rdfs:isDefinedBy <https://w3id.org/pmd/co> ;
                                  rdfs:label "process"@en ;
                                  <http://www.w3.org/2004/02/skos/core#altLabel> "has process"@en ;
                                  <http://www.w3.org/2004/02/skos/core#definition> "Describes that a process is associated with a project."@en .


###  https://w3id.org/pmd/co/relatesTo
<https://w3id.org/pmd/co/relatesTo> rdf:type owl:ObjectProperty ;
                                    rdfs:domain <https://w3id.org/pmd/co/ValueObject> ;
                                    rdfs:isDefinedBy <https://w3id.org/pmd/co> ;
                                    rdfs:label "relates to"@en ;
                                    <http://www.w3.org/2004/02/skos/core#definition> "Describes a general relationship between domain objects."@en .


###  https://w3id.org/pmd/co/relatesToElement
<https://w3id.org/pmd/co/relatesToElement> rdf:type owl:ObjectProperty ;
                                           rdfs:subPropertyOf <https://w3id.org/pmd/co/relatesTo> ;
                                           rdfs:isDefinedBy <https://w3id.org/pmd/co> ;
                                           rdfs:label "relates to element"@en .


###  https://w3id.org/pmd/co/resource
<https://w3id.org/pmd/co/resource> rdf:type owl:ObjectProperty ,
                                            owl:FunctionalProperty ;
                                   rdfs:domain <https://w3id.org/pmd/co/ValueObject> ;
                                   rdfs:isDefinedBy <https://w3id.org/pmd/co> ;
                                   rdfs:label "resource"@en ;
                                   <http://www.w3.org/2004/02/skos/core#altLabel> "has resource"@en .


###  https://w3id.org/pmd/co/state
<https://w3id.org/pmd/co/state> rdf:type owl:ObjectProperty ;
                                rdfs:isDefinedBy <https://w3id.org/pmd/co> ;
                                rdfs:label "state"@en .


###  https://w3id.org/pmd/co/subordinateProcess
<https://w3id.org/pmd/co/subordinateProcess> rdf:type owl:ObjectProperty ;
                                             owl:inverseOf <https://w3id.org/pmd/co/superordinateProcess> ;
                                             rdfs:isDefinedBy <https://w3id.org/pmd/co> ;
                                             rdfs:label "subordinate process"@en ;
                                             <http://www.w3.org/2004/02/skos/core#altLabel> "has subordinate process" ;
                                             <http://www.w3.org/2004/02/skos/core#definition> "This property is used to link a process to its subordinate processes."@en .


###  https://w3id.org/pmd/co/superordinateProcess
<https://w3id.org/pmd/co/superordinateProcess> rdf:type owl:ObjectProperty ;
                                               rdfs:isDefinedBy <https://w3id.org/pmd/co> ;
                                               rdfs:label "superordinate process"@en ;
                                               <http://www.w3.org/2004/02/skos/core#altLabel> "has superordinate process"@en ;
                                               <http://www.w3.org/2004/02/skos/core#definition> "This property is used to link a process to its super ordinated processes."@en .


###  https://w3id.org/pmd/co/unit
<https://w3id.org/pmd/co/unit> rdf:type owl:ObjectProperty ;
                               rdfs:domain <https://w3id.org/pmd/co/ValueObject> ;
                               rdfs:comment "Examples for rdsf:range are units from qudt or wikidata or own defindes units." ;
                               rdfs:isDefinedBy <https://w3id.org/pmd/co> ;
                               rdfs:label "unit"@en ;
                               <http://www.w3.org/2004/02/skos/core#altLabel> "has unit"@en ;
                               <http://www.w3.org/2004/02/skos/core#definition> "Unit of measurement."@en .


#################################################################
#    Data properties
#################################################################

###  https://w3id.org/pmd/co/fromValue
<https://w3id.org/pmd/co/fromValue> rdf:type owl:DatatypeProperty ;
                                    rdfs:subPropertyOf <https://w3id.org/pmd/co/value> ;
                                    rdfs:isDefinedBy <https://w3id.org/pmd/co> ;
                                    rdfs:label "from value"@en ;
                                    <http://www.w3.org/2004/02/skos/core#definition> "refers to the begin of a value range" .


###  https://w3id.org/pmd/co/maxValue
<https://w3id.org/pmd/co/maxValue> rdf:type owl:DatatypeProperty ;
                                   rdfs:subPropertyOf <https://w3id.org/pmd/co/value> ;
                                   rdfs:isDefinedBy <https://w3id.org/pmd/co> ;
                                   rdfs:label "max value"@en ;
                                   <http://www.w3.org/2004/02/skos/core#definition> "refers to all values equal or smaller than the given one"@en .


###  https://w3id.org/pmd/co/minValue
<https://w3id.org/pmd/co/minValue> rdf:type owl:DatatypeProperty ;
                                   rdfs:subPropertyOf <https://w3id.org/pmd/co/value> ;
                                   rdfs:isDefinedBy <https://w3id.org/pmd/co> ;
                                   rdfs:label "min value"@en ;
                                   <http://www.w3.org/2004/02/skos/core#definition> "refers to all values equal or larger than the given one"@en .


###  https://w3id.org/pmd/co/toValue
<https://w3id.org/pmd/co/toValue> rdf:type owl:DatatypeProperty ;
                                  rdfs:subPropertyOf <https://w3id.org/pmd/co/value> ;
                                  rdfs:isDefinedBy <https://w3id.org/pmd/co> ;
                                  rdfs:label "to value"@en ;
                                  <http://www.w3.org/2004/02/skos/core#definition> "refers to the end of a value range" .


###  https://w3id.org/pmd/co/value
<https://w3id.org/pmd/co/value> rdf:type owl:DatatypeProperty ;
                                rdfs:domain <https://w3id.org/pmd/co/ValueObject> ;
                                rdfs:isDefinedBy <https://w3id.org/pmd/co> ;
                                rdfs:label "hat Wert"@de ,
                                           "value"@en ;
                                <http://www.w3.org/2004/02/skos/core#definition> "Provides the actual value a value object is referring to."@en .


#################################################################
#    Classes
#################################################################

###  https://w3id.org/pmd/co/MaterialProperty
<https://w3id.org/pmd/co/MaterialProperty> rdf:type owl:Class ;
                                           rdfs:subClassOf <https://w3id.org/pmd/co/MaterialRelated> ;
                                           rdfs:isDefinedBy <https://w3id.org/pmd/co> ;
                                           rdfs:label "Material Property"@en ,
                                                      "Materialeigenschaft"@de ;
                                           <http://www.w3.org/2004/02/skos/core#definition> "A materials property is an intensive property of a material, i.e., a physical property that does not depend on the amount of the material. These quantitative properties may be used as a metric by which the benefits of one material versus another can be compared, thereby aiding in materials selection."@en ,
                                                                                            "Eine Materialeigenschaft ist eine intensive Eigenschaft eines Materials, d. h. eine physikalische Eigenschaft, die nicht von der Menge des Materials abhängt. Diese quantitativen Eigenschaften können als Maßstab verwendet werden, um die Vorteile eines Materials mit denen eines anderen zu vergleichen und so die Materialauswahl zu erleichtern."@de ;
                                           <https://w3id.org/pmd/co/definitionSource> "“List of materials properties.” Wikipedia The Free Encyclopedia, https://en.wikipedia.org/wiki/List_of_materials_properties. Accessed 13 Jan. 2023."@en .


###  https://w3id.org/pmd/co/MaterialRelated
<https://w3id.org/pmd/co/MaterialRelated> rdf:type owl:Class ;
                                          rdfs:subClassOf <https://w3id.org/pmd/co/ValueObject> ;
                                          rdfs:isDefinedBy <https://w3id.org/pmd/co> ;
                                          rdfs:label "Material Related"@en ,
                                                     "Materialbezug"@de ;
                                          <http://www.w3.org/2004/02/skos/core#definition> "Diese Klasse dient der qualitativen und quantitativen Beschreibung eines Materials, indem sie Informationen über ein Material angibt, z. B. durch die Einbeziehung von Materialeigenschaften, Materialstruktur usw."@de ,
                                                                                           "This property is used to qualitatively and quantitatively describe a material by providing information on a material, e.g., by including material properties, material structure, etc."@en .


###  https://w3id.org/pmd/co/Measurement
<https://w3id.org/pmd/co/Measurement> rdf:type owl:Class ;
                                      rdfs:isDefinedBy <https://w3id.org/pmd/co> ;
                                      rdfs:label "Measurement"@en ,
                                                 "Messwert"@de ;
                                      <http://www.w3.org/2004/02/skos/core#definition> """Die Wertekategorie Messung ermöglicht die Kategorisierung von ValueObjects als gemessen.
Messung ist die Quantifizierung von Eigenschaften eines Objekts oder Ereignisses, die zum Vergleich mit anderen Objekten oder Ereignissen verwendet werden können."""@de ,
                                                                                       """The ValueScope category Measurement enables the categorization of ValueObjects as measured.
Measurement is the quantification of attributes of an object or event, which can be used to compare with other objects or events."""@en ,
                                                                                       "This value scope describes that a :ValueObject is the quantification of attributes of an object or event, which can be used to compare with other objects or events."@en ;
                                      <https://w3id.org/pmd/co/definitionSource> "https://en.wikipedia.org/wiki/Measurement"@en .


###  https://w3id.org/pmd/co/Metadata
<https://w3id.org/pmd/co/Metadata> rdf:type owl:Class ;
                                   rdfs:subClassOf <https://w3id.org/pmd/co/ValueObject> ;
                                   owl:disjointWith <https://w3id.org/pmd/co/PrimaryData> ,
                                                    <https://w3id.org/pmd/co/SecondaryData> ;
                                   rdfs:isDefinedBy <https://w3id.org/pmd/co> ;
                                   rdfs:label "Metadata"@en ,
                                              "Metadaten"@de ;
                                   <http://www.w3.org/2004/02/skos/core#definition> "Die DataScope Metadaten umfassen Attribute und zusätzliche Daten (Provenienz), die z.B. die Fabrik, das Labor, das Prozesssystem und die Objekte betreffen und die eine Bewertung der Qualität / Zuverlässigkeit der Messungen und eine systematische Suche in einer Datenbank ermöglichen."@de ,
                                                                                    "This data scope expresses that a :ValueObject refers to attributes and additional data (provenance) on production, laboratory, process system and objects that enable an evaluation of the quality/reliability of the measurements and a systematic search task in a database."@en .


###  https://w3id.org/pmd/co/Object
<https://w3id.org/pmd/co/Object> rdf:type owl:Class ;
                                 rdfs:isDefinedBy <https://w3id.org/pmd/co> ;
                                 rdfs:label "Object"@en ,
                                            "Objekt"@de ;
                                 <http://www.w3.org/2004/02/skos/core#definition> "A discernable, tangible or simulated entity that is processed in a process by a processing node."@en .


###  https://w3id.org/pmd/co/PrimaryData
<https://w3id.org/pmd/co/PrimaryData> rdf:type owl:Class ;
                                      owl:disjointWith <https://w3id.org/pmd/co/SecondaryData> ;
                                      rdfs:isDefinedBy <https://w3id.org/pmd/co> ;
                                      rdfs:label "Primary Data"@en ,
                                                 "Primärdaten"@de ;
                                      <http://www.w3.org/2004/02/skos/core#definition> "Die Datenkategorie Primärdaten umfasst Daten, die vor / nach einem Prozess erfasst werden, entweder bezogen auf die Geometrie des Objekts (z.B. ao, bo, do, au, bu, du, Lu) oder als Register des gesamten Aufbaus (z.B. Skizzen, Fotos oder Videos)"@de ,
                                                                                       "This data scope expresses that a ValueObject refers to data that is directly acquired during a process by sensors (time, force, length, temperature)"@en .


###  https://w3id.org/pmd/co/SecondaryData
<https://w3id.org/pmd/co/SecondaryData> rdf:type owl:Class ;
                                        rdfs:isDefinedBy <https://w3id.org/pmd/co> ;
                                        rdfs:label "Secondary Data"@en ,
                                                   "Sekundärdaten"@de ;
                                        <http://www.w3.org/2004/02/skos/core#definition> "Der Datenkategorie Sekundärdaten umfasst Werte (z. B. Testergebnisse), die durch Gleichungen oder Algorithmen unter Verwendung von Primärdaten und Metadaten ermittelt werden."@de ,
                                                                                         "This data scope expresses that a ValueObject refers to characteristic values (e.g. test results) determined by equations or algorithms using primary data and/or metadata."@en .


###  https://w3id.org/pmd/co/SetPoint
<https://w3id.org/pmd/co/SetPoint> rdf:type owl:Class ;
                                   rdfs:isDefinedBy <https://w3id.org/pmd/co> ;
                                   rdfs:label "Set Point"@en ,
                                              "Sollwert"@de ;
                                   <http://www.w3.org/2004/02/skos/core#definition> "Die Wertekategorie Sollwert bezeichnet allgemein den gewünschten Wert eines quantitativen Merkmals eines Systems, von dem der Istwert möglichst wenig abweichen soll."@de ,
                                                                                    "Sollwert bezeichnet allgemein den angestrebten Wert eines quantitativen Merkmales eines Systems, von dem der tatsächliche Istwert so wenig wie möglich abweichen soll. Der Sollwert wird von einem anderen System (z. B. Technik, Mensch) vorgegeben."@de ,
                                                                                    "The ValueScope Setpoint generally refers to the desired value of a quantitative characteristic of a system, from which the actual value should deviate as little as possible."@en ,
                                                                                    "This value scope expresses that a :ValueObject is the desired or target value for an essential variable, or process value (PV) of a control system."@en ;
                                   <https://w3id.org/pmd/co/definitionSource> "https://de.wikipedia.org/wiki/Sollwert"@de ,
                                                                              "https://en.wikipedia.org/wiki/Setpoint_(control_system)"@en .


###  https://w3id.org/pmd/co/ValueObject
<https://w3id.org/pmd/co/ValueObject> rdf:type owl:Class ;
                                      owl:equivalentClass [ rdf:type owl:Class ;
                                                            owl:unionOf ( <https://w3id.org/pmd/co/Metadata>
                                                                          [ owl:intersectionOf ( [ rdf:type owl:Class ;
                                                                                                   owl:unionOf ( <https://w3id.org/pmd/co/Measurement>
                                                                                                                 <https://w3id.org/pmd/co/SetPoint>
                                                                                                               )
                                                                                                 ]
                                                                                                 [ rdf:type owl:Class ;
                                                                                                   owl:unionOf ( <https://w3id.org/pmd/co/PrimaryData>
                                                                                                                 <https://w3id.org/pmd/co/SecondaryData>
                                                                                                               )
                                                                                                 ]
                                                                                               ) ;
                                                                            rdf:type owl:Class
                                                                          ]
                                                                        )
                                                          ] ;
                                      rdfs:isDefinedBy <https://w3id.org/pmd/co> ;
                                      rdfs:label "Value Object"@en ,
                                                 "Wertobjekt"@de ;
                                      <http://www.w3.org/2004/02/skos/core#definition> """A :ValueObject is an entity which represents a specific value. This value can be a numerical, textual, or a more complex data structure. If a literal value is to be specified, the :value datatype property has to be used. In cases where the value is represented by a resource (e.g. URI), the :resource object property has to be used.

A value object, respectively its value, is always associated with an entity of type :Process, :ProcessingNode, :Object (e.g. :Specimen), :DigitalEntity, :Project, or other :ValueObject. The value is meant to be a charactaristic of the associated entity. To express this association it is indended to use the :characteristic object property if the value decribes some \\\"quality\\\", or the :participant (:input,:output) if it is participating a process.

A value object might also refer to a unit. The :unit property might be used (e.g. with QUDT ontology).

Instances of a value object might also be a type of :ValueScope, namely a :SetPoint (nominal value), or :Measurement (measured value). With :Setpoint the intend is to express, that the value is meant to be some preset, setting or nominal value. :Measurement expresses, that the value has been measured or determined somehow (see example).

Instances of a value object might also be specified in a specific :DataScope (:Metadata, :PrimaryData, :SecondaryData)."""@en ;
                                      <http://www.w3.org/2004/02/skos/core#example> """- the length of a specimen
- the model number of a machine
- a person involved in a process
- a force on an object"""@en ,
                                                                                    """:Length rdfs:subClass :ValueObject .
ex:vo1 a :Length .
ex:vo1 a :Measurement .
ex:vo1 a :PrimaryData .
ex:vo1 :unit qudt:MilliM . 
ex:vo1 :value \"123.45\"
ex:p1 a :LengthMeasuringProcess .
ex:p1 :characteristic ex:vo1 ."""@en ,
                                                                                    "The length of a specimen, which has been measured as primary data. Its actual value is 123.45 millimeters."@en .


#################################################################
#    Annotations
#################################################################

<http://purl.obolibrary.org/obo/IAO_0000002> <http://purl.obolibrary.org/obo/IAO_0000111> "example to be eventually removed"@en ;
                                             rdfs:isDefinedBy <http://purl.obolibrary.org/obo/iao.owl> ;
                                             rdfs:label "example to be eventually removed"@en .


<http://purl.obolibrary.org/obo/IAO_0000114> rdfs:isDefinedBy <http://purl.obolibrary.org/obo/iao.owl> .


<http://purl.obolibrary.org/obo/IAO_0000120> <http://purl.obolibrary.org/obo/IAO_0000111> "metadata complete"@en ;
                                             <http://purl.obolibrary.org/obo/IAO_0000115> "Class has all its metadata, but is either not guaranteed to be in its final location in the asserted IS_A hierarchy or refers to another class that is not complete."@en ;
                                             rdfs:isDefinedBy <http://purl.obolibrary.org/obo/iao.owl> ;
                                             rdfs:label "metadata complete"@en .


<http://purl.obolibrary.org/obo/IAO_0000121> <http://purl.obolibrary.org/obo/IAO_0000111> "organizational term"@en ;
                                             <http://purl.obolibrary.org/obo/IAO_0000115> "Term created to ease viewing/sort terms for development purpose, and will not be included in a release"@en ;
                                             rdfs:isDefinedBy <http://purl.obolibrary.org/obo/iao.owl> ;
                                             rdfs:label "organizational term"@en .


<http://purl.obolibrary.org/obo/IAO_0000122> <http://purl.obolibrary.org/obo/IAO_0000111> "ready for release"@en ;
                                             <http://purl.obolibrary.org/obo/IAO_0000115> "Class has undergone final review, is ready for use, and will be included in the next release. Any class lacking \"ready_for_release\" should be considered likely to change place in hierarchy, have its definition refined, or be obsoleted in the next release.  Those classes deemed \"ready_for_release\" will also derived from a chain of ancestor classes that are also \"ready_for_release.\""@en ;
                                             rdfs:isDefinedBy <http://purl.obolibrary.org/obo/iao.owl> ;
                                             rdfs:label "ready for release"@en .


<http://purl.obolibrary.org/obo/IAO_0000123> <http://purl.obolibrary.org/obo/IAO_0000111> "metadata incomplete"@en ;
                                             <http://purl.obolibrary.org/obo/IAO_0000115> "Class is being worked on; however, the metadata (including definition) are not complete or sufficiently clear to the branch editors."@en ;
                                             rdfs:isDefinedBy <http://purl.obolibrary.org/obo/iao.owl> ;
                                             rdfs:label "metadata incomplete"@en .


<http://purl.obolibrary.org/obo/IAO_0000124> <http://purl.obolibrary.org/obo/IAO_0000111> "uncurated"@en ;
                                             <http://purl.obolibrary.org/obo/IAO_0000115> "Nothing done yet beyond assigning a unique class ID and proposing a preferred term."@en ;
                                             rdfs:isDefinedBy <http://purl.obolibrary.org/obo/iao.owl> ;
                                             rdfs:label "uncurated"@en .


<http://purl.obolibrary.org/obo/IAO_0000125> <http://purl.obolibrary.org/obo/IAO_0000111> "pending final vetting"@en ;
                                             <http://purl.obolibrary.org/obo/IAO_0000115> "All definitions, placement in the asserted IS_A hierarchy and required minimal metadata are complete. The class is awaiting a final review by someone other than the term editor."@en ;
                                             rdfs:isDefinedBy <http://purl.obolibrary.org/obo/iao.owl> ;
                                             rdfs:label "pending final vetting"@en .


<http://purl.obolibrary.org/obo/IAO_0000423> <http://purl.obolibrary.org/obo/IAO_0000111> "to be replaced with external ontology term"@en ;
                                             <http://purl.obolibrary.org/obo/IAO_0000115> "Terms with this status should eventually replaced with a term from another ontology."@en ;
                                             <http://purl.obolibrary.org/obo/IAO_0000117> "Alan Ruttenberg"@en ;
                                             <http://purl.obolibrary.org/obo/IAO_0000119> "group:OBI"@en ;
                                             rdfs:isDefinedBy <http://purl.obolibrary.org/obo/iao.owl> ;
                                             rdfs:label "to be replaced with external ontology term"@en .


<http://purl.obolibrary.org/obo/IAO_0000428> <http://purl.obolibrary.org/obo/IAO_0000115> "A term that is metadata complete, has been reviewed, and problems have been identified that require discussion before release. Such a term requires editor note(s) to identify the outstanding issues."@en ;
                                             rdfs:isDefinedBy <http://purl.obolibrary.org/obo/iao.owl> ;
                                             rdfs:label "requires discussion"@en .


rdfs:Literal rdfs:isDefinedBy <http://www.w3.org/2000/01/rdf-schema.owl> .


xsd:boolean rdfs:isDefinedBy <http://www.w3.org/2001/xmlschema.owl> .


<http://www.w3.org/ns/prov#constraints> rdfs:isDefinedBy <http://www.w3.org/ns/prov.owl> .


<http://www.w3.org/ns/prov#editorialNote> rdfs:isDefinedBy <http://www.w3.org/ns/prov.owl> .


<https://w3id.org/pmd/co/symbol> rdfs:isDefinedBy <https://w3id.org/pmd/co.owl> .


###  Generated by the OWL API (version 4.5.29) https://github.com/owlcs/owlapi
