<?xml version="1.0"?>
<rdf:RDF xmlns="http://OntoCAPE/chemical_process_system/CPS_function/process.owl#"
     xml:base="http://OntoCAPE/chemical_process_system/CPS_function/process.owl"
     xmlns:fc="http://meta_model/fundamental_concepts/fundamental_concepts.owl#"
     xmlns:owl="http://www.w3.org/2002/07/owl#"
     xmlns:rdf="http://www.w3.org/1999/02/22-rdf-syntax-ns#"
     xmlns:xml="http://www.w3.org/XML/1998/namespace"
     xmlns:xsd="http://www.w3.org/2001/XMLSchema#"
     xmlns:rdfs="http://www.w3.org/2000/01/rdf-schema#"
     xmlns:terms="http://purl.org/dc/terms/"
     xmlns:system="http://OntoCAPE/upper_level/system.owl#"
     xmlns:der_dim="http://OntoCAPE/supporting_concepts/physical_dimension/derived_dimensions.owl#"
     xmlns:process="http://OntoCAPE/chemical_process_system/CPS_function/process.owl#"
     xmlns:material="http://OntoCAPE/material/material.owl#"
     xmlns:phys_dim="http://OntoCAPE/supporting_concepts/physical_dimension/physical_dimension.owl#"
     xmlns:phase_system="http://OntoCAPE/material/phase_system/phase_system.owl#"
     xmlns:network_system="http://OntoCAPE/upper_level/network_system.owl#">
    <owl:Ontology rdf:about="http://OntoCAPE/chemical_process_system/CPS_function/process.owl">
        <terms:license>Copyright (C) [2009] [Andreas Wiesner]
                This program is free software; you can redistribute it and/or modify it under the terms of the GNU General Public License as published by the Free Software Foundation; either version 3 of the License, or (at your option) any later version.
                This program is distributed in the hope that it will be useful, but WITHOUT ANY WARRANTY; without even the implied warranty of MERCHANTABILITY or FITNESS FOR A PARTICULAR PURPOSE. See the GNU General Public License for more details.
                You should have received a copy of the GNU General Public License along with this program; if not, see &lt;http://www.gnu.org/licenses/&gt;.
    </terms:license>
        <rdfs:comment>The ontology module &apos;process&apos; provides concepts a functional description of an chemical process system at an early stage of design.
The following classes and relations from other ontology modules are used within &apos;process&apos;:
    
 &lt;owl:Class rdf:about=&quot;http://OntoCAPE/material/material.owl#Material&quot;&gt;    
 &lt;owl:Class rdf:about=&quot;http://OntoCAPE/material/phase_system/phase_system.owl#ReactionNetwork&quot;&gt; 
 &lt;owl:Class rdf:about=&quot;http://OntoCAPE/material/phase_system/phase_system.owl#MultiphaseSystem&quot;&gt; 
 &lt;owl:Class rdf:about=&quot;http://OntoCAPE/material/phase_system/phase_system.owl#SinglePhase&quot;&gt; 
 &lt;owl:Class rdf:about=&quot;http://OntoCAPE/material/phase_system/phase_system.owl#SinglePhaseInMultiphaseSystem&quot;&gt; 
 &lt;owl:Class rdf:about=&quot;http://OntoCAPE/upper_level/system.owl#ScalarQuantity&quot;&gt;
 &lt;owl:Class rdf:about=&quot;http://OntoCAPE/upper_level/network_system.owl#DirectedConnection&quot;&gt;
 &lt;owl:Class rdf:about=&quot;http://OntoCAPE/material/phase_system/phase_system.owl#ReactionNetwork&quot;&gt;
 &lt;owl:Class rdf:about=&quot;http://OntoCAPE/upper_level/network_system.owl#Device&quot;&gt;
 &lt;owl:Class rdf:about=&quot;http://OntoCAPE/upper_level/system.owl#Property&quot;&gt;
    
 &lt;owl:ObjectProperty rdf:about=&quot;http://OntoCAPE/material/phase_system/phase_system.owl#hasStateOfAggregation&quot;&gt;   
 &lt;owl:ObjectProperty rdf:about=&quot;http://OntoCAPE/upper_level/system.owl#isComposedOfSubsystem&quot;&gt;    
 &lt;owl:ObjectProperty rdf:about=&quot;http://OntoCAPE/upper_level/system.owl#hasProperty&quot;&gt;    
 &lt;owl:ObjectProperty rdf:about=&quot;http://OntoCAPE/material/material.owl#thermodynamicBehavior&quot;&gt;
 &lt;owl:ObjectProperty rdf:about=&quot;http://OntoCAPE/upper_level/network_system.owl#enters&quot;&gt;
 &lt;owl:ObjectProperty rdf:about=&quot;http://OntoCAPE/upper_level/network_system.owl#leaves&quot;&gt;
 &lt;owl:ObjectProperty rdf:about=&quot;http://OntoCAPE/upper_level/system.owl#hasDimension&quot;&gt;
 &lt;owl:ObjectProperty rdf:about=&quot;http://OntoCAPE/upper_level/system.owl#isSubsystemOf&quot;&gt;
 &lt;owl:ObjectProperty rdf:about=&quot;http://OntoCAPE/upper_level/system.owl#hasDirectSubsystem&quot;&gt;
 &lt;owl:ObjectProperty rdf:about=&quot;http://OntoCAPE/upper_level/system.owl#isDirectSubsystemOf&quot;&gt;
 &lt;owl:ObjectProperty rdf:about=&quot;http://OntoCAPE/upper_level/system.owl#isDirectlyRelatedTo&quot;&gt;
 &lt;owl:ObjectProperty rdf:about=&quot;http://OntoCAPE/upper_level/network_system.owl#hasOutput&quot;&gt;
 &lt;owl:ObjectProperty rdf:about=&quot;http://OntoCAPE/upper_level/network_system.owl#hasInput&quot;&gt;
 
 &lt;phase_system:StateOfAggregation rdf:about=&quot;http://OntoCAPE/material/phase_system/phase_system.owl#liquid&quot;&gt;
 &lt;phase_system:StateOfAggregation rdf:about=&quot;http://OntoCAPE/material/phase_system/phase_system.owl#gaseous&quot;&gt;
 &lt;phase_system:StateOfAggregation rdf:about=&quot;http://OntoCAPE/material/phase_system/phase_system.owl#solid&quot;&gt;
 &lt;der_dim:Mechanics rdf:about=&quot;der_dim;#pressure&quot;&gt;
 &lt;phys_dim:SupplementaryDimension rdf:about=&quot;phys_dim;#identity_dimension&quot;&gt;
 
 The following classes and relations from the Meta Model are refined within &apos;process&apos;:
 
 &lt;owl:Class rdf:about=&quot;http://OntoCAPE/meta_model/fundamental_concepts/fundamental_concepts.owl#ValueSet&quot;&gt;
 
 &lt;owl:ObjectProperty rdf:about=&quot;http://OntoCAPE/meta_model/fundamental_concepts/fundamental_concepts.owl#isOfType&quot;&gt;
    
    </rdfs:comment>
        <owl:versionInfo>2.0</owl:versionInfo>
    </owl:Ontology>
    


    <!-- 
    ///////////////////////////////////////////////////////////////////////////////////////
    //
    // Annotation properties
    //
    ///////////////////////////////////////////////////////////////////////////////////////
     -->

    


    <!-- http://purl.org/dc/terms/license -->

    <owl:AnnotationProperty rdf:about="http://purl.org/dc/terms/license"/>
    


    <!-- 
    ///////////////////////////////////////////////////////////////////////////////////////
    //
    // Object Properties
    //
    ///////////////////////////////////////////////////////////////////////////////////////
     -->

    


    <!-- http://OntoCAPE/chemical_process_system/CPS_function/process.owl#hasChemicalReactionNetwork -->

    <owl:ObjectProperty rdf:about="http://OntoCAPE/chemical_process_system/CPS_function/process.owl#hasChemicalReactionNetwork">
        <rdfs:subPropertyOf rdf:resource="http://OntoCAPE/upper_level/system.owl#isDirectlyRelatedTo"/>
        <rdfs:domain rdf:resource="http://OntoCAPE/chemical_process_system/CPS_function/process.owl#Reaction"/>
        <rdfs:range rdf:resource="http://OntoCAPE/material/phase_system/phase_system.owl#ReactionNetwork"/>
        <rdfs:comment>The relation hasChemicalRectionNetwork indicates that a reaction as considered on a rather macroscopic perspective of an early design stage may be the result of an sequence of reactions occurring on the bases of several phases.</rdfs:comment>
    </owl:ObjectProperty>
    


    <!-- http://OntoCAPE/chemical_process_system/CPS_function/process.owl#hasOperationMode -->

    <owl:ObjectProperty rdf:about="http://OntoCAPE/chemical_process_system/CPS_function/process.owl#hasOperationMode">
        <rdfs:subPropertyOf rdf:resource="http://OntoCAPE/meta_model/fundamental_concepts/fundamental_concepts.owl#isOfType"/>
        <rdfs:domain>
            <owl:Class>
                <owl:unionOf rdf:parseType="Collection">
                    <rdf:Description rdf:about="http://OntoCAPE/chemical_process_system/CPS_function/process.owl#BatchProcess"/>
                    <rdf:Description rdf:about="http://OntoCAPE/chemical_process_system/CPS_function/process.owl#ProcessStream"/>
                </owl:unionOf>
            </owl:Class>
        </rdfs:domain>
        <rdfs:range rdf:resource="http://OntoCAPE/chemical_process_system/CPS_function/process.owl#ModeOfOperation"/>
        <rdfs:comment>The relation hasOperationMode indicates by which operation modes a particular process state is achieved.</rdfs:comment>
    </owl:ObjectProperty>
    


    <!-- http://OntoCAPE/chemical_process_system/CPS_function/process.owl#hasPressureDifference -->

    <owl:ObjectProperty rdf:about="http://OntoCAPE/chemical_process_system/CPS_function/process.owl#hasPressureDifference">
        <rdfs:subPropertyOf rdf:resource="http://OntoCAPE/upper_level/system.owl#hasProperty"/>
        <rdfs:domain rdf:resource="http://OntoCAPE/chemical_process_system/CPS_function/process.owl#PressureChange"/>
        <rdfs:range rdf:resource="http://OntoCAPE/chemical_process_system/CPS_function/process.owl#PressureDifference"/>
        <rdfs:comment>The relation hasPressureDifference indicates the intended difference between two pressure state.</rdfs:comment>
    </owl:ObjectProperty>
    


    <!-- http://OntoCAPE/chemical_process_system/CPS_function/process.owl#hasVapourRatio -->

    <owl:ObjectProperty rdf:about="http://OntoCAPE/chemical_process_system/CPS_function/process.owl#hasVapourRatio">
        <rdfs:subPropertyOf rdf:resource="http://OntoCAPE/upper_level/system.owl#hasProperty"/>
        <rdfs:domain rdf:resource="http://OntoCAPE/chemical_process_system/CPS_function/process.owl#Flashing"/>
        <rdfs:range rdf:resource="http://OntoCAPE/chemical_process_system/CPS_function/process.owl#FlashVaporRatio"/>
        <rdfs:comment>The relation hasVaporRatio indicates the liquid-vapor ratio of a particular mixture at a certain state within a vessel.</rdfs:comment>
    </owl:ObjectProperty>
    


    <!-- http://OntoCAPE/meta_model/fundamental_concepts/fundamental_concepts.owl#isOfType -->

    <owl:ObjectProperty rdf:about="http://OntoCAPE/meta_model/fundamental_concepts/fundamental_concepts.owl#isOfType"/>
    


    <!-- http://OntoCAPE/upper_level/network_system.owl#enters -->

    <owl:ObjectProperty rdf:about="http://OntoCAPE/upper_level/network_system.owl#enters">
        <rdfs:subPropertyOf rdf:resource="http://OntoCAPE/upper_level/network_system.owl#isPredecessorOf"/>
        <owl:inverseOf rdf:resource="http://OntoCAPE/upper_level/network_system.owl#hasInput"/>
        <rdfs:domain rdf:resource="http://OntoCAPE/upper_level/network_system.owl#DirectedConnection"/>
        <rdfs:range rdf:resource="http://OntoCAPE/upper_level/network_system.owl#Device"/>
        <rdfs:comment>The relation Enters interconnects an ingoing DirectedConnection  to its target Device.</rdfs:comment>
    </owl:ObjectProperty>
    


    <!-- http://OntoCAPE/upper_level/network_system.owl#hasInput -->

    <owl:ObjectProperty rdf:about="http://OntoCAPE/upper_level/network_system.owl#hasInput">
        <rdfs:subPropertyOf rdf:resource="http://OntoCAPE/upper_level/network_system.owl#isSuccessorOf"/>
        <rdfs:domain rdf:resource="http://OntoCAPE/upper_level/network_system.owl#Device"/>
        <rdfs:range rdf:resource="http://OntoCAPE/upper_level/network_system.owl#DirectedConnection"/>
        <rdfs:comment>The relation hasInput connects a Device to an incoming DirectedConnection.</rdfs:comment>
    </owl:ObjectProperty>
    


    <!-- http://OntoCAPE/upper_level/network_system.owl#hasOutput -->

    <owl:ObjectProperty rdf:about="http://OntoCAPE/upper_level/network_system.owl#hasOutput">
        <rdfs:subPropertyOf rdf:resource="http://OntoCAPE/upper_level/network_system.owl#isPredecessorOf"/>
        <owl:inverseOf rdf:resource="http://OntoCAPE/upper_level/network_system.owl#leaves"/>
        <rdfs:domain rdf:resource="http://OntoCAPE/upper_level/network_system.owl#Device"/>
        <rdfs:range rdf:resource="http://OntoCAPE/upper_level/network_system.owl#DirectedConnection"/>
        <rdfs:comment>The relation hasOutput connects a Device to an outgoing DirectedConnection.</rdfs:comment>
    </owl:ObjectProperty>
    


    <!-- http://OntoCAPE/upper_level/network_system.owl#isPredecessorOf -->

    <owl:ObjectProperty rdf:about="http://OntoCAPE/upper_level/network_system.owl#isPredecessorOf">
        <rdfs:subPropertyOf rdf:resource="http://OntoCAPE/upper_level/system.owl#isConnectedTo"/>
        <owl:inverseOf rdf:resource="http://OntoCAPE/upper_level/network_system.owl#isSuccessorOf"/>
        <rdf:type rdf:resource="http://www.w3.org/2002/07/owl#TransitiveProperty"/>
        <rdfs:domain>
            <owl:Class>
                <owl:unionOf rdf:parseType="Collection">
                    <rdf:Description rdf:about="http://OntoCAPE/upper_level/network_system.owl#Device"/>
                    <rdf:Description rdf:about="http://OntoCAPE/upper_level/network_system.owl#DirectedConnection"/>
                </owl:unionOf>
            </owl:Class>
        </rdfs:domain>
        <rdfs:range>
            <owl:Class>
                <owl:unionOf rdf:parseType="Collection">
                    <rdf:Description rdf:about="http://OntoCAPE/upper_level/network_system.owl#Device"/>
                    <rdf:Description rdf:about="http://OntoCAPE/upper_level/network_system.owl#DirectedConnection"/>
                </owl:unionOf>
            </owl:Class>
        </rdfs:range>
        <rdfs:comment>The relation isPredecessorOf identifies all Devices and DirectedConnections that are predecessors of the considered one.</rdfs:comment>
    </owl:ObjectProperty>
    


    <!-- http://OntoCAPE/upper_level/network_system.owl#isSuccessorOf -->

    <owl:ObjectProperty rdf:about="http://OntoCAPE/upper_level/network_system.owl#isSuccessorOf">
        <rdfs:subPropertyOf rdf:resource="http://OntoCAPE/upper_level/system.owl#isConnectedTo"/>
        <rdf:type rdf:resource="http://www.w3.org/2002/07/owl#TransitiveProperty"/>
        <rdfs:domain>
            <owl:Class>
                <owl:unionOf rdf:parseType="Collection">
                    <rdf:Description rdf:about="http://OntoCAPE/upper_level/network_system.owl#Device"/>
                    <rdf:Description rdf:about="http://OntoCAPE/upper_level/network_system.owl#DirectedConnection"/>
                </owl:unionOf>
            </owl:Class>
        </rdfs:domain>
        <rdfs:range>
            <owl:Class>
                <owl:unionOf rdf:parseType="Collection">
                    <rdf:Description rdf:about="http://OntoCAPE/upper_level/network_system.owl#Device"/>
                    <rdf:Description rdf:about="http://OntoCAPE/upper_level/network_system.owl#DirectedConnection"/>
                </owl:unionOf>
            </owl:Class>
        </rdfs:range>
        <rdfs:comment>The relation isSuccessorOf identifies all Devices and DirectedConnections that are successors of the considered one.</rdfs:comment>
    </owl:ObjectProperty>
    


    <!-- http://OntoCAPE/upper_level/network_system.owl#leaves -->

    <owl:ObjectProperty rdf:about="http://OntoCAPE/upper_level/network_system.owl#leaves">
        <rdfs:subPropertyOf rdf:resource="http://OntoCAPE/upper_level/network_system.owl#isSuccessorOf"/>
        <rdfs:domain rdf:resource="http://OntoCAPE/upper_level/network_system.owl#DirectedConnection"/>
        <rdfs:range rdf:resource="http://OntoCAPE/upper_level/network_system.owl#Device"/>
        <rdfs:comment>The relation Leaves connects an outgoing DirectedConnection to its source Device.</rdfs:comment>
    </owl:ObjectProperty>
    


    <!-- http://OntoCAPE/upper_level/network_system.owl#sameAs -->

    <owl:ObjectProperty rdf:about="http://OntoCAPE/upper_level/network_system.owl#sameAs">
        <rdfs:subPropertyOf rdf:resource="http://OntoCAPE/upper_level/system.owl#isDirectlyRelatedTo"/>
        <owl:inverseOf rdf:resource="http://OntoCAPE/upper_level/network_system.owl#sameAs"/>
        <rdf:type rdf:resource="http://www.w3.org/2002/07/owl#SymmetricProperty"/>
        <rdfs:domain rdf:resource="http://OntoCAPE/upper_level/network_system.owl#Connection"/>
        <rdfs:range>
            <owl:Class>
                <owl:intersectionOf rdf:parseType="Collection">
                    <rdf:Description rdf:about="http://OntoCAPE/upper_level/network_system.owl#Connection"/>
                    <owl:Restriction>
                        <owl:onProperty rdf:resource="http://OntoCAPE/upper_level/system.owl#isDirectlyConnectedTo"/>
                        <owl:someValuesFrom rdf:resource="http://OntoCAPE/upper_level/network_system.owl#Device"/>
                    </owl:Restriction>
                </owl:intersectionOf>
            </owl:Class>
        </rdfs:range>
        <rdfs:comment>The relation denotes a correspondence between a Connection and its placeholder in a composition hierarchy</rdfs:comment>
    </owl:ObjectProperty>
    


    <!-- http://OntoCAPE/upper_level/system.owl#comprises -->

    <owl:ObjectProperty rdf:about="http://OntoCAPE/upper_level/system.owl#comprises">
        <rdfs:subPropertyOf rdf:resource="http://meta_model/fundamental_concepts/fundamental_concepts.owl#inter-objectRelation"/>
        <rdf:type rdf:resource="http://www.w3.org/2002/07/owl#TransitiveProperty"/>
        <rdfs:domain rdf:resource="http://OntoCAPE/upper_level/system.owl#PropertySet"/>
        <rdfs:range rdf:resource="http://OntoCAPE/upper_level/system.owl#Property"/>
        <rdfs:comment>The relation Comprises indicates the members of a PropertySet.</rdfs:comment>
    </owl:ObjectProperty>
    


    <!-- http://OntoCAPE/upper_level/system.owl#comprisesDirectly -->

    <owl:ObjectProperty rdf:about="http://OntoCAPE/upper_level/system.owl#comprisesDirectly">
        <rdfs:subPropertyOf rdf:resource="http://OntoCAPE/upper_level/system.owl#comprises"/>
        <rdfs:comment>The relation ComprisesDirectly indicates the direct members of a PropertySet.</rdfs:comment>
    </owl:ObjectProperty>
    


    <!-- http://OntoCAPE/upper_level/system.owl#contains -->

    <owl:ObjectProperty rdf:about="http://OntoCAPE/upper_level/system.owl#contains">
        <rdfs:subPropertyOf rdf:resource="http://OntoCAPE/upper_level/system.owl#isRelatedTo"/>
        <rdf:type rdf:resource="http://www.w3.org/2002/07/owl#TransitiveProperty"/>
        <rdfs:domain rdf:resource="http://OntoCAPE/upper_level/system.owl#Supersystem"/>
        <rdfs:comment>The Contains relation constitutes an alternative to the hasSubsystem relation. It should be used instead of hasSubsystem 
-   if the hasSubsystem relation causes performance problems, or
-   if only one side of the aggregation relation is of interest, namely the indication of the constituting elements of a supersystem</rdfs:comment>
    </owl:ObjectProperty>
    


    <!-- http://OntoCAPE/upper_level/system.owl#containsDirectly -->

    <owl:ObjectProperty rdf:about="http://OntoCAPE/upper_level/system.owl#containsDirectly">
        <rdfs:subPropertyOf rdf:resource="http://OntoCAPE/upper_level/system.owl#contains"/>
        <rdfs:subPropertyOf rdf:resource="http://OntoCAPE/upper_level/system.owl#isDirectlyRelatedTo"/>
        <rdfs:comment>The relation containsDirectly is an alternative to the hasDirectSubsystem relation. It should be used instead of hasDirectSubsystem 
-   if the hasDirectSubsystem relation causes performance problems, or
-   if only one side of the aggregation relation is of interest, namely the indication of the direct constituents Supersystem.</rdfs:comment>
    </owl:ObjectProperty>
    


    <!-- http://OntoCAPE/upper_level/system.owl#hasAspectSystem -->

    <owl:ObjectProperty rdf:about="http://OntoCAPE/upper_level/system.owl#hasAspectSystem">
        <rdfs:subPropertyOf rdf:resource="http://OntoCAPE/upper_level/system.owl#isComposedOfSubsystem"/>
        <owl:inverseOf rdf:resource="http://OntoCAPE/upper_level/system.owl#representsAspectOf"/>
        <rdfs:range rdf:resource="http://OntoCAPE/upper_level/system.owl#AspectSystem"/>
        <rdfs:comment>The relation hasAspectSystem designates the AspectSystems of a System.</rdfs:comment>
    </owl:ObjectProperty>
    


    <!-- http://OntoCAPE/upper_level/system.owl#hasCharacteristic -->

    <owl:ObjectProperty rdf:about="http://OntoCAPE/upper_level/system.owl#hasCharacteristic">
        <rdfs:domain rdf:resource="http://OntoCAPE/upper_level/system.owl#System"/>
        <rdfs:range>
            <owl:Class>
                <owl:unionOf rdf:parseType="Collection">
                    <rdf:Description rdf:about="http://OntoCAPE/upper_level/system.owl#QuantitativeValue"/>
                    <rdf:Description rdf:about="http://OntoCAPE/upper_level/system.owl#ValueEnumeration"/>
                </owl:unionOf>
            </owl:Class>
        </rdfs:range>
        <rdfs:comment>The hasCharacteristic relation constitutes a shorthand notation for the specification of a ConstantProperty and its Value.</rdfs:comment>
    </owl:ObjectProperty>
    


    <!-- http://OntoCAPE/upper_level/system.owl#hasDimension -->

    <owl:ObjectProperty rdf:about="http://OntoCAPE/upper_level/system.owl#hasDimension">
        <rdf:type rdf:resource="http://www.w3.org/2002/07/owl#FunctionalProperty"/>
        <rdfs:domain>
            <owl:Class>
                <owl:unionOf rdf:parseType="Collection">
                    <rdf:Description rdf:about="http://OntoCAPE/upper_level/system.owl#Property"/>
                    <rdf:Description rdf:about="http://OntoCAPE/upper_level/system.owl#UnitOfMeasure"/>
                </owl:unionOf>
            </owl:Class>
        </rdfs:domain>
        <rdfs:range rdf:resource="http://OntoCAPE/upper_level/system.owl#PhysicalDimension"/>
        <rdfs:comment>The relation hasDimension specifies the PhysicalDimension of a PhysicalQuantity or a UnitOfMeasure.</rdfs:comment>
    </owl:ObjectProperty>
    


    <!-- http://OntoCAPE/upper_level/system.owl#hasDirectSubsystem -->

    <owl:ObjectProperty rdf:about="http://OntoCAPE/upper_level/system.owl#hasDirectSubsystem">
        <rdfs:subPropertyOf rdf:resource="http://OntoCAPE/upper_level/system.owl#hasSubsystem"/>
        <rdfs:subPropertyOf rdf:resource="http://OntoCAPE/upper_level/system.owl#isDirectlyRelatedTo"/>
        <owl:inverseOf rdf:resource="http://OntoCAPE/upper_level/system.owl#isDirectSubsystemOf"/>
        <rdfs:domain rdf:resource="http://OntoCAPE/upper_level/system.owl#Supersystem"/>
        <rdfs:range rdf:resource="http://OntoCAPE/upper_level/system.owl#Subsystem"/>
        <rdfs:comment>The relation hasDirectSubsystem refers from a Supersystem to its direct Subsystem.</rdfs:comment>
    </owl:ObjectProperty>
    


    <!-- http://OntoCAPE/upper_level/system.owl#hasProperty -->

    <owl:ObjectProperty rdf:about="http://OntoCAPE/upper_level/system.owl#hasProperty">
        <rdfs:subPropertyOf rdf:resource="http://meta_model/fundamental_concepts/fundamental_concepts.owl#inter-objectRelation"/>
        <owl:inverseOf rdf:resource="http://OntoCAPE/upper_level/system.owl#isPropertyOf"/>
        <rdf:type rdf:resource="http://www.w3.org/2002/07/owl#InverseFunctionalProperty"/>
        <rdfs:domain rdf:resource="http://OntoCAPE/upper_level/system.owl#System"/>
        <rdfs:range rdf:resource="http://OntoCAPE/upper_level/system.owl#Property"/>
        <rdfs:comment>The relation hasProperty indicates the Properties of a System.</rdfs:comment>
    </owl:ObjectProperty>
    


    <!-- http://OntoCAPE/upper_level/system.owl#hasSubsystem -->

    <owl:ObjectProperty rdf:about="http://OntoCAPE/upper_level/system.owl#hasSubsystem">
        <rdfs:subPropertyOf rdf:resource="http://OntoCAPE/upper_level/system.owl#isRelatedTo"/>
        <owl:inverseOf rdf:resource="http://OntoCAPE/upper_level/system.owl#isSubsystemOf"/>
        <rdf:type rdf:resource="http://www.w3.org/2002/07/owl#TransitiveProperty"/>
        <rdfs:domain rdf:resource="http://OntoCAPE/upper_level/system.owl#Supersystem"/>
        <rdfs:range rdf:resource="http://OntoCAPE/upper_level/system.owl#Subsystem"/>
        <rdfs:comment>The relation hasSubsystem denotes the relation between a Supersystem and its Subsystem.</rdfs:comment>
    </owl:ObjectProperty>
    


    <!-- http://OntoCAPE/upper_level/system.owl#hasUnitOfMeasure -->

    <owl:ObjectProperty rdf:about="http://OntoCAPE/upper_level/system.owl#hasUnitOfMeasure">
        <rdfs:subPropertyOf rdf:resource="http://meta_model/fundamental_concepts/fundamental_concepts.owl#object-featureRelation"/>
        <rdf:type rdf:resource="http://www.w3.org/2002/07/owl#FunctionalProperty"/>
        <rdfs:domain rdf:resource="http://OntoCAPE/upper_level/system.owl#QuantitativeValue"/>
        <rdfs:range rdf:resource="http://OntoCAPE/upper_level/system.owl#UnitOfMeasure"/>
        <rdfs:comment>The relation hasUnitOfMeasure establishes the UnitOfMeasure of a ScalarValue.</rdfs:comment>
    </owl:ObjectProperty>
    


    <!-- http://OntoCAPE/upper_level/system.owl#hasValue -->

    <owl:ObjectProperty rdf:about="http://OntoCAPE/upper_level/system.owl#hasValue">
        <rdfs:subPropertyOf rdf:resource="http://meta_model/fundamental_concepts/fundamental_concepts.owl#inter-objectRelation"/>
        <owl:inverseOf rdf:resource="http://OntoCAPE/upper_level/system.owl#isValueOf"/>
        <rdf:type rdf:resource="http://www.w3.org/2002/07/owl#InverseFunctionalProperty"/>
        <rdfs:domain rdf:resource="http://OntoCAPE/upper_level/system.owl#Property"/>
        <rdfs:range rdf:resource="http://OntoCAPE/upper_level/system.owl#Value"/>
        <rdfs:comment>The hasValue relation designates the Values of a Property.</rdfs:comment>
    </owl:ObjectProperty>
    


    <!-- http://OntoCAPE/upper_level/system.owl#isBackdropOf -->

    <owl:ObjectProperty rdf:about="http://OntoCAPE/upper_level/system.owl#isBackdropOf">
        <rdfs:subPropertyOf rdf:resource="http://meta_model/fundamental_concepts/fundamental_concepts.owl#inter-objectRelation"/>
        <owl:inverseOf rdf:resource="http://OntoCAPE/upper_level/system.owl#isObservedAgainstBackdrop"/>
        <rdfs:domain rdf:resource="http://OntoCAPE/upper_level/system.owl#Value"/>
        <rdfs:range rdf:resource="http://OntoCAPE/upper_level/system.owl#Value"/>
        <rdfs:comment>The isBackdropOf relation states that the Value serves as a backdrop for the observation of some other Value.</rdfs:comment>
    </owl:ObjectProperty>
    


    <!-- http://OntoCAPE/upper_level/system.owl#isComposedOfSubsystem -->

    <owl:ObjectProperty rdf:about="http://OntoCAPE/upper_level/system.owl#isComposedOfSubsystem">
        <rdfs:subPropertyOf rdf:resource="http://OntoCAPE/upper_level/system.owl#hasDirectSubsystem"/>
        <owl:inverseOf rdf:resource="http://OntoCAPE/upper_level/system.owl#isExclusivelySubsystemOf"/>
        <rdfs:domain rdf:resource="http://OntoCAPE/upper_level/system.owl#Supersystem"/>
        <rdfs:comment>The relation isComposedOf indicates the non-sharable, direct Subsystem of a Supersystem.</rdfs:comment>
    </owl:ObjectProperty>
    


    <!-- http://OntoCAPE/upper_level/system.owl#isConnectedTo -->

    <owl:ObjectProperty rdf:about="http://OntoCAPE/upper_level/system.owl#isConnectedTo">
        <rdfs:subPropertyOf rdf:resource="http://OntoCAPE/upper_level/system.owl#isRelatedTo"/>
        <owl:inverseOf rdf:resource="http://OntoCAPE/upper_level/system.owl#isConnectedTo"/>
        <rdf:type rdf:resource="http://www.w3.org/2002/07/owl#SymmetricProperty"/>
        <rdf:type rdf:resource="http://www.w3.org/2002/07/owl#TransitiveProperty"/>
        <rdfs:domain rdf:resource="http://OntoCAPE/upper_level/system.owl#System"/>
        <rdfs:range rdf:resource="http://OntoCAPE/upper_level/system.owl#System"/>
        <rdfs:comment>The relation isConnectedTo represents topological connectivity between System.</rdfs:comment>
    </owl:ObjectProperty>
    


    <!-- http://OntoCAPE/upper_level/system.owl#isConsideredUnderAspectOf -->

    <owl:ObjectProperty rdf:about="http://OntoCAPE/upper_level/system.owl#isConsideredUnderAspectOf">
        <rdfs:subPropertyOf rdf:resource="http://meta_model/fundamental_concepts/fundamental_concepts.owl#object-featureRelation"/>
        <rdfs:domain rdf:resource="http://OntoCAPE/upper_level/system.owl#AspectSystem"/>
        <rdfs:range rdf:resource="http://OntoCAPE/upper_level/system.owl#Aspect"/>
        <rdfs:comment>The relation isConsideredUnderAspectOf indicates the type of an AspectSystem by referring to an instance of the Aspect class.</rdfs:comment>
    </owl:ObjectProperty>
    


    <!-- http://OntoCAPE/upper_level/system.owl#isDirectSubsystemOf -->

    <owl:ObjectProperty rdf:about="http://OntoCAPE/upper_level/system.owl#isDirectSubsystemOf">
        <rdfs:subPropertyOf rdf:resource="http://OntoCAPE/upper_level/system.owl#isDirectlyRelatedTo"/>
        <rdfs:subPropertyOf rdf:resource="http://OntoCAPE/upper_level/system.owl#isSubsystemOf"/>
        <rdfs:domain rdf:resource="http://OntoCAPE/upper_level/system.owl#Subsystem"/>
        <rdfs:range rdf:resource="http://OntoCAPE/upper_level/system.owl#Supersystem"/>
        <rdfs:comment>The relation isDirectlySubsystemOf links a Subsystem to its direct Supersystem.</rdfs:comment>
    </owl:ObjectProperty>
    


    <!-- http://OntoCAPE/upper_level/system.owl#isDirectlyConnectedTo -->

    <owl:ObjectProperty rdf:about="http://OntoCAPE/upper_level/system.owl#isDirectlyConnectedTo">
        <rdfs:subPropertyOf rdf:resource="http://OntoCAPE/upper_level/system.owl#isConnectedTo"/>
        <rdfs:subPropertyOf rdf:resource="http://OntoCAPE/upper_level/system.owl#isDirectlyRelatedTo"/>
        <rdf:type rdf:resource="http://www.w3.org/2002/07/owl#SymmetricProperty"/>
        <rdfs:comment>The relation isDirectlyConnectedTo denotes the direct topological connectedness of two System.</rdfs:comment>
    </owl:ObjectProperty>
    


    <!-- http://OntoCAPE/upper_level/system.owl#isDirectlyRelatedTo -->

    <owl:ObjectProperty rdf:about="http://OntoCAPE/upper_level/system.owl#isDirectlyRelatedTo">
        <rdfs:subPropertyOf rdf:resource="http://OntoCAPE/upper_level/system.owl#isRelatedTo"/>
        <owl:inverseOf rdf:resource="http://OntoCAPE/upper_level/system.owl#isDirectlyRelatedTo"/>
        <rdf:type rdf:resource="http://www.w3.org/2002/07/owl#SymmetricProperty"/>
        <rdfs:comment>The relation isDirectlyRelatedTo subsumes all kinds of direct inter-system relations.</rdfs:comment>
    </owl:ObjectProperty>
    


    <!-- http://OntoCAPE/upper_level/system.owl#isExclusivelySubsystemOf -->

    <owl:ObjectProperty rdf:about="http://OntoCAPE/upper_level/system.owl#isExclusivelySubsystemOf">
        <rdfs:subPropertyOf rdf:resource="http://OntoCAPE/upper_level/system.owl#isDirectSubsystemOf"/>
        <rdfs:domain rdf:resource="http://OntoCAPE/upper_level/system.owl#Subsystem"/>
        <rdfs:range rdf:resource="http://OntoCAPE/upper_level/system.owl#Supersystem"/>
        <rdfs:comment>The relation isExclusivelySubsystemOf links a non-sharable Subsystem to its direct Supersystem.</rdfs:comment>
    </owl:ObjectProperty>
    


    <!-- http://OntoCAPE/upper_level/system.owl#isModeledBy -->

    <owl:ObjectProperty rdf:about="http://OntoCAPE/upper_level/system.owl#isModeledBy">
        <rdfs:subPropertyOf rdf:resource="http://OntoCAPE/upper_level/system.owl#isDirectlyRelatedTo"/>
        <owl:inverseOf rdf:resource="http://OntoCAPE/upper_level/system.owl#models"/>
        <rdfs:domain rdf:resource="http://OntoCAPE/upper_level/system.owl#System"/>
        <rdfs:range rdf:resource="http://OntoCAPE/upper_level/system.owl#Model"/>
        <rdfs:comment>The relation isModeldBy points from a modeled System to its Model.</rdfs:comment>
    </owl:ObjectProperty>
    


    <!-- http://OntoCAPE/upper_level/system.owl#isObservedAgainstBackdrop -->

    <owl:ObjectProperty rdf:about="http://OntoCAPE/upper_level/system.owl#isObservedAgainstBackdrop">
        <rdfs:subPropertyOf rdf:resource="http://meta_model/fundamental_concepts/fundamental_concepts.owl#inter-objectRelation"/>
        <rdfs:domain rdf:resource="http://OntoCAPE/upper_level/system.owl#Value"/>
        <rdfs:range rdf:resource="http://OntoCAPE/upper_level/system.owl#Value"/>
        <rdfs:comment>The isObservedAgainstBackdrop relation maps a Value against a backdrop Value.</rdfs:comment>
    </owl:ObjectProperty>
    


    <!-- http://OntoCAPE/upper_level/system.owl#isPropertyOf -->

    <owl:ObjectProperty rdf:about="http://OntoCAPE/upper_level/system.owl#isPropertyOf">
        <rdfs:subPropertyOf rdf:resource="http://meta_model/fundamental_concepts/fundamental_concepts.owl#inter-objectRelation"/>
        <rdf:type rdf:resource="http://www.w3.org/2002/07/owl#FunctionalProperty"/>
        <rdfs:domain rdf:resource="http://OntoCAPE/upper_level/system.owl#Property"/>
        <rdfs:range rdf:resource="http://OntoCAPE/upper_level/system.owl#System"/>
        <rdfs:comment>The relation isPropertyOf links a Property instance to a System instance.</rdfs:comment>
    </owl:ObjectProperty>
    


    <!-- http://OntoCAPE/upper_level/system.owl#isRelatedTo -->

    <owl:ObjectProperty rdf:about="http://OntoCAPE/upper_level/system.owl#isRelatedTo">
        <rdfs:subPropertyOf rdf:resource="http://meta_model/fundamental_concepts/fundamental_concepts.owl#inter-objectRelation"/>
        <owl:inverseOf rdf:resource="http://OntoCAPE/upper_level/system.owl#isRelatedTo"/>
        <rdf:type rdf:resource="http://www.w3.org/2002/07/owl#SymmetricProperty"/>
        <rdf:type rdf:resource="http://www.w3.org/2002/07/owl#TransitiveProperty"/>
        <rdfs:domain rdf:resource="http://OntoCAPE/upper_level/system.owl#System"/>
        <rdfs:range rdf:resource="http://OntoCAPE/upper_level/system.owl#System"/>
        <rdfs:comment>The relation isRelatedTo subsumes all kinds of inter-system relations.</rdfs:comment>
    </owl:ObjectProperty>
    


    <!-- http://OntoCAPE/upper_level/system.owl#isSubsystemOf -->

    <owl:ObjectProperty rdf:about="http://OntoCAPE/upper_level/system.owl#isSubsystemOf">
        <rdfs:subPropertyOf rdf:resource="http://OntoCAPE/upper_level/system.owl#isRelatedTo"/>
        <rdf:type rdf:resource="http://www.w3.org/2002/07/owl#TransitiveProperty"/>
        <rdfs:domain rdf:resource="http://OntoCAPE/upper_level/system.owl#Subsystem"/>
        <rdfs:range rdf:resource="http://OntoCAPE/upper_level/system.owl#Supersystem"/>
        <rdfs:comment>The relation isSubsystemOf refers from a Subsystem to its Supersystem.</rdfs:comment>
    </owl:ObjectProperty>
    


    <!-- http://OntoCAPE/upper_level/system.owl#isValueOf -->

    <owl:ObjectProperty rdf:about="http://OntoCAPE/upper_level/system.owl#isValueOf">
        <rdfs:subPropertyOf rdf:resource="http://meta_model/fundamental_concepts/fundamental_concepts.owl#inter-objectRelation"/>
        <rdf:type rdf:resource="http://www.w3.org/2002/07/owl#FunctionalProperty"/>
        <rdfs:domain rdf:resource="http://OntoCAPE/upper_level/system.owl#Value"/>
        <rdfs:range rdf:resource="http://OntoCAPE/upper_level/system.owl#Property"/>
        <rdfs:comment>The relation isValueOf assigns a Value to a Property.</rdfs:comment>
    </owl:ObjectProperty>
    


    <!-- http://OntoCAPE/upper_level/system.owl#models -->

    <owl:ObjectProperty rdf:about="http://OntoCAPE/upper_level/system.owl#models">
        <rdfs:subPropertyOf rdf:resource="http://OntoCAPE/upper_level/system.owl#isDirectlyRelatedTo"/>
        <rdfs:domain rdf:resource="http://OntoCAPE/upper_level/system.owl#Model"/>
        <rdfs:range rdf:resource="http://OntoCAPE/upper_level/system.owl#System"/>
        <rdfs:comment>The relation &apos;models&apos; links a Model to the modeled System.</rdfs:comment>
    </owl:ObjectProperty>
    


    <!-- http://OntoCAPE/upper_level/system.owl#qualitativeValue -->

    <owl:ObjectProperty rdf:about="http://OntoCAPE/upper_level/system.owl#qualitativeValue">
        <rdfs:subPropertyOf rdf:resource="http://meta_model/fundamental_concepts/fundamental_concepts.owl#object-featureRelation"/>
        <rdfs:domain rdf:resource="http://OntoCAPE/upper_level/system.owl#QualitativeValue"/>
        <rdfs:range rdf:resource="http://OntoCAPE/upper_level/system.owl#ValueEnumeration"/>
        <rdfs:comment>The relation qualitativeValue specifies the actual value of a QualitativeValue.</rdfs:comment>
    </owl:ObjectProperty>
    


    <!-- http://OntoCAPE/upper_level/system.owl#representsAspectOf -->

    <owl:ObjectProperty rdf:about="http://OntoCAPE/upper_level/system.owl#representsAspectOf">
        <rdfs:subPropertyOf rdf:resource="http://OntoCAPE/upper_level/system.owl#isExclusivelySubsystemOf"/>
        <rdfs:domain rdf:resource="http://OntoCAPE/upper_level/system.owl#AspectSystem"/>
        <rdfs:comment>The relation representsAspectOf links a AspectSystem to its respective System.</rdfs:comment>
    </owl:ObjectProperty>
    


    <!-- http://meta_model/fundamental_concepts/fundamental_concepts.owl#inter-objectRelation -->

    <owl:ObjectProperty rdf:about="http://meta_model/fundamental_concepts/fundamental_concepts.owl#inter-objectRelation"/>
    


    <!-- http://meta_model/fundamental_concepts/fundamental_concepts.owl#object-featureRelation -->

    <owl:ObjectProperty rdf:about="http://meta_model/fundamental_concepts/fundamental_concepts.owl#object-featureRelation"/>
    


    <!-- 
    ///////////////////////////////////////////////////////////////////////////////////////
    //
    // Data properties
    //
    ///////////////////////////////////////////////////////////////////////////////////////
     -->

    


    <!-- http://OntoCAPE/chemical_process_system/CPS_function/process.owl#is_at_numbered_tray -->

    <owl:DatatypeProperty rdf:about="http://OntoCAPE/chemical_process_system/CPS_function/process.owl#is_at_numbered_tray">
        <rdfs:range rdf:resource="http://www.w3.org/2001/XMLSchema#integer"/>
    </owl:DatatypeProperty>
    


    <!-- http://OntoCAPE/upper_level/system.owl#numericalValue -->

    <owl:DatatypeProperty rdf:about="http://OntoCAPE/upper_level/system.owl#numericalValue">
        <rdfs:domain rdf:resource="http://OntoCAPE/upper_level/system.owl#ScalarValue"/>
        <rdfs:comment>The attribute numericalValue specifies the number part of a QuantitativeValue.</rdfs:comment>
    </owl:DatatypeProperty>
    


    <!-- http://OntoCAPE/upper_level/system.owl#value -->

    <owl:DatatypeProperty rdf:about="http://OntoCAPE/upper_level/system.owl#value">
        <rdfs:domain rdf:resource="http://OntoCAPE/upper_level/system.owl#QualitativeValue"/>
        <rdfs:comment>The Value attribute holds the actual value of a QualitativeValue.</rdfs:comment>
    </owl:DatatypeProperty>
    


    <!-- 
    ///////////////////////////////////////////////////////////////////////////////////////
    //
    // Classes
    //
    ///////////////////////////////////////////////////////////////////////////////////////
     -->

    


    <!-- http://OntoCAPE/chemical_process_system/CPS_function/process.owl#AggregatedProcessStep -->

    <owl:Class rdf:about="http://OntoCAPE/chemical_process_system/CPS_function/process.owl#AggregatedProcessStep">
        <owl:equivalentClass>
            <owl:Class>
                <owl:intersectionOf rdf:parseType="Collection">
                    <rdf:Description rdf:about="http://OntoCAPE/chemical_process_system/CPS_function/process.owl#ProcessStep"/>
                    <owl:Restriction>
                        <owl:onProperty rdf:resource="http://OntoCAPE/upper_level/system.owl#hasDirectSubsystem"/>
                        <owl:someValuesFrom rdf:resource="http://OntoCAPE/chemical_process_system/CPS_function/process.owl#ProcessStep"/>
                    </owl:Restriction>
                </owl:intersectionOf>
            </owl:Class>
        </owl:equivalentClass>
        <rdfs:comment>An AggregatedProcessStep is a ProcessStep which consists of a number of ProcessSteps in a certain sequence.</rdfs:comment>
    </owl:Class>
    


    <!-- http://OntoCAPE/chemical_process_system/CPS_function/process.owl#BatchProcess -->

    <owl:Class rdf:about="http://OntoCAPE/chemical_process_system/CPS_function/process.owl#BatchProcess">
        <owl:equivalentClass>
            <owl:Class>
                <owl:intersectionOf rdf:parseType="Collection">
                    <rdf:Description rdf:about="http://OntoCAPE/chemical_process_system/CPS_function/process.owl#ProcessState"/>
                    <owl:Restriction>
                        <owl:onProperty rdf:resource="http://OntoCAPE/chemical_process_system/CPS_function/process.owl#hasOperationMode"/>
                        <owl:hasValue rdf:resource="http://OntoCAPE/chemical_process_system/CPS_function/process.owl#Batch"/>
                    </owl:Restriction>
                </owl:intersectionOf>
            </owl:Class>
        </owl:equivalentClass>
        <owl:disjointWith rdf:resource="http://OntoCAPE/chemical_process_system/CPS_function/process.owl#ProcessStream"/>
        <rdfs:comment>A BatchProcess indicates the batch mode of operation applied to the Process.</rdfs:comment>
    </owl:Class>
    


    <!-- http://OntoCAPE/chemical_process_system/CPS_function/process.owl#By-product -->

    <owl:Class rdf:about="http://OntoCAPE/chemical_process_system/CPS_function/process.owl#By-product">
        <rdfs:subClassOf rdf:resource="http://OntoCAPE/chemical_process_system/CPS_function/process.owl#EndProduct"/>
        <owl:disjointWith rdf:resource="http://OntoCAPE/chemical_process_system/CPS_function/process.owl#Co-product"/>
        <owl:disjointWith rdf:resource="http://OntoCAPE/chemical_process_system/CPS_function/process.owl#CoreProduct"/>
        <rdfs:comment>A Byproduct is an EndProduct whose production is unavoidable while a CoreProduct is produced.</rdfs:comment>
    </owl:Class>
    


    <!-- http://OntoCAPE/chemical_process_system/CPS_function/process.owl#Co-product -->

    <owl:Class rdf:about="http://OntoCAPE/chemical_process_system/CPS_function/process.owl#Co-product">
        <rdfs:subClassOf rdf:resource="http://OntoCAPE/chemical_process_system/CPS_function/process.owl#EndProduct"/>
        <owl:disjointWith rdf:resource="http://OntoCAPE/chemical_process_system/CPS_function/process.owl#CoreProduct"/>
        <rdfs:comment>A Co- product is an EndProduct whose production is unintended.</rdfs:comment>
    </owl:Class>
    


    <!-- http://OntoCAPE/chemical_process_system/CPS_function/process.owl#Combination -->

    <owl:Class rdf:about="http://OntoCAPE/chemical_process_system/CPS_function/process.owl#Combination">
        <rdfs:subClassOf rdf:resource="http://OntoCAPE/chemical_process_system/CPS_function/process.owl#UnitOperation"/>
        <rdfs:subClassOf>
            <owl:Restriction>
                <owl:onProperty rdf:resource="http://OntoCAPE/upper_level/network_system.owl#hasInput"/>
                <owl:minCardinality rdf:datatype="http://www.w3.org/2001/XMLSchema#nonNegativeInteger">2</owl:minCardinality>
            </owl:Restriction>
        </rdfs:subClassOf>
        <rdfs:subClassOf>
            <owl:Restriction>
                <owl:onProperty rdf:resource="http://OntoCAPE/upper_level/network_system.owl#hasOutput"/>
                <owl:cardinality rdf:datatype="http://www.w3.org/2001/XMLSchema#nonNegativeInteger">1</owl:cardinality>
            </owl:Restriction>
        </rdfs:subClassOf>
        <owl:disjointWith rdf:resource="http://OntoCAPE/chemical_process_system/CPS_function/process.owl#EnthalpyChange"/>
        <owl:disjointWith rdf:resource="http://OntoCAPE/chemical_process_system/CPS_function/process.owl#Separation"/>
        <rdfs:comment>A combination in terms of unit operation means to get together different process steps to achieve a particular one.</rdfs:comment>
    </owl:Class>
    


    <!-- http://OntoCAPE/chemical_process_system/CPS_function/process.owl#CoreProduct -->

    <owl:Class rdf:about="http://OntoCAPE/chemical_process_system/CPS_function/process.owl#CoreProduct">
        <rdfs:subClassOf rdf:resource="http://OntoCAPE/chemical_process_system/CPS_function/process.owl#EndProduct"/>
        <rdfs:comment>A CoreProduct is a main (or an intended) EndProduct.</rdfs:comment>
    </owl:Class>
    


    <!-- http://OntoCAPE/chemical_process_system/CPS_function/process.owl#EndProduct -->

    <owl:Class rdf:about="http://OntoCAPE/chemical_process_system/CPS_function/process.owl#EndProduct">
        <rdfs:subClassOf rdf:resource="http://OntoCAPE/chemical_process_system/CPS_function/process.owl#OutputProduct"/>
        <owl:disjointWith rdf:resource="http://OntoCAPE/chemical_process_system/CPS_function/process.owl#WasteProduct"/>
        <rdfs:comment>An EndProduct is an OutputProduct that is valuable.</rdfs:comment>
    </owl:Class>
    


    <!-- http://OntoCAPE/chemical_process_system/CPS_function/process.owl#EnthalpyChange -->

    <owl:Class rdf:about="http://OntoCAPE/chemical_process_system/CPS_function/process.owl#EnthalpyChange">
        <rdfs:subClassOf rdf:resource="http://OntoCAPE/chemical_process_system/CPS_function/process.owl#UnitOperation"/>
        <rdfs:subClassOf>
            <owl:Restriction>
                <owl:onProperty rdf:resource="http://OntoCAPE/upper_level/network_system.owl#hasInput"/>
                <owl:cardinality rdf:datatype="http://www.w3.org/2001/XMLSchema#nonNegativeInteger">1</owl:cardinality>
            </owl:Restriction>
        </rdfs:subClassOf>
        <rdfs:subClassOf>
            <owl:Restriction>
                <owl:onProperty rdf:resource="http://OntoCAPE/upper_level/network_system.owl#hasOutput"/>
                <owl:cardinality rdf:datatype="http://www.w3.org/2001/XMLSchema#nonNegativeInteger">1</owl:cardinality>
            </owl:Restriction>
        </rdfs:subClassOf>
        <owl:disjointWith rdf:resource="http://OntoCAPE/chemical_process_system/CPS_function/process.owl#Separation"/>
        <rdfs:comment>EnthalpyChange in terms of unit operation considers a conversion of energy which often result in a change of the state of aggregation.</rdfs:comment>
    </owl:Class>
    


    <!-- http://OntoCAPE/chemical_process_system/CPS_function/process.owl#FlashVaporRatio -->

    <owl:Class rdf:about="http://OntoCAPE/chemical_process_system/CPS_function/process.owl#FlashVaporRatio">
        <rdfs:subClassOf rdf:resource="http://OntoCAPE/chemical_process_system/CPS_function/process.owl#ProcessStepProperty"/>
        <rdfs:subClassOf>
            <owl:Restriction>
                <owl:onProperty rdf:resource="http://OntoCAPE/upper_level/system.owl#hasDimension"/>
                <owl:hasValue rdf:resource="http://OntoCAPE/supporting_concepts/physical_dimension/physical_dimension.owl#identity_dimension"/>
            </owl:Restriction>
        </rdfs:subClassOf>
        <owl:disjointWith rdf:resource="http://OntoCAPE/chemical_process_system/CPS_function/process.owl#KeyChemicalComponentConversionRatio"/>
    </owl:Class>
    


    <!-- http://OntoCAPE/chemical_process_system/CPS_function/process.owl#Flashing -->

    <owl:Class rdf:about="http://OntoCAPE/chemical_process_system/CPS_function/process.owl#Flashing">
        <rdfs:subClassOf rdf:resource="http://OntoCAPE/chemical_process_system/CPS_function/process.owl#Separation"/>
        <rdfs:subClassOf>
            <owl:Restriction>
                <owl:onProperty rdf:resource="http://OntoCAPE/chemical_process_system/CPS_function/process.owl#hasVapourRatio"/>
                <owl:someValuesFrom rdf:resource="http://OntoCAPE/chemical_process_system/CPS_function/process.owl#FlashVaporRatio"/>
            </owl:Restriction>
        </rdfs:subClassOf>
        <rdfs:subClassOf>
            <owl:Restriction>
                <owl:onProperty rdf:resource="http://OntoCAPE/chemical_process_system/CPS_function/process.owl#hasVapourRatio"/>
                <owl:cardinality rdf:datatype="http://www.w3.org/2001/XMLSchema#nonNegativeInteger">1</owl:cardinality>
            </owl:Restriction>
        </rdfs:subClassOf>
        <rdfs:subClassOf>
            <owl:Restriction>
                <owl:onProperty rdf:resource="http://OntoCAPE/upper_level/network_system.owl#hasInput"/>
                <owl:cardinality rdf:datatype="http://www.w3.org/2001/XMLSchema#nonNegativeInteger">1</owl:cardinality>
            </owl:Restriction>
        </rdfs:subClassOf>
        <rdfs:subClassOf>
            <owl:Restriction>
                <owl:onProperty rdf:resource="http://OntoCAPE/upper_level/network_system.owl#hasOutput"/>
                <owl:cardinality rdf:datatype="http://www.w3.org/2001/XMLSchema#nonNegativeInteger">2</owl:cardinality>
            </owl:Restriction>
        </rdfs:subClassOf>
        <owl:disjointWith rdf:resource="http://OntoCAPE/chemical_process_system/CPS_function/process.owl#Leaching"/>
        <rdfs:comment>Flashing utilized the state of phase equilibrium between a vapor and a liquid phase and the resulting material transport if a mixture with different fugacity is existent. In terms of unit operation this is usually accomplished in a vessel.</rdfs:comment>
    </owl:Class>
    


    <!-- http://OntoCAPE/chemical_process_system/CPS_function/process.owl#Fragmentation -->

    <owl:Class rdf:about="http://OntoCAPE/chemical_process_system/CPS_function/process.owl#Fragmentation">
        <rdfs:subClassOf rdf:resource="http://OntoCAPE/chemical_process_system/CPS_function/process.owl#UnitOperation"/>
        <rdfs:comment>Fragmentation in terms of unit operation is the breakup of solid material for further processing.</rdfs:comment>
    </owl:Class>
    


    <!-- http://OntoCAPE/chemical_process_system/CPS_function/process.owl#IntermediateProduct -->

    <owl:Class rdf:about="http://OntoCAPE/chemical_process_system/CPS_function/process.owl#IntermediateProduct">
        <owl:equivalentClass>
            <owl:Class>
                <owl:intersectionOf rdf:parseType="Collection">
                    <rdf:Description rdf:about="http://OntoCAPE/chemical_process_system/CPS_function/process.owl#ProcessState"/>
                    <owl:Restriction>
                        <owl:onProperty rdf:resource="http://OntoCAPE/upper_level/network_system.owl#enters"/>
                        <owl:someValuesFrom rdf:resource="http://OntoCAPE/chemical_process_system/CPS_function/process.owl#ProcessStep"/>
                    </owl:Restriction>
                    <owl:Restriction>
                        <owl:onProperty rdf:resource="http://OntoCAPE/upper_level/network_system.owl#leaves"/>
                        <owl:someValuesFrom rdf:resource="http://OntoCAPE/chemical_process_system/CPS_function/process.owl#ProcessStep"/>
                    </owl:Restriction>
                </owl:intersectionOf>
            </owl:Class>
        </owl:equivalentClass>
        <owl:disjointWith rdf:resource="http://OntoCAPE/chemical_process_system/CPS_function/process.owl#RawMaterial"/>
        <rdfs:comment>An IntermediateProduct is a ChemicalProduct that is produced in a ProcessStep and is used in another ProcessStep in the whole processing system.</rdfs:comment>
    </owl:Class>
    


    <!-- http://OntoCAPE/chemical_process_system/CPS_function/process.owl#KeyChemicalComponentConversionRatio -->

    <owl:Class rdf:about="http://OntoCAPE/chemical_process_system/CPS_function/process.owl#KeyChemicalComponentConversionRatio">
        <rdfs:subClassOf rdf:resource="http://OntoCAPE/chemical_process_system/CPS_function/process.owl#ProcessStepProperty"/>
        <rdfs:subClassOf>
            <owl:Restriction>
                <owl:onProperty rdf:resource="http://OntoCAPE/upper_level/system.owl#hasDimension"/>
                <owl:hasValue rdf:resource="http://OntoCAPE/supporting_concepts/physical_dimension/physical_dimension.owl#identity_dimension"/>
            </owl:Restriction>
        </rdfs:subClassOf>
    </owl:Class>
    


    <!-- http://OntoCAPE/chemical_process_system/CPS_function/process.owl#Leaching -->

    <owl:Class rdf:about="http://OntoCAPE/chemical_process_system/CPS_function/process.owl#Leaching">
        <rdfs:subClassOf rdf:resource="http://OntoCAPE/chemical_process_system/CPS_function/process.owl#Separation"/>
        <rdfs:subClassOf>
            <owl:Restriction>
                <owl:onProperty rdf:resource="http://OntoCAPE/upper_level/network_system.owl#hasInput"/>
                <owl:cardinality rdf:datatype="http://www.w3.org/2001/XMLSchema#nonNegativeInteger">2</owl:cardinality>
            </owl:Restriction>
        </rdfs:subClassOf>
        <rdfs:subClassOf>
            <owl:Restriction>
                <owl:onProperty rdf:resource="http://OntoCAPE/upper_level/network_system.owl#hasOutput"/>
                <owl:cardinality rdf:datatype="http://www.w3.org/2001/XMLSchema#nonNegativeInteger">2</owl:cardinality>
            </owl:Restriction>
        </rdfs:subClassOf>
        <rdfs:comment>Leaching in terms of unit operation is a particular form of extraction. Usually, a solute, a insolvable carrier and a solvent are applied for solid extraction</rdfs:comment>
    </owl:Class>
    


    <!-- http://OntoCAPE/chemical_process_system/CPS_function/process.owl#Mixing -->

    <owl:Class rdf:about="http://OntoCAPE/chemical_process_system/CPS_function/process.owl#Mixing">
        <rdfs:subClassOf rdf:resource="http://OntoCAPE/chemical_process_system/CPS_function/process.owl#Combination"/>
        <rdfs:comment>Mixing in terms of unit operations is a special type of combination which results in a mixture which is required for further processing. It is usually accomplished by means of stirrer.</rdfs:comment>
    </owl:Class>
    


    <!-- http://OntoCAPE/chemical_process_system/CPS_function/process.owl#ModeOfOperation -->

    <owl:Class rdf:about="http://OntoCAPE/chemical_process_system/CPS_function/process.owl#ModeOfOperation">
        <owl:equivalentClass>
            <owl:Class>
                <owl:oneOf rdf:parseType="Collection">
                    <rdf:Description rdf:about="http://OntoCAPE/chemical_process_system/CPS_function/process.owl#Batch"/>
                    <rdf:Description rdf:about="http://OntoCAPE/chemical_process_system/CPS_function/process.owl#Continuous"/>
                </owl:oneOf>
            </owl:Class>
        </owl:equivalentClass>
        <rdfs:subClassOf rdf:resource="http://OntoCAPE/meta_model/fundamental_concepts/fundamental_concepts.owl#ValueSet"/>
    </owl:Class>
    


    <!-- http://OntoCAPE/chemical_process_system/CPS_function/process.owl#NonReusableWasteProduct -->

    <owl:Class rdf:about="http://OntoCAPE/chemical_process_system/CPS_function/process.owl#NonReusableWasteProduct">
        <rdfs:subClassOf rdf:resource="http://OntoCAPE/chemical_process_system/CPS_function/process.owl#WasteProduct"/>
        <rdfs:comment>A NonReusableWasteProduct is a waste product that can not be reused.</rdfs:comment>
    </owl:Class>
    


    <!-- http://OntoCAPE/chemical_process_system/CPS_function/process.owl#OutputProduct -->

    <owl:Class rdf:about="http://OntoCAPE/chemical_process_system/CPS_function/process.owl#OutputProduct">
        <rdfs:subClassOf rdf:resource="http://OntoCAPE/chemical_process_system/CPS_function/process.owl#ProcessState"/>
        <rdfs:subClassOf>
            <owl:Restriction>
                <owl:onProperty rdf:resource="http://OntoCAPE/upper_level/network_system.owl#leaves"/>
                <owl:someValuesFrom rdf:resource="http://OntoCAPE/chemical_process_system/CPS_function/process.owl#ProcessStep"/>
            </owl:Restriction>
        </rdfs:subClassOf>
        <rdfs:subClassOf>
            <owl:Restriction>
                <owl:onProperty rdf:resource="http://OntoCAPE/upper_level/network_system.owl#enters"/>
                <owl:cardinality rdf:datatype="http://www.w3.org/2001/XMLSchema#nonNegativeInteger">0</owl:cardinality>
            </owl:Restriction>
        </rdfs:subClassOf>
        <owl:disjointWith rdf:resource="http://OntoCAPE/chemical_process_system/CPS_function/process.owl#RawMaterial"/>
        <rdfs:comment>An OutputProduct is a Material that is output by a ProcessStep.</rdfs:comment>
    </owl:Class>
    


    <!-- http://OntoCAPE/chemical_process_system/CPS_function/process.owl#PhaseChange -->

    <owl:Class rdf:about="http://OntoCAPE/chemical_process_system/CPS_function/process.owl#PhaseChange">
        <rdfs:subClassOf rdf:resource="http://OntoCAPE/chemical_process_system/CPS_function/process.owl#EnthalpyChange"/>
        <owl:disjointWith rdf:resource="http://OntoCAPE/chemical_process_system/CPS_function/process.owl#PressureChange"/>
        <owl:disjointWith rdf:resource="http://OntoCAPE/chemical_process_system/CPS_function/process.owl#TemperatureChange"/>
        <rdfs:comment>PhaseChange is a specialization of EnthalpyChange an usually it is applied for the purpose of heat exchange between spatially separated phases</rdfs:comment>
    </owl:Class>
    


    <!-- http://OntoCAPE/chemical_process_system/CPS_function/process.owl#PressureChange -->

    <owl:Class rdf:about="http://OntoCAPE/chemical_process_system/CPS_function/process.owl#PressureChange">
        <rdfs:subClassOf rdf:resource="http://OntoCAPE/chemical_process_system/CPS_function/process.owl#EnthalpyChange"/>
        <rdfs:subClassOf>
            <owl:Restriction>
                <owl:onProperty rdf:resource="http://OntoCAPE/chemical_process_system/CPS_function/process.owl#hasPressureDifference"/>
                <owl:someValuesFrom rdf:resource="http://OntoCAPE/chemical_process_system/CPS_function/process.owl#PressureDifference"/>
            </owl:Restriction>
        </rdfs:subClassOf>
        <rdfs:subClassOf>
            <owl:Restriction>
                <owl:onProperty rdf:resource="http://OntoCAPE/chemical_process_system/CPS_function/process.owl#hasPressureDifference"/>
                <owl:allValuesFrom rdf:resource="http://OntoCAPE/chemical_process_system/CPS_function/process.owl#PressureDifference"/>
            </owl:Restriction>
        </rdfs:subClassOf>
        <rdfs:subClassOf>
            <owl:Restriction>
                <owl:onProperty rdf:resource="http://OntoCAPE/chemical_process_system/CPS_function/process.owl#hasPressureDifference"/>
                <owl:cardinality rdf:datatype="http://www.w3.org/2001/XMLSchema#nonNegativeInteger">1</owl:cardinality>
            </owl:Restriction>
        </rdfs:subClassOf>
        <owl:disjointWith rdf:resource="http://OntoCAPE/chemical_process_system/CPS_function/process.owl#TemperatureChange"/>
        <rdfs:comment>By means of a PressureChange a heat content of a particular fluid may be exchanged which may be used for heating or cooling purposes in terms of unit operations.</rdfs:comment>
    </owl:Class>
    


    <!-- http://OntoCAPE/chemical_process_system/CPS_function/process.owl#PressureChangeOfGas -->

    <owl:Class rdf:about="http://OntoCAPE/chemical_process_system/CPS_function/process.owl#PressureChangeOfGas">
        <rdfs:subClassOf rdf:resource="http://OntoCAPE/chemical_process_system/CPS_function/process.owl#PressureChange"/>
        <owl:disjointWith rdf:resource="http://OntoCAPE/chemical_process_system/CPS_function/process.owl#PressureChangeOfLiquid"/>
    </owl:Class>
    


    <!-- http://OntoCAPE/chemical_process_system/CPS_function/process.owl#PressureChangeOfLiquid -->

    <owl:Class rdf:about="http://OntoCAPE/chemical_process_system/CPS_function/process.owl#PressureChangeOfLiquid">
        <rdfs:subClassOf rdf:resource="http://OntoCAPE/chemical_process_system/CPS_function/process.owl#PressureChange"/>
    </owl:Class>
    


    <!-- http://OntoCAPE/chemical_process_system/CPS_function/process.owl#PressureDifference -->

    <owl:Class rdf:about="http://OntoCAPE/chemical_process_system/CPS_function/process.owl#PressureDifference">
        <rdfs:subClassOf rdf:resource="http://OntoCAPE/chemical_process_system/CPS_function/process.owl#ProcessStepProperty"/>
        <rdfs:subClassOf>
            <owl:Restriction>
                <owl:onProperty rdf:resource="http://OntoCAPE/upper_level/system.owl#hasDimension"/>
                <owl:hasValue rdf:resource="http://OntoCAPE/supporting_concepts/physical_dimension/derived_dimensions.owl#pressure"/>
            </owl:Restriction>
        </rdfs:subClassOf>
    </owl:Class>
    


    <!-- http://OntoCAPE/chemical_process_system/CPS_function/process.owl#Process -->

    <owl:Class rdf:about="http://OntoCAPE/chemical_process_system/CPS_function/process.owl#Process">
        <owl:equivalentClass>
            <owl:Class>
                <owl:intersectionOf rdf:parseType="Collection">
                    <rdf:Description rdf:about="http://OntoCAPE/chemical_process_system/CPS_function/process.owl#AggregatedProcessStep"/>
                    <owl:Class>
                        <owl:complementOf>
                            <owl:Restriction>
                                <owl:onProperty rdf:resource="http://OntoCAPE/upper_level/system.owl#isSubsystemOf"/>
                                <owl:someValuesFrom rdf:resource="http://OntoCAPE/chemical_process_system/CPS_function/process.owl#ProcessStep"/>
                            </owl:Restriction>
                        </owl:complementOf>
                    </owl:Class>
                </owl:intersectionOf>
            </owl:Class>
        </owl:equivalentClass>
        <rdfs:comment>An AggregatedProcessStep representing the entire function of the Process considered</rdfs:comment>
    </owl:Class>
    


    <!-- http://OntoCAPE/chemical_process_system/CPS_function/process.owl#ProcessState -->

    <owl:Class rdf:about="http://OntoCAPE/chemical_process_system/CPS_function/process.owl#ProcessState">
        <rdfs:subClassOf rdf:resource="http://OntoCAPE/upper_level/network_system.owl#DirectedConnection"/>
        <rdfs:subClassOf>
            <owl:Restriction>
                <owl:onProperty rdf:resource="http://OntoCAPE/upper_level/network_system.owl#enters"/>
                <owl:allValuesFrom rdf:resource="http://OntoCAPE/chemical_process_system/CPS_function/process.owl#ProcessStep"/>
            </owl:Restriction>
        </rdfs:subClassOf>
        <rdfs:subClassOf>
            <owl:Restriction>
                <owl:onProperty rdf:resource="http://OntoCAPE/upper_level/network_system.owl#leaves"/>
                <owl:allValuesFrom rdf:resource="http://OntoCAPE/chemical_process_system/CPS_function/process.owl#ProcessStep"/>
            </owl:Restriction>
        </rdfs:subClassOf>
        <rdfs:subClassOf>
            <owl:Restriction>
                <owl:onProperty rdf:resource="http://OntoCAPE/upper_level/system.owl#hasDirectSubsystem"/>
                <owl:allValuesFrom>
                    <owl:Class>
                        <owl:unionOf rdf:parseType="Collection">
                            <rdf:Description rdf:about="http://OntoCAPE/chemical_process_system/CPS_function/process.owl#ProcessState"/>
                            <rdf:Description rdf:about="http://OntoCAPE/chemical_process_system/CPS_function/process.owl#ProcessStep"/>
                        </owl:unionOf>
                    </owl:Class>
                </owl:allValuesFrom>
            </owl:Restriction>
        </rdfs:subClassOf>
        <rdfs:subClassOf>
            <owl:Restriction>
                <owl:onProperty rdf:resource="http://OntoCAPE/upper_level/system.owl#isDirectSubsystemOf"/>
                <owl:allValuesFrom>
                    <owl:Class>
                        <owl:unionOf rdf:parseType="Collection">
                            <rdf:Description rdf:about="http://OntoCAPE/chemical_process_system/CPS_function/process.owl#ProcessState"/>
                            <rdf:Description rdf:about="http://OntoCAPE/chemical_process_system/CPS_function/process.owl#ProcessStep"/>
                        </owl:unionOf>
                    </owl:Class>
                </owl:allValuesFrom>
            </owl:Restriction>
        </rdfs:subClassOf>
        <rdfs:comment>A ProcessState represents the collectivity of properties of a CertainMaterialAmount  which is produced in the associating process step.</rdfs:comment>
    </owl:Class>
    


    <!-- http://OntoCAPE/chemical_process_system/CPS_function/process.owl#ProcessStep -->

    <owl:Class rdf:about="http://OntoCAPE/chemical_process_system/CPS_function/process.owl#ProcessStep">
        <rdfs:subClassOf rdf:resource="http://OntoCAPE/upper_level/network_system.owl#Device"/>
        <rdfs:subClassOf>
            <owl:Restriction>
                <owl:onProperty rdf:resource="http://OntoCAPE/upper_level/network_system.owl#hasInput"/>
                <owl:someValuesFrom rdf:resource="http://OntoCAPE/chemical_process_system/CPS_function/process.owl#ProcessState"/>
            </owl:Restriction>
        </rdfs:subClassOf>
        <rdfs:subClassOf>
            <owl:Restriction>
                <owl:onProperty rdf:resource="http://OntoCAPE/upper_level/network_system.owl#hasOutput"/>
                <owl:someValuesFrom rdf:resource="http://OntoCAPE/chemical_process_system/CPS_function/process.owl#ProcessState"/>
            </owl:Restriction>
        </rdfs:subClassOf>
        <rdfs:subClassOf>
            <owl:Restriction>
                <owl:onProperty rdf:resource="http://OntoCAPE/upper_level/network_system.owl#hasInput"/>
                <owl:allValuesFrom rdf:resource="http://OntoCAPE/chemical_process_system/CPS_function/process.owl#ProcessState"/>
            </owl:Restriction>
        </rdfs:subClassOf>
        <rdfs:subClassOf>
            <owl:Restriction>
                <owl:onProperty rdf:resource="http://OntoCAPE/upper_level/network_system.owl#hasOutput"/>
                <owl:allValuesFrom rdf:resource="http://OntoCAPE/chemical_process_system/CPS_function/process.owl#ProcessState"/>
            </owl:Restriction>
        </rdfs:subClassOf>
        <rdfs:subClassOf>
            <owl:Restriction>
                <owl:onProperty rdf:resource="http://OntoCAPE/upper_level/system.owl#hasDirectSubsystem"/>
                <owl:allValuesFrom>
                    <owl:Class>
                        <owl:unionOf rdf:parseType="Collection">
                            <rdf:Description rdf:about="http://OntoCAPE/chemical_process_system/CPS_function/process.owl#ProcessState"/>
                            <rdf:Description rdf:about="http://OntoCAPE/chemical_process_system/CPS_function/process.owl#ProcessStep"/>
                        </owl:unionOf>
                    </owl:Class>
                </owl:allValuesFrom>
            </owl:Restriction>
        </rdfs:subClassOf>
        <rdfs:subClassOf>
            <owl:Restriction>
                <owl:onProperty rdf:resource="http://OntoCAPE/upper_level/system.owl#isDirectSubsystemOf"/>
                <owl:allValuesFrom>
                    <owl:Class>
                        <owl:unionOf rdf:parseType="Collection">
                            <rdf:Description rdf:about="http://OntoCAPE/chemical_process_system/CPS_function/process.owl#ProcessState"/>
                            <rdf:Description rdf:about="http://OntoCAPE/chemical_process_system/CPS_function/process.owl#ProcessStep"/>
                        </owl:unionOf>
                    </owl:Class>
                </owl:allValuesFrom>
            </owl:Restriction>
        </rdfs:subClassOf>
        <rdfs:comment>A ProcessStep is a certain material processing procedure.</rdfs:comment>
    </owl:Class>
    


    <!-- http://OntoCAPE/chemical_process_system/CPS_function/process.owl#ProcessStepProperty -->

    <owl:Class rdf:about="http://OntoCAPE/chemical_process_system/CPS_function/process.owl#ProcessStepProperty">
        <rdfs:subClassOf rdf:resource="http://OntoCAPE/upper_level/system.owl#ScalarQuantity"/>
    </owl:Class>
    


    <!-- http://OntoCAPE/chemical_process_system/CPS_function/process.owl#ProcessStream -->

    <owl:Class rdf:about="http://OntoCAPE/chemical_process_system/CPS_function/process.owl#ProcessStream">
        <owl:equivalentClass>
            <owl:Class>
                <owl:intersectionOf rdf:parseType="Collection">
                    <rdf:Description rdf:about="http://OntoCAPE/chemical_process_system/CPS_function/process.owl#ProcessState"/>
                    <owl:Restriction>
                        <owl:onProperty rdf:resource="http://OntoCAPE/chemical_process_system/CPS_function/process.owl#hasOperationMode"/>
                        <owl:hasValue rdf:resource="http://OntoCAPE/chemical_process_system/CPS_function/process.owl#Continuous"/>
                    </owl:Restriction>
                </owl:intersectionOf>
            </owl:Class>
        </owl:equivalentClass>
        <rdfs:comment>A ProcessStream indicated the continuous mode of operation applied to the Process.</rdfs:comment>
    </owl:Class>
    


    <!-- http://OntoCAPE/chemical_process_system/CPS_function/process.owl#RawMaterial -->

    <owl:Class rdf:about="http://OntoCAPE/chemical_process_system/CPS_function/process.owl#RawMaterial">
        <rdfs:subClassOf rdf:resource="http://OntoCAPE/chemical_process_system/CPS_function/process.owl#ProcessState"/>
        <rdfs:subClassOf>
            <owl:Restriction>
                <owl:onProperty rdf:resource="http://OntoCAPE/upper_level/network_system.owl#enters"/>
                <owl:someValuesFrom rdf:resource="http://OntoCAPE/chemical_process_system/CPS_function/process.owl#ProcessStep"/>
            </owl:Restriction>
        </rdfs:subClassOf>
        <rdfs:subClassOf>
            <owl:Restriction>
                <owl:onProperty rdf:resource="http://OntoCAPE/upper_level/network_system.owl#leaves"/>
                <owl:cardinality rdf:datatype="http://www.w3.org/2001/XMLSchema#nonNegativeInteger">0</owl:cardinality>
            </owl:Restriction>
        </rdfs:subClassOf>
        <rdfs:comment>A RawMaterial is a Material that enters a ProcessStep.</rdfs:comment>
    </owl:Class>
    


    <!-- http://OntoCAPE/chemical_process_system/CPS_function/process.owl#Reaction -->

    <owl:Class rdf:about="http://OntoCAPE/chemical_process_system/CPS_function/process.owl#Reaction">
        <rdfs:subClassOf rdf:resource="http://OntoCAPE/chemical_process_system/CPS_function/process.owl#ProcessStep"/>
        <rdfs:subClassOf>
            <owl:Restriction>
                <owl:onProperty rdf:resource="http://OntoCAPE/chemical_process_system/CPS_function/process.owl#hasChemicalReactionNetwork"/>
                <owl:someValuesFrom rdf:resource="http://OntoCAPE/material/phase_system/phase_system.owl#ReactionNetwork"/>
            </owl:Restriction>
        </rdfs:subClassOf>
        <rdfs:subClassOf>
            <owl:Restriction>
                <owl:onProperty rdf:resource="http://OntoCAPE/upper_level/system.owl#hasProperty"/>
                <owl:someValuesFrom rdf:resource="http://OntoCAPE/chemical_process_system/CPS_function/process.owl#KeyChemicalComponentConversionRatio"/>
            </owl:Restriction>
        </rdfs:subClassOf>
        <rdfs:subClassOf>
            <owl:Restriction>
                <owl:onProperty rdf:resource="http://OntoCAPE/chemical_process_system/CPS_function/process.owl#hasChemicalReactionNetwork"/>
                <owl:allValuesFrom rdf:resource="http://OntoCAPE/material/phase_system/phase_system.owl#ReactionNetwork"/>
            </owl:Restriction>
        </rdfs:subClassOf>
        <rdfs:subClassOf>
            <owl:Restriction>
                <owl:onProperty rdf:resource="http://OntoCAPE/chemical_process_system/CPS_function/process.owl#hasChemicalReactionNetwork"/>
                <owl:cardinality rdf:datatype="http://www.w3.org/2001/XMLSchema#nonNegativeInteger">1</owl:cardinality>
            </owl:Restriction>
        </rdfs:subClassOf>
        <owl:disjointWith rdf:resource="http://OntoCAPE/chemical_process_system/CPS_function/process.owl#UnitOperation"/>
        <rdfs:comment>A Reaction is a ProcessStep in which some material is converted to some other material through chemical or biochemical reactions</rdfs:comment>
    </owl:Class>
    


    <!-- http://OntoCAPE/chemical_process_system/CPS_function/process.owl#ReusableWasteProduct -->

    <owl:Class rdf:about="http://OntoCAPE/chemical_process_system/CPS_function/process.owl#ReusableWasteProduct">
        <rdfs:subClassOf rdf:resource="http://OntoCAPE/chemical_process_system/CPS_function/process.owl#WasteProduct"/>
        <rdfs:comment>A ReusableWasteProduct is a WasteProduct that can be reused for production.</rdfs:comment>
    </owl:Class>
    


    <!-- http://OntoCAPE/chemical_process_system/CPS_function/process.owl#Separation -->

    <owl:Class rdf:about="http://OntoCAPE/chemical_process_system/CPS_function/process.owl#Separation">
        <rdfs:subClassOf rdf:resource="http://OntoCAPE/chemical_process_system/CPS_function/process.owl#UnitOperation"/>
        <rdfs:subClassOf>
            <owl:Restriction>
                <owl:onProperty rdf:resource="http://OntoCAPE/upper_level/network_system.owl#hasOutput"/>
                <owl:minCardinality rdf:datatype="http://www.w3.org/2001/XMLSchema#nonNegativeInteger">2</owl:minCardinality>
            </owl:Restriction>
        </rdfs:subClassOf>
        <rdfs:comment>Separation in terms of unit operation means to achieve single components of a mixture by means of physical of chemical phenomenon.</rdfs:comment>
    </owl:Class>
    


    <!-- http://OntoCAPE/chemical_process_system/CPS_function/process.owl#Splitting -->

    <owl:Class rdf:about="http://OntoCAPE/chemical_process_system/CPS_function/process.owl#Splitting">
        <rdfs:subClassOf rdf:resource="http://OntoCAPE/chemical_process_system/CPS_function/process.owl#Fragmentation"/>
    </owl:Class>
    


    <!-- http://OntoCAPE/chemical_process_system/CPS_function/process.owl#TemperatureChange -->

    <owl:Class rdf:about="http://OntoCAPE/chemical_process_system/CPS_function/process.owl#TemperatureChange">
        <rdfs:subClassOf rdf:resource="http://OntoCAPE/chemical_process_system/CPS_function/process.owl#EnthalpyChange"/>
        <rdfs:comment>TemperatureChange in terms of unit operation means to transport the heat content of one material to another and it is applied for heating or cooling purposes.</rdfs:comment>
    </owl:Class>
    


    <!-- http://OntoCAPE/chemical_process_system/CPS_function/process.owl#UnitOperation -->

    <owl:Class rdf:about="http://OntoCAPE/chemical_process_system/CPS_function/process.owl#UnitOperation">
        <rdfs:subClassOf rdf:resource="http://OntoCAPE/chemical_process_system/CPS_function/process.owl#ProcessStep"/>
        <rdfs:comment>A UnitOperation is a basic step in a process. This basic step might comprise mixing, separation, enthalpy change and many more to achieve the desired product.</rdfs:comment>
    </owl:Class>
    


    <!-- http://OntoCAPE/chemical_process_system/CPS_function/process.owl#WasteProduct -->

    <owl:Class rdf:about="http://OntoCAPE/chemical_process_system/CPS_function/process.owl#WasteProduct">
        <rdfs:subClassOf rdf:resource="http://OntoCAPE/chemical_process_system/CPS_function/process.owl#OutputProduct"/>
        <rdfs:comment>A WasteProduct is an OutputProduct that has no value.</rdfs:comment>
    </owl:Class>
    


    <!-- http://OntoCAPE/material/phase_system/phase_system.owl#ReactionNetwork -->

    <owl:Class rdf:about="http://OntoCAPE/material/phase_system/phase_system.owl#ReactionNetwork"/>
    


    <!-- http://OntoCAPE/meta_model/fundamental_concepts/fundamental_concepts.owl#ValueSet -->

    <owl:Class rdf:about="http://OntoCAPE/meta_model/fundamental_concepts/fundamental_concepts.owl#ValueSet"/>
    


    <!-- http://OntoCAPE/upper_level/network_system.owl#Connection -->

    <owl:Class rdf:about="http://OntoCAPE/upper_level/network_system.owl#Connection">
        <rdfs:subClassOf rdf:resource="http://OntoCAPE/upper_level/system.owl#System"/>
        <rdfs:subClassOf>
            <owl:Restriction>
                <owl:onProperty rdf:resource="http://OntoCAPE/upper_level/system.owl#hasDirectSubsystem"/>
                <owl:allValuesFrom>
                    <owl:Class>
                        <owl:unionOf rdf:parseType="Collection">
                            <rdf:Description rdf:about="http://OntoCAPE/upper_level/network_system.owl#Connection"/>
                            <rdf:Description rdf:about="http://OntoCAPE/upper_level/network_system.owl#ConnectionPoint"/>
                            <rdf:Description rdf:about="http://OntoCAPE/upper_level/network_system.owl#Device"/>
                        </owl:unionOf>
                    </owl:Class>
                </owl:allValuesFrom>
            </owl:Restriction>
        </rdfs:subClassOf>
        <rdfs:subClassOf>
            <owl:Restriction>
                <owl:onProperty rdf:resource="http://OntoCAPE/upper_level/system.owl#hasSubsystem"/>
                <owl:allValuesFrom>
                    <owl:Class>
                        <owl:unionOf rdf:parseType="Collection">
                            <rdf:Description rdf:about="http://OntoCAPE/upper_level/network_system.owl#Connection"/>
                            <rdf:Description rdf:about="http://OntoCAPE/upper_level/network_system.owl#ConnectionPoint"/>
                            <rdf:Description rdf:about="http://OntoCAPE/upper_level/network_system.owl#Device"/>
                            <rdf:Description rdf:about="http://OntoCAPE/upper_level/network_system.owl#Port"/>
                        </owl:unionOf>
                    </owl:Class>
                </owl:allValuesFrom>
            </owl:Restriction>
        </rdfs:subClassOf>
        <rdfs:subClassOf>
            <owl:Restriction>
                <owl:onProperty rdf:resource="http://OntoCAPE/upper_level/system.owl#isDirectSubsystemOf"/>
                <owl:allValuesFrom>
                    <owl:Class>
                        <owl:unionOf rdf:parseType="Collection">
                            <rdf:Description rdf:about="http://OntoCAPE/upper_level/network_system.owl#Connection"/>
                            <rdf:Description rdf:about="http://OntoCAPE/upper_level/network_system.owl#Device"/>
                        </owl:unionOf>
                    </owl:Class>
                </owl:allValuesFrom>
            </owl:Restriction>
        </rdfs:subClassOf>
        <rdfs:subClassOf>
            <owl:Restriction>
                <owl:onProperty rdf:resource="http://OntoCAPE/upper_level/system.owl#isDirectlyConnectedTo"/>
                <owl:allValuesFrom rdf:resource="http://OntoCAPE/upper_level/network_system.owl#Device"/>
            </owl:Restriction>
        </rdfs:subClassOf>
        <rdfs:subClassOf>
            <owl:Restriction>
                <owl:onProperty rdf:resource="http://OntoCAPE/upper_level/system.owl#isDirectlyConnectedTo"/>
                <owl:maxCardinality rdf:datatype="http://www.w3.org/2001/XMLSchema#nonNegativeInteger">2</owl:maxCardinality>
            </owl:Restriction>
        </rdfs:subClassOf>
        <owl:disjointWith rdf:resource="http://OntoCAPE/upper_level/network_system.owl#Device"/>
        <rdfs:comment>Connections are those elements of a NetworkSystem that represent the linkages between the Devices.</rdfs:comment>
    </owl:Class>
    


    <!-- http://OntoCAPE/upper_level/network_system.owl#ConnectionPoint -->

    <owl:Class rdf:about="http://OntoCAPE/upper_level/network_system.owl#ConnectionPoint">
        <rdfs:subClassOf rdf:resource="http://OntoCAPE/upper_level/system.owl#SystemInterface"/>
        <rdfs:subClassOf>
            <owl:Restriction>
                <owl:onProperty rdf:resource="http://OntoCAPE/upper_level/system.owl#isSubsystemOf"/>
                <owl:someValuesFrom rdf:resource="http://OntoCAPE/upper_level/network_system.owl#Connection"/>
            </owl:Restriction>
        </rdfs:subClassOf>
        <rdfs:subClassOf>
            <owl:Restriction>
                <owl:onProperty rdf:resource="http://OntoCAPE/upper_level/system.owl#isDirectSubsystemOf"/>
                <owl:allValuesFrom rdf:resource="http://OntoCAPE/upper_level/network_system.owl#Connection"/>
            </owl:Restriction>
        </rdfs:subClassOf>
        <rdfs:subClassOf>
            <owl:Restriction>
                <owl:onProperty rdf:resource="http://OntoCAPE/upper_level/system.owl#isDirectlyConnectedTo"/>
                <owl:allValuesFrom rdf:resource="http://OntoCAPE/upper_level/network_system.owl#Port"/>
            </owl:Restriction>
        </rdfs:subClassOf>
        <rdfs:subClassOf>
            <owl:Restriction>
                <owl:onProperty rdf:resource="http://OntoCAPE/upper_level/system.owl#isDirectlyConnectedTo"/>
                <owl:maxCardinality rdf:datatype="http://www.w3.org/2001/XMLSchema#nonNegativeInteger">1</owl:maxCardinality>
            </owl:Restriction>
        </rdfs:subClassOf>
        <owl:disjointWith rdf:resource="http://OntoCAPE/upper_level/network_system.owl#Port"/>
        <rdfs:comment>A ConnectionPoint represents the interface through which a Connection can be connected to the Port of a device. ConnectionPoints may have certain attributes that further specify the type of connection. ConnectionPoints are subsystems of the corresponding Connection or DirectedConnection, respectively.</rdfs:comment>
    </owl:Class>
    


    <!-- http://OntoCAPE/upper_level/network_system.owl#Device -->

    <owl:Class rdf:about="http://OntoCAPE/upper_level/network_system.owl#Device">
        <rdfs:subClassOf rdf:resource="http://OntoCAPE/upper_level/system.owl#System"/>
        <rdfs:subClassOf>
            <owl:Restriction>
                <owl:onProperty rdf:resource="http://OntoCAPE/upper_level/network_system.owl#hasInput"/>
                <owl:allValuesFrom rdf:resource="http://OntoCAPE/upper_level/network_system.owl#DirectedConnection"/>
            </owl:Restriction>
        </rdfs:subClassOf>
        <rdfs:subClassOf>
            <owl:Restriction>
                <owl:onProperty rdf:resource="http://OntoCAPE/upper_level/network_system.owl#hasOutput"/>
                <owl:allValuesFrom rdf:resource="http://OntoCAPE/upper_level/network_system.owl#DirectedConnection"/>
            </owl:Restriction>
        </rdfs:subClassOf>
        <rdfs:subClassOf>
            <owl:Restriction>
                <owl:onProperty rdf:resource="http://OntoCAPE/upper_level/system.owl#hasDirectSubsystem"/>
                <owl:allValuesFrom>
                    <owl:Class>
                        <owl:unionOf rdf:parseType="Collection">
                            <rdf:Description rdf:about="http://OntoCAPE/upper_level/network_system.owl#Connection"/>
                            <rdf:Description rdf:about="http://OntoCAPE/upper_level/network_system.owl#Device"/>
                            <rdf:Description rdf:about="http://OntoCAPE/upper_level/network_system.owl#Port"/>
                        </owl:unionOf>
                    </owl:Class>
                </owl:allValuesFrom>
            </owl:Restriction>
        </rdfs:subClassOf>
        <rdfs:subClassOf>
            <owl:Restriction>
                <owl:onProperty rdf:resource="http://OntoCAPE/upper_level/system.owl#hasSubsystem"/>
                <owl:allValuesFrom>
                    <owl:Class>
                        <owl:unionOf rdf:parseType="Collection">
                            <rdf:Description rdf:about="http://OntoCAPE/upper_level/network_system.owl#Connection"/>
                            <rdf:Description rdf:about="http://OntoCAPE/upper_level/network_system.owl#ConnectionPoint"/>
                            <rdf:Description rdf:about="http://OntoCAPE/upper_level/network_system.owl#Device"/>
                            <rdf:Description rdf:about="http://OntoCAPE/upper_level/network_system.owl#Port"/>
                        </owl:unionOf>
                    </owl:Class>
                </owl:allValuesFrom>
            </owl:Restriction>
        </rdfs:subClassOf>
        <rdfs:subClassOf>
            <owl:Restriction>
                <owl:onProperty rdf:resource="http://OntoCAPE/upper_level/system.owl#isDirectSubsystemOf"/>
                <owl:allValuesFrom>
                    <owl:Class>
                        <owl:unionOf rdf:parseType="Collection">
                            <rdf:Description rdf:about="http://OntoCAPE/upper_level/network_system.owl#Connection"/>
                            <rdf:Description rdf:about="http://OntoCAPE/upper_level/network_system.owl#Device"/>
                        </owl:unionOf>
                    </owl:Class>
                </owl:allValuesFrom>
            </owl:Restriction>
        </rdfs:subClassOf>
        <rdfs:subClassOf>
            <owl:Restriction>
                <owl:onProperty rdf:resource="http://OntoCAPE/upper_level/system.owl#isDirectlyConnectedTo"/>
                <owl:allValuesFrom rdf:resource="http://OntoCAPE/upper_level/network_system.owl#Connection"/>
            </owl:Restriction>
        </rdfs:subClassOf>
        <rdfs:comment>Devices are the crucial elements of a NetworkSystem, holding the major functionality.</rdfs:comment>
    </owl:Class>
    


    <!-- http://OntoCAPE/upper_level/network_system.owl#DirectedConnection -->

    <owl:Class rdf:about="http://OntoCAPE/upper_level/network_system.owl#DirectedConnection">
        <rdfs:subClassOf rdf:resource="http://OntoCAPE/upper_level/network_system.owl#Connection"/>
        <rdfs:subClassOf>
            <owl:Restriction>
                <owl:onProperty rdf:resource="http://OntoCAPE/upper_level/network_system.owl#enters"/>
                <owl:allValuesFrom rdf:resource="http://OntoCAPE/upper_level/network_system.owl#Device"/>
            </owl:Restriction>
        </rdfs:subClassOf>
        <rdfs:subClassOf>
            <owl:Restriction>
                <owl:onProperty rdf:resource="http://OntoCAPE/upper_level/network_system.owl#leaves"/>
                <owl:allValuesFrom rdf:resource="http://OntoCAPE/upper_level/network_system.owl#Device"/>
            </owl:Restriction>
        </rdfs:subClassOf>
        <rdfs:subClassOf>
            <owl:Restriction>
                <owl:onProperty rdf:resource="http://OntoCAPE/upper_level/system.owl#isDirectlyConnectedTo"/>
                <owl:cardinality rdf:datatype="http://www.w3.org/2001/XMLSchema#nonNegativeInteger">0</owl:cardinality>
            </owl:Restriction>
        </rdfs:subClassOf>
        <rdfs:subClassOf>
            <owl:Restriction>
                <owl:onProperty rdf:resource="http://OntoCAPE/upper_level/network_system.owl#enters"/>
                <owl:maxCardinality rdf:datatype="http://www.w3.org/2001/XMLSchema#nonNegativeInteger">1</owl:maxCardinality>
            </owl:Restriction>
        </rdfs:subClassOf>
        <rdfs:subClassOf>
            <owl:Restriction>
                <owl:onProperty rdf:resource="http://OntoCAPE/upper_level/network_system.owl#leaves"/>
                <owl:maxCardinality rdf:datatype="http://www.w3.org/2001/XMLSchema#nonNegativeInteger">1</owl:maxCardinality>
            </owl:Restriction>
        </rdfs:subClassOf>
        <rdfs:comment>DirectedConnection is a specialization of Connection and represents likewise the connecting element between Devices. However, the usage of DirectedConnection implies the indication of a directed interconnection.</rdfs:comment>
    </owl:Class>
    


    <!-- http://OntoCAPE/upper_level/network_system.owl#EnvironmentConnection -->

    <owl:Class rdf:about="http://OntoCAPE/upper_level/network_system.owl#EnvironmentConnection">
        <owl:equivalentClass>
            <owl:Class>
                <owl:intersectionOf rdf:parseType="Collection">
                    <rdf:Description rdf:about="http://OntoCAPE/upper_level/network_system.owl#Connection"/>
                    <owl:Restriction>
                        <owl:onProperty rdf:resource="http://OntoCAPE/upper_level/system.owl#isDirectlyConnectedTo"/>
                        <owl:someValuesFrom rdf:resource="http://OntoCAPE/upper_level/network_system.owl#Device"/>
                    </owl:Restriction>
                    <owl:Restriction>
                        <owl:onProperty rdf:resource="http://OntoCAPE/upper_level/system.owl#isDirectlyConnectedTo"/>
                        <owl:cardinality rdf:datatype="http://www.w3.org/2001/XMLSchema#nonNegativeInteger">1</owl:cardinality>
                    </owl:Restriction>
                </owl:intersectionOf>
            </owl:Class>
        </owl:equivalentClass>
        <rdfs:subClassOf>
            <owl:Restriction>
                <owl:onProperty rdf:resource="http://OntoCAPE/upper_level/system.owl#hasDirectSubsystem"/>
                <owl:cardinality rdf:datatype="http://www.w3.org/2001/XMLSchema#nonNegativeInteger">0</owl:cardinality>
            </owl:Restriction>
        </rdfs:subClassOf>
        <rdfs:subClassOf>
            <owl:Restriction>
                <owl:onProperty rdf:resource="http://OntoCAPE/upper_level/system.owl#isDirectSubsystemOf"/>
                <owl:cardinality rdf:datatype="http://www.w3.org/2001/XMLSchema#nonNegativeInteger">0</owl:cardinality>
            </owl:Restriction>
        </rdfs:subClassOf>
    </owl:Class>
    


    <!-- http://OntoCAPE/upper_level/network_system.owl#NetworkSystem -->

    <owl:Class rdf:about="http://OntoCAPE/upper_level/network_system.owl#NetworkSystem">
        <owl:equivalentClass>
            <owl:Class>
                <owl:intersectionOf rdf:parseType="Collection">
                    <rdf:Description rdf:about="http://OntoCAPE/upper_level/system.owl#CompositeSystem"/>
                    <owl:Restriction>
                        <owl:onProperty rdf:resource="http://OntoCAPE/upper_level/system.owl#isComposedOfSubsystem"/>
                        <owl:someValuesFrom rdf:resource="http://OntoCAPE/upper_level/network_system.owl#Connection"/>
                    </owl:Restriction>
                    <owl:Restriction>
                        <owl:onProperty rdf:resource="http://OntoCAPE/upper_level/system.owl#isComposedOfSubsystem"/>
                        <owl:someValuesFrom rdf:resource="http://OntoCAPE/upper_level/network_system.owl#Device"/>
                    </owl:Restriction>
                </owl:intersectionOf>
            </owl:Class>
        </owl:equivalentClass>
        <rdfs:subClassOf>
            <owl:Class>
                <owl:unionOf rdf:parseType="Collection">
                    <rdf:Description rdf:about="http://OntoCAPE/upper_level/network_system.owl#Connection"/>
                    <rdf:Description rdf:about="http://OntoCAPE/upper_level/network_system.owl#Device"/>
                </owl:unionOf>
            </owl:Class>
        </rdfs:subClassOf>
        <rdfs:subClassOf>
            <owl:Restriction>
                <owl:onProperty rdf:resource="http://OntoCAPE/upper_level/system.owl#isComposedOfSubsystem"/>
                <owl:allValuesFrom>
                    <owl:Class>
                        <owl:unionOf rdf:parseType="Collection">
                            <rdf:Description rdf:about="http://OntoCAPE/upper_level/network_system.owl#Connection"/>
                            <rdf:Description rdf:about="http://OntoCAPE/upper_level/network_system.owl#Device"/>
                        </owl:unionOf>
                    </owl:Class>
                </owl:allValuesFrom>
            </owl:Restriction>
        </rdfs:subClassOf>
        <rdfs:comment>A NetworkSystem is a system that is composed of some Connections and some Devices.</rdfs:comment>
    </owl:Class>
    


    <!-- http://OntoCAPE/upper_level/network_system.owl#Port -->

    <owl:Class rdf:about="http://OntoCAPE/upper_level/network_system.owl#Port">
        <rdfs:subClassOf rdf:resource="http://OntoCAPE/upper_level/system.owl#SystemInterface"/>
        <rdfs:subClassOf>
            <owl:Restriction>
                <owl:onProperty rdf:resource="http://OntoCAPE/upper_level/system.owl#isSubsystemOf"/>
                <owl:someValuesFrom rdf:resource="http://OntoCAPE/upper_level/network_system.owl#Device"/>
            </owl:Restriction>
        </rdfs:subClassOf>
        <rdfs:subClassOf>
            <owl:Restriction>
                <owl:onProperty rdf:resource="http://OntoCAPE/upper_level/system.owl#isDirectSubsystemOf"/>
                <owl:allValuesFrom rdf:resource="http://OntoCAPE/upper_level/network_system.owl#Device"/>
            </owl:Restriction>
        </rdfs:subClassOf>
        <rdfs:subClassOf>
            <owl:Restriction>
                <owl:onProperty rdf:resource="http://OntoCAPE/upper_level/system.owl#isDirectlyConnectedTo"/>
                <owl:allValuesFrom rdf:resource="http://OntoCAPE/upper_level/network_system.owl#ConnectionPoint"/>
            </owl:Restriction>
        </rdfs:subClassOf>
        <rdfs:subClassOf>
            <owl:Restriction>
                <owl:onProperty rdf:resource="http://OntoCAPE/upper_level/system.owl#isDirectlyConnectedTo"/>
                <owl:maxCardinality rdf:datatype="http://www.w3.org/2001/XMLSchema#nonNegativeInteger">1</owl:maxCardinality>
            </owl:Restriction>
        </rdfs:subClassOf>
        <rdfs:comment>Ports represents the interfaces through which Devices are connected to Connections. A Port may have certain attributes that characterize the type of the connection.</rdfs:comment>
    </owl:Class>
    


    <!-- http://OntoCAPE/upper_level/system.owl#Aspect -->

    <owl:Class rdf:about="http://OntoCAPE/upper_level/system.owl#Aspect">
        <rdfs:subClassOf rdf:resource="http://meta_model/fundamental_concepts/fundamental_concepts.owl#NonExhaustiveValueSet"/>
        <owl:disjointWith rdf:resource="http://OntoCAPE/upper_level/system.owl#PhysicalDimension"/>
        <owl:disjointWith rdf:resource="http://OntoCAPE/upper_level/system.owl#UnitOfMeasure"/>
        <rdfs:comment>An aspect represents a particular viewpoint of a system. An instance of the aspect class explicitly denominates that viewpoint.</rdfs:comment>
    </owl:Class>
    


    <!-- http://OntoCAPE/upper_level/system.owl#AspectSystem -->

    <owl:Class rdf:about="http://OntoCAPE/upper_level/system.owl#AspectSystem">
        <owl:equivalentClass>
            <owl:Class>
                <owl:intersectionOf rdf:parseType="Collection">
                    <rdf:Description rdf:about="http://OntoCAPE/upper_level/system.owl#ExclusiveSubsystem"/>
                    <owl:Restriction>
                        <owl:onProperty rdf:resource="http://OntoCAPE/upper_level/system.owl#isConsideredUnderAspectOf"/>
                        <owl:someValuesFrom rdf:resource="http://OntoCAPE/upper_level/system.owl#Aspect"/>
                    </owl:Restriction>
                </owl:intersectionOf>
            </owl:Class>
        </owl:equivalentClass>
        <rdfs:subClassOf>
            <owl:Restriction>
                <owl:onProperty rdf:resource="http://OntoCAPE/upper_level/system.owl#representsAspectOf"/>
                <owl:someValuesFrom rdf:resource="http://OntoCAPE/upper_level/system.owl#CompositeSystem"/>
            </owl:Restriction>
        </rdfs:subClassOf>
        <rdfs:subClassOf>
            <owl:Restriction>
                <owl:onProperty rdf:resource="http://OntoCAPE/upper_level/system.owl#isConsideredUnderAspectOf"/>
                <owl:allValuesFrom rdf:resource="http://OntoCAPE/upper_level/system.owl#Aspect"/>
            </owl:Restriction>
        </rdfs:subClassOf>
        <rdfs:subClassOf>
            <owl:Restriction>
                <owl:onProperty rdf:resource="http://OntoCAPE/upper_level/system.owl#representsAspectOf"/>
                <owl:allValuesFrom rdf:resource="http://OntoCAPE/upper_level/system.owl#CompositeSystem"/>
            </owl:Restriction>
        </rdfs:subClassOf>
        <rdfs:subClassOf>
            <owl:Restriction>
                <owl:onProperty rdf:resource="http://OntoCAPE/upper_level/system.owl#isConsideredUnderAspectOf"/>
                <owl:cardinality rdf:datatype="http://www.w3.org/2001/XMLSchema#nonNegativeInteger">1</owl:cardinality>
            </owl:Restriction>
        </rdfs:subClassOf>
        <rdfs:subClassOf>
            <owl:Restriction>
                <owl:onProperty rdf:resource="http://OntoCAPE/upper_level/system.owl#representsAspectOf"/>
                <owl:cardinality rdf:datatype="http://www.w3.org/2001/XMLSchema#nonNegativeInteger">1</owl:cardinality>
            </owl:Restriction>
        </rdfs:subClassOf>
        <owl:disjointWith rdf:resource="http://OntoCAPE/upper_level/system.owl#SystemInterface"/>
        <rdfs:comment>An AspectSystem is an ExclusiveSubsystem that contains those system components, relationships, and constraints that are of relevance to a particular Aspect.</rdfs:comment>
    </owl:Class>
    


    <!-- http://OntoCAPE/upper_level/system.owl#CompositeSystem -->

    <owl:Class rdf:about="http://OntoCAPE/upper_level/system.owl#CompositeSystem">
        <owl:equivalentClass>
            <owl:Restriction>
                <owl:onProperty rdf:resource="http://OntoCAPE/upper_level/system.owl#isComposedOfSubsystem"/>
                <owl:someValuesFrom rdf:resource="http://OntoCAPE/upper_level/system.owl#System"/>
            </owl:Restriction>
        </owl:equivalentClass>
        <rdfs:subClassOf rdf:resource="http://OntoCAPE/upper_level/system.owl#Supersystem"/>
        <rdfs:subClassOf>
            <owl:Restriction>
                <owl:onProperty rdf:resource="http://OntoCAPE/upper_level/system.owl#hasAspectSystem"/>
                <owl:allValuesFrom rdf:resource="http://OntoCAPE/upper_level/system.owl#AspectSystem"/>
            </owl:Restriction>
        </rdfs:subClassOf>
        <rdfs:subClassOf>
            <owl:Restriction>
                <owl:onProperty rdf:resource="http://OntoCAPE/upper_level/system.owl#isComposedOfSubsystem"/>
                <owl:allValuesFrom rdf:resource="http://OntoCAPE/upper_level/system.owl#System"/>
            </owl:Restriction>
        </rdfs:subClassOf>
        <rdfs:comment>A CompositeSystem is a System that is composed of other Systems.</rdfs:comment>
    </owl:Class>
    


    <!-- http://OntoCAPE/upper_level/system.owl#ConstantProperty -->

    <owl:Class rdf:about="http://OntoCAPE/upper_level/system.owl#ConstantProperty">
        <owl:equivalentClass>
            <owl:Class>
                <owl:intersectionOf rdf:parseType="Collection">
                    <rdf:Description rdf:about="http://OntoCAPE/upper_level/system.owl#Property"/>
                    <owl:Restriction>
                        <owl:onProperty rdf:resource="http://OntoCAPE/upper_level/system.owl#hasValue"/>
                        <owl:cardinality rdf:datatype="http://www.w3.org/2001/XMLSchema#nonNegativeInteger">1</owl:cardinality>
                    </owl:Restriction>
                </owl:intersectionOf>
            </owl:Class>
        </owl:equivalentClass>
        <rdfs:comment>A ConstantProperty is a Property that has exactly one Value.</rdfs:comment>
    </owl:Class>
    


    <!-- http://OntoCAPE/upper_level/system.owl#ElementarySystem -->

    <owl:Class rdf:about="http://OntoCAPE/upper_level/system.owl#ElementarySystem">
        <owl:equivalentClass>
            <owl:Class>
                <owl:intersectionOf rdf:parseType="Collection">
                    <rdf:Description rdf:about="http://OntoCAPE/upper_level/system.owl#Subsystem"/>
                    <owl:Class>
                        <owl:complementOf rdf:resource="http://OntoCAPE/upper_level/system.owl#Supersystem"/>
                    </owl:Class>
                </owl:intersectionOf>
            </owl:Class>
        </owl:equivalentClass>
        <rdfs:subClassOf>
            <owl:Restriction>
                <owl:onProperty rdf:resource="http://OntoCAPE/upper_level/system.owl#isDirectlyConnectedTo"/>
                <owl:allValuesFrom rdf:resource="http://OntoCAPE/upper_level/system.owl#ElementarySystem"/>
            </owl:Restriction>
        </rdfs:subClassOf>
        <rdfs:subClassOf>
            <owl:Restriction>
                <owl:onProperty rdf:resource="http://OntoCAPE/upper_level/system.owl#hasDirectSubsystem"/>
                <owl:cardinality rdf:datatype="http://www.w3.org/2001/XMLSchema#nonNegativeInteger">0</owl:cardinality>
            </owl:Restriction>
        </rdfs:subClassOf>
        <owl:disjointWith rdf:resource="http://OntoCAPE/upper_level/system.owl#Supersystem"/>
        <rdfs:comment>An ElementarySystem is a Subsystem that cannot further partitioned into Subsystems.</rdfs:comment>
    </owl:Class>
    


    <!-- http://OntoCAPE/upper_level/system.owl#ExclusiveSubsystem -->

    <owl:Class rdf:about="http://OntoCAPE/upper_level/system.owl#ExclusiveSubsystem">
        <owl:equivalentClass>
            <owl:Restriction>
                <owl:onProperty rdf:resource="http://OntoCAPE/upper_level/system.owl#isExclusivelySubsystemOf"/>
                <owl:someValuesFrom rdf:resource="http://OntoCAPE/upper_level/system.owl#System"/>
            </owl:Restriction>
        </owl:equivalentClass>
        <rdfs:subClassOf rdf:resource="http://OntoCAPE/upper_level/system.owl#Subsystem"/>
        <rdfs:subClassOf>
            <owl:Restriction>
                <owl:onProperty rdf:resource="http://OntoCAPE/upper_level/system.owl#isExclusivelySubsystemOf"/>
                <owl:allValuesFrom rdf:resource="http://OntoCAPE/upper_level/system.owl#System"/>
            </owl:Restriction>
        </rdfs:subClassOf>
        <rdfs:comment>An ExclusiveSubsystem is a direct subsystem of a CompositeSystem; it cannot be a direct subsystem of any other System.</rdfs:comment>
    </owl:Class>
    


    <!-- http://OntoCAPE/upper_level/system.owl#ExtensibleValueSet -->

    <owl:Class rdf:about="http://OntoCAPE/upper_level/system.owl#ExtensibleValueSet">
        <rdfs:subClassOf rdf:resource="http://OntoCAPE/upper_level/system.owl#ValueEnumeration"/>
        <owl:disjointWith rdf:resource="http://OntoCAPE/upper_level/system.owl#FixedValueSet"/>
        <rdfs:comment>An ExtensibleValueSet is a ValueEnumeration which, unlike a FixedValueSet, is not defined by an (exhaustive) enumeration of its instances. Thus, the number of possible values may change at run time.</rdfs:comment>
    </owl:Class>
    


    <!-- http://OntoCAPE/upper_level/system.owl#FirstLevelSubsystem -->

    <owl:Class rdf:about="http://OntoCAPE/upper_level/system.owl#FirstLevelSubsystem">
        <owl:equivalentClass>
            <owl:Restriction>
                <owl:onProperty rdf:resource="http://OntoCAPE/upper_level/system.owl#isDirectSubsystemOf"/>
                <owl:someValuesFrom rdf:resource="http://OntoCAPE/upper_level/system.owl#TopLevelSystem"/>
            </owl:Restriction>
        </owl:equivalentClass>
        <rdfs:subClassOf rdf:resource="http://OntoCAPE/upper_level/system.owl#Subsystem"/>
        <rdfs:subClassOf>
            <owl:Restriction>
                <owl:onProperty rdf:resource="http://OntoCAPE/upper_level/system.owl#isDirectlyConnectedTo"/>
                <owl:allValuesFrom rdf:resource="http://OntoCAPE/upper_level/system.owl#FirstLevelSubsystem"/>
            </owl:Restriction>
        </rdfs:subClassOf>
        <owl:disjointWith rdf:resource="http://OntoCAPE/upper_level/system.owl#SecondLevelSubsystem"/>
        <rdfs:comment>A Subsystem at the first level of decomposition.</rdfs:comment>
    </owl:Class>
    


    <!-- http://OntoCAPE/upper_level/system.owl#FixedValueSet -->

    <owl:Class rdf:about="http://OntoCAPE/upper_level/system.owl#FixedValueSet">
        <rdfs:subClassOf rdf:resource="http://OntoCAPE/upper_level/system.owl#ValueEnumeration"/>
        <rdfs:comment>A FixedValueSet is a ValueEnumeration that is defined by an exhaustive enumeration of its instances. Thus, the number of possible values is fixed.</rdfs:comment>
    </owl:Class>
    


    <!-- http://OntoCAPE/upper_level/system.owl#InternalProperties -->

    <owl:Class rdf:about="http://OntoCAPE/upper_level/system.owl#InternalProperties">
        <owl:equivalentClass>
            <owl:Class>
                <owl:intersectionOf rdf:parseType="Collection">
                    <rdf:Description rdf:about="http://OntoCAPE/upper_level/system.owl#Property"/>
                    <owl:Restriction>
                        <owl:onProperty rdf:resource="http://OntoCAPE/upper_level/system.owl#isPropertyOf"/>
                        <owl:someValuesFrom>
                            <owl:Class>
                                <owl:intersectionOf rdf:parseType="Collection">
                                    <rdf:Description rdf:about="http://OntoCAPE/upper_level/system.owl#System"/>
                                    <owl:Restriction>
                                        <owl:onProperty rdf:resource="http://OntoCAPE/upper_level/system.owl#isSubsystemOf"/>
                                        <owl:hasValue rdf:resource="http://OntoCAPE/upper_level/system.owl#S"/>
                                    </owl:Restriction>
                                </owl:intersectionOf>
                            </owl:Class>
                        </owl:someValuesFrom>
                    </owl:Restriction>
                </owl:intersectionOf>
            </owl:Class>
        </owl:equivalentClass>
        <rdfs:comment>The &apos;internal Properties&apos; of a System are the Properties of its constituent Subsystems. They can be specified by means of a query class and thus inferred by reasoner. Such a query class must be defined individually for each System instance. The query class InternalProperties exemplarily demonstrates this approach for a sample System S.</rdfs:comment>
    </owl:Class>
    


    <!-- http://OntoCAPE/upper_level/system.owl#Model -->

    <owl:Class rdf:about="http://OntoCAPE/upper_level/system.owl#Model">
        <owl:equivalentClass>
            <owl:Class>
                <owl:intersectionOf rdf:parseType="Collection">
                    <rdf:Description rdf:about="http://OntoCAPE/upper_level/system.owl#System"/>
                    <owl:Restriction>
                        <owl:onProperty rdf:resource="http://OntoCAPE/upper_level/system.owl#models"/>
                        <owl:someValuesFrom rdf:resource="http://OntoCAPE/upper_level/system.owl#System"/>
                    </owl:Restriction>
                </owl:intersectionOf>
            </owl:Class>
        </owl:equivalentClass>
        <rdfs:subClassOf>
            <owl:Restriction>
                <owl:onProperty rdf:resource="http://OntoCAPE/upper_level/system.owl#models"/>
                <owl:allValuesFrom rdf:resource="http://OntoCAPE/upper_level/system.owl#System"/>
            </owl:Restriction>
        </rdfs:subClassOf>
        <rdfs:comment>A Model is a system that is used to enable the understanding of or the command over the original system, or to replace the original system. Model system and original system share certain characteristics that are of relevance to the task at hand (Wsteneck, 1963).</rdfs:comment>
    </owl:Class>
    


    <!-- http://OntoCAPE/upper_level/system.owl#PhysicalConstant -->

    <owl:Class rdf:about="http://OntoCAPE/upper_level/system.owl#PhysicalConstant">
        <rdfs:subClassOf rdf:resource="http://OntoCAPE/upper_level/system.owl#ScalarQuantity"/>
        <rdfs:subClassOf>
            <owl:Restriction>
                <owl:onProperty rdf:resource="http://OntoCAPE/upper_level/system.owl#hasValue"/>
                <owl:someValuesFrom rdf:resource="http://OntoCAPE/upper_level/system.owl#ScalarValue"/>
            </owl:Restriction>
        </rdfs:subClassOf>
        <rdfs:subClassOf>
            <owl:Restriction>
                <owl:onProperty rdf:resource="http://OntoCAPE/upper_level/system.owl#hasValue"/>
                <owl:cardinality rdf:datatype="http://www.w3.org/2001/XMLSchema#nonNegativeInteger">1</owl:cardinality>
            </owl:Restriction>
        </rdfs:subClassOf>
        <rdfs:subClassOf>
            <owl:Restriction>
                <owl:onProperty rdf:resource="http://OntoCAPE/upper_level/system.owl#isPropertyOf"/>
                <owl:cardinality rdf:datatype="http://www.w3.org/2001/XMLSchema#nonNegativeInteger">0</owl:cardinality>
            </owl:Restriction>
        </rdfs:subClassOf>
        <rdfs:comment>A PhysicalConstant is a ScalarQuantity, the Value of which is believed to be both universal in nature and invariant over time. Examples are the elementary charge, the gravitational constant, Planck&apos;s constant, and the speed of light in the vacuum.</rdfs:comment>
    </owl:Class>
    


    <!-- http://OntoCAPE/upper_level/system.owl#PhysicalDimension -->

    <owl:Class rdf:about="http://OntoCAPE/upper_level/system.owl#PhysicalDimension">
        <rdfs:subClassOf rdf:resource="http://meta_model/fundamental_concepts/fundamental_concepts.owl#NonExhaustiveValueSet"/>
        <owl:disjointWith rdf:resource="http://OntoCAPE/upper_level/system.owl#UnitOfMeasure"/>
        <rdfs:comment>A PhysicalDimension is a characteristic associated with PhysicalQuantities and UnitsOfMeasure for purposes of organization or differentiation. Mass, length, and force are exemplary instances of PhysicalDimension.</rdfs:comment>
    </owl:Class>
    


    <!-- http://OntoCAPE/upper_level/system.owl#PhysicalQuantity -->

    <owl:Class rdf:about="http://OntoCAPE/upper_level/system.owl#PhysicalQuantity">
        <owl:equivalentClass>
            <owl:Class>
                <owl:intersectionOf rdf:parseType="Collection">
                    <rdf:Description rdf:about="http://OntoCAPE/upper_level/system.owl#Property"/>
                    <owl:Restriction>
                        <owl:onProperty rdf:resource="http://OntoCAPE/upper_level/system.owl#hasDimension"/>
                        <owl:someValuesFrom rdf:resource="http://OntoCAPE/upper_level/system.owl#PhysicalDimension"/>
                    </owl:Restriction>
                </owl:intersectionOf>
            </owl:Class>
        </owl:equivalentClass>
        <rdfs:subClassOf>
            <owl:Restriction>
                <owl:onProperty rdf:resource="http://OntoCAPE/upper_level/system.owl#hasDimension"/>
                <owl:allValuesFrom rdf:resource="http://OntoCAPE/upper_level/system.owl#PhysicalDimension"/>
            </owl:Restriction>
        </rdfs:subClassOf>
        <rdfs:subClassOf>
            <owl:Restriction>
                <owl:onProperty rdf:resource="http://OntoCAPE/upper_level/system.owl#hasValue"/>
                <owl:allValuesFrom rdf:resource="http://OntoCAPE/upper_level/system.owl#QuantitativeValue"/>
            </owl:Restriction>
        </rdfs:subClassOf>
        <rdfs:subClassOf>
            <owl:Restriction>
                <owl:onProperty rdf:resource="http://OntoCAPE/upper_level/system.owl#hasDimension"/>
                <owl:cardinality rdf:datatype="http://www.w3.org/2001/XMLSchema#nonNegativeInteger">1</owl:cardinality>
            </owl:Restriction>
        </rdfs:subClassOf>
        <rdfs:comment>A PhysicalQuantity is a Property that has quantifiable Values. The concept includes scalars as well as vectors and higher-order tensors. Moreover, it comprises both physical quantities, such as mass or velocity, and nonphysical quantities, such as amount of money or rate of inflation</rdfs:comment>
    </owl:Class>
    


    <!-- http://OntoCAPE/upper_level/system.owl#Property -->

    <owl:Class rdf:about="http://OntoCAPE/upper_level/system.owl#Property">
        <rdfs:subClassOf rdf:resource="http://meta_model/fundamental_concepts/fundamental_concepts.owl#Object"/>
        <rdfs:subClassOf>
            <owl:Restriction>
                <owl:onProperty rdf:resource="http://OntoCAPE/upper_level/system.owl#hasValue"/>
                <owl:allValuesFrom rdf:resource="http://OntoCAPE/upper_level/system.owl#Value"/>
            </owl:Restriction>
        </rdfs:subClassOf>
        <rdfs:subClassOf>
            <owl:Restriction>
                <owl:onProperty rdf:resource="http://OntoCAPE/upper_level/system.owl#isPropertyOf"/>
                <owl:allValuesFrom rdf:resource="http://OntoCAPE/upper_level/system.owl#System"/>
            </owl:Restriction>
        </rdfs:subClassOf>
        <rdfs:subClassOf>
            <owl:Restriction>
                <owl:onProperty rdf:resource="http://OntoCAPE/upper_level/system.owl#isPropertyOf"/>
                <owl:maxCardinality rdf:datatype="http://www.w3.org/2001/XMLSchema#nonNegativeInteger">1</owl:maxCardinality>
            </owl:Restriction>
        </rdfs:subClassOf>
        <owl:disjointWith rdf:resource="http://OntoCAPE/upper_level/system.owl#System"/>
        <owl:disjointWith rdf:resource="http://OntoCAPE/upper_level/system.owl#Value"/>
        <rdfs:comment>The Property class represents the individual properties (traits, qualities) of a System, which distinguish the System from others. Typical examples are Size, Color, or Weight, which are modeled as subclasses of Property.</rdfs:comment>
    </owl:Class>
    


    <!-- http://OntoCAPE/upper_level/system.owl#PropertySet -->

    <owl:Class rdf:about="http://OntoCAPE/upper_level/system.owl#PropertySet">
        <owl:equivalentClass>
            <owl:Class>
                <owl:intersectionOf rdf:parseType="Collection">
                    <rdf:Description rdf:about="http://OntoCAPE/upper_level/system.owl#Property"/>
                    <owl:Restriction>
                        <owl:onProperty rdf:resource="http://OntoCAPE/upper_level/system.owl#comprisesDirectly"/>
                        <owl:someValuesFrom rdf:resource="http://OntoCAPE/upper_level/system.owl#Property"/>
                    </owl:Restriction>
                </owl:intersectionOf>
            </owl:Class>
        </owl:equivalentClass>
        <rdfs:subClassOf>
            <owl:Restriction>
                <owl:onProperty rdf:resource="http://OntoCAPE/upper_level/system.owl#comprisesDirectly"/>
                <owl:allValuesFrom rdf:resource="http://OntoCAPE/upper_level/system.owl#Property"/>
            </owl:Restriction>
        </rdfs:subClassOf>
        <rdfs:subClassOf>
            <owl:Restriction>
                <owl:onProperty rdf:resource="http://OntoCAPE/upper_level/system.owl#hasValue"/>
                <owl:cardinality rdf:datatype="http://www.w3.org/2001/XMLSchema#nonNegativeInteger">0</owl:cardinality>
            </owl:Restriction>
        </rdfs:subClassOf>
        <owl:disjointWith>
            <owl:Restriction>
                <owl:onProperty rdf:resource="http://OntoCAPE/upper_level/system.owl#hasValue"/>
                <owl:someValuesFrom rdf:resource="http://OntoCAPE/upper_level/system.owl#Value"/>
            </owl:Restriction>
        </owl:disjointWith>
        <rdfs:comment>A Property set constitutes an (unordered) collection of Properties, which may be of different types.</rdfs:comment>
    </owl:Class>
    


    <!-- http://OntoCAPE/upper_level/system.owl#QualitativeValue -->

    <owl:Class rdf:about="http://OntoCAPE/upper_level/system.owl#QualitativeValue">
        <rdfs:subClassOf rdf:resource="http://OntoCAPE/upper_level/system.owl#Value"/>
        <rdfs:subClassOf>
            <owl:Class>
                <owl:unionOf rdf:parseType="Collection">
                    <owl:Class>
                        <owl:intersectionOf rdf:parseType="Collection">
                            <owl:Restriction>
                                <owl:onProperty rdf:resource="http://OntoCAPE/upper_level/system.owl#qualitativeValue"/>
                                <owl:cardinality rdf:datatype="http://www.w3.org/2001/XMLSchema#nonNegativeInteger">0</owl:cardinality>
                            </owl:Restriction>
                            <owl:Restriction>
                                <owl:onProperty rdf:resource="http://OntoCAPE/upper_level/system.owl#value"/>
                                <owl:cardinality rdf:datatype="http://www.w3.org/2001/XMLSchema#nonNegativeInteger">1</owl:cardinality>
                            </owl:Restriction>
                        </owl:intersectionOf>
                    </owl:Class>
                    <owl:Class>
                        <owl:intersectionOf rdf:parseType="Collection">
                            <owl:Restriction>
                                <owl:onProperty rdf:resource="http://OntoCAPE/upper_level/system.owl#qualitativeValue"/>
                                <owl:cardinality rdf:datatype="http://www.w3.org/2001/XMLSchema#nonNegativeInteger">1</owl:cardinality>
                            </owl:Restriction>
                            <owl:Restriction>
                                <owl:onProperty rdf:resource="http://OntoCAPE/upper_level/system.owl#value"/>
                                <owl:cardinality rdf:datatype="http://www.w3.org/2001/XMLSchema#nonNegativeInteger">0</owl:cardinality>
                            </owl:Restriction>
                        </owl:intersectionOf>
                    </owl:Class>
                </owl:unionOf>
            </owl:Class>
        </rdfs:subClassOf>
        <rdfs:subClassOf>
            <owl:Class>
                <owl:unionOf rdf:parseType="Collection">
                    <owl:Restriction>
                        <owl:onProperty rdf:resource="http://OntoCAPE/upper_level/system.owl#qualitativeValue"/>
                        <owl:someValuesFrom rdf:resource="http://OntoCAPE/upper_level/system.owl#ValueEnumeration"/>
                    </owl:Restriction>
                    <owl:Restriction>
                        <owl:onProperty rdf:resource="http://OntoCAPE/upper_level/system.owl#value"/>
                        <owl:cardinality rdf:datatype="http://www.w3.org/2001/XMLSchema#nonNegativeInteger">1</owl:cardinality>
                    </owl:Restriction>
                </owl:unionOf>
            </owl:Class>
        </rdfs:subClassOf>
        <rdfs:subClassOf>
            <owl:Restriction>
                <owl:onProperty rdf:resource="http://OntoCAPE/upper_level/system.owl#qualitativeValue"/>
                <owl:allValuesFrom rdf:resource="http://OntoCAPE/upper_level/system.owl#ValueEnumeration"/>
            </owl:Restriction>
        </rdfs:subClassOf>
        <owl:disjointWith rdf:resource="http://OntoCAPE/upper_level/system.owl#QuantitativeValue"/>
        <rdfs:comment>A QualitativeValue is a value that is not (numerically) quantifiable.</rdfs:comment>
    </owl:Class>
    


    <!-- http://OntoCAPE/upper_level/system.owl#QuantitativeValue -->

    <owl:Class rdf:about="http://OntoCAPE/upper_level/system.owl#QuantitativeValue">
        <owl:equivalentClass>
            <owl:Class>
                <owl:intersectionOf rdf:parseType="Collection">
                    <rdf:Description rdf:about="http://OntoCAPE/upper_level/system.owl#Value"/>
                    <owl:Restriction>
                        <owl:onProperty rdf:resource="http://OntoCAPE/upper_level/system.owl#isValueOf"/>
                        <owl:someValuesFrom rdf:resource="http://OntoCAPE/upper_level/system.owl#PhysicalQuantity"/>
                    </owl:Restriction>
                </owl:intersectionOf>
            </owl:Class>
        </owl:equivalentClass>
        <rdfs:subClassOf>
            <owl:Restriction>
                <owl:onProperty rdf:resource="http://OntoCAPE/upper_level/system.owl#isValueOf"/>
                <owl:allValuesFrom rdf:resource="http://OntoCAPE/upper_level/system.owl#PhysicalQuantity"/>
            </owl:Restriction>
        </rdfs:subClassOf>
        <rdfs:comment>A QuantitativeValue is the value of a PhysicalQuantity.</rdfs:comment>
    </owl:Class>
    


    <!-- http://OntoCAPE/upper_level/system.owl#ScalarQuantity -->

    <owl:Class rdf:about="http://OntoCAPE/upper_level/system.owl#ScalarQuantity">
        <rdfs:subClassOf rdf:resource="http://OntoCAPE/upper_level/system.owl#PhysicalQuantity"/>
        <rdfs:subClassOf>
            <owl:Restriction>
                <owl:onProperty rdf:resource="http://OntoCAPE/upper_level/system.owl#hasValue"/>
                <owl:allValuesFrom rdf:resource="http://OntoCAPE/upper_level/system.owl#ScalarValue"/>
            </owl:Restriction>
        </rdfs:subClassOf>
        <rdfs:comment>A ScalarQuantity is a scalar-valued PhysicalQuantity.</rdfs:comment>
    </owl:Class>
    


    <!-- http://OntoCAPE/upper_level/system.owl#ScalarValue -->

    <owl:Class rdf:about="http://OntoCAPE/upper_level/system.owl#ScalarValue">
        <rdfs:subClassOf rdf:resource="http://OntoCAPE/upper_level/system.owl#QuantitativeValue"/>
        <rdfs:subClassOf>
            <owl:Restriction>
                <owl:onProperty rdf:resource="http://OntoCAPE/upper_level/system.owl#hasUnitOfMeasure"/>
                <owl:allValuesFrom rdf:resource="http://OntoCAPE/upper_level/system.owl#UnitOfMeasure"/>
            </owl:Restriction>
        </rdfs:subClassOf>
        <rdfs:subClassOf>
            <owl:Restriction>
                <owl:onProperty rdf:resource="http://OntoCAPE/upper_level/system.owl#isValueOf"/>
                <owl:allValuesFrom rdf:resource="http://OntoCAPE/upper_level/system.owl#ScalarQuantity"/>
            </owl:Restriction>
        </rdfs:subClassOf>
        <rdfs:subClassOf>
            <owl:Restriction>
                <owl:onProperty rdf:resource="http://OntoCAPE/upper_level/system.owl#hasUnitOfMeasure"/>
                <owl:maxCardinality rdf:datatype="http://www.w3.org/2001/XMLSchema#nonNegativeInteger">1</owl:maxCardinality>
            </owl:Restriction>
        </rdfs:subClassOf>
        <rdfs:subClassOf>
            <owl:Restriction>
                <owl:onProperty rdf:resource="http://OntoCAPE/upper_level/system.owl#numericalValue"/>
                <owl:cardinality rdf:datatype="http://www.w3.org/2001/XMLSchema#nonNegativeInteger">1</owl:cardinality>
            </owl:Restriction>
        </rdfs:subClassOf>
        <rdfs:comment>A ScalarValue is the value of a ScalarQuantity.</rdfs:comment>
    </owl:Class>
    


    <!-- http://OntoCAPE/upper_level/system.owl#SecondLevelSubsystem -->

    <owl:Class rdf:about="http://OntoCAPE/upper_level/system.owl#SecondLevelSubsystem">
        <owl:equivalentClass>
            <owl:Restriction>
                <owl:onProperty rdf:resource="http://OntoCAPE/upper_level/system.owl#isDirectSubsystemOf"/>
                <owl:someValuesFrom rdf:resource="http://OntoCAPE/upper_level/system.owl#FirstLevelSubsystem"/>
            </owl:Restriction>
        </owl:equivalentClass>
        <rdfs:subClassOf rdf:resource="http://OntoCAPE/upper_level/system.owl#Subsystem"/>
        <rdfs:subClassOf>
            <owl:Restriction>
                <owl:onProperty rdf:resource="http://OntoCAPE/upper_level/system.owl#isDirectlyConnectedTo"/>
                <owl:allValuesFrom rdf:resource="http://OntoCAPE/upper_level/system.owl#SecondLevelSubsystem"/>
            </owl:Restriction>
        </rdfs:subClassOf>
        <rdfs:comment>A Subsystem at the second level of decomposition.</rdfs:comment>
    </owl:Class>
    


    <!-- http://OntoCAPE/upper_level/system.owl#Subsystem -->

    <owl:Class rdf:about="http://OntoCAPE/upper_level/system.owl#Subsystem">
        <owl:equivalentClass>
            <owl:Class>
                <owl:intersectionOf rdf:parseType="Collection">
                    <rdf:Description rdf:about="http://OntoCAPE/upper_level/system.owl#System"/>
                    <owl:Restriction>
                        <owl:onProperty rdf:resource="http://OntoCAPE/upper_level/system.owl#isSubsystemOf"/>
                        <owl:someValuesFrom rdf:resource="http://OntoCAPE/upper_level/system.owl#System"/>
                    </owl:Restriction>
                </owl:intersectionOf>
            </owl:Class>
        </owl:equivalentClass>
        <rdfs:subClassOf>
            <owl:Restriction>
                <owl:onProperty rdf:resource="http://OntoCAPE/upper_level/system.owl#isSubsystemOf"/>
                <owl:allValuesFrom rdf:resource="http://OntoCAPE/upper_level/system.owl#System"/>
            </owl:Restriction>
        </rdfs:subClassOf>
        <owl:disjointWith rdf:resource="http://OntoCAPE/upper_level/system.owl#TopLevelSystem"/>
        <rdfs:comment>A Subsystem is a System that is a constituent of another System.</rdfs:comment>
    </owl:Class>
    


    <!-- http://OntoCAPE/upper_level/system.owl#Supersystem -->

    <owl:Class rdf:about="http://OntoCAPE/upper_level/system.owl#Supersystem">
        <owl:equivalentClass>
            <owl:Class>
                <owl:intersectionOf rdf:parseType="Collection">
                    <rdf:Description rdf:about="http://OntoCAPE/upper_level/system.owl#System"/>
                    <owl:Restriction>
                        <owl:onProperty rdf:resource="http://OntoCAPE/upper_level/system.owl#hasSubsystem"/>
                        <owl:someValuesFrom rdf:resource="http://OntoCAPE/upper_level/system.owl#System"/>
                    </owl:Restriction>
                </owl:intersectionOf>
            </owl:Class>
        </owl:equivalentClass>
        <rdfs:subClassOf>
            <owl:Restriction>
                <owl:onProperty rdf:resource="http://OntoCAPE/upper_level/system.owl#hasSubsystem"/>
                <owl:allValuesFrom rdf:resource="http://OntoCAPE/upper_level/system.owl#System"/>
            </owl:Restriction>
        </rdfs:subClassOf>
        <rdfs:comment>A Supersystem is a System that has some constituent Subsystems.</rdfs:comment>
    </owl:Class>
    


    <!-- http://OntoCAPE/upper_level/system.owl#System -->

    <owl:Class rdf:about="http://OntoCAPE/upper_level/system.owl#System">
        <rdfs:subClassOf rdf:resource="http://meta_model/fundamental_concepts/fundamental_concepts.owl#Object"/>
        <rdfs:subClassOf>
            <owl:Restriction>
                <owl:onProperty rdf:resource="http://OntoCAPE/upper_level/system.owl#contains"/>
                <owl:allValuesFrom rdf:resource="http://OntoCAPE/upper_level/system.owl#System"/>
            </owl:Restriction>
        </rdfs:subClassOf>
        <rdfs:subClassOf>
            <owl:Restriction>
                <owl:onProperty rdf:resource="http://OntoCAPE/upper_level/system.owl#hasCharacteristic"/>
                <owl:allValuesFrom>
                    <owl:Class>
                        <owl:unionOf rdf:parseType="Collection">
                            <rdf:Description rdf:about="http://OntoCAPE/upper_level/system.owl#ScalarValue"/>
                            <rdf:Description rdf:about="http://OntoCAPE/upper_level/system.owl#ValueEnumeration"/>
                        </owl:unionOf>
                    </owl:Class>
                </owl:allValuesFrom>
            </owl:Restriction>
        </rdfs:subClassOf>
        <rdfs:subClassOf>
            <owl:Restriction>
                <owl:onProperty rdf:resource="http://OntoCAPE/upper_level/system.owl#hasProperty"/>
                <owl:allValuesFrom rdf:resource="http://OntoCAPE/upper_level/system.owl#Property"/>
            </owl:Restriction>
        </rdfs:subClassOf>
        <rdfs:subClassOf>
            <owl:Restriction>
                <owl:onProperty rdf:resource="http://OntoCAPE/upper_level/system.owl#isModeledBy"/>
                <owl:allValuesFrom rdf:resource="http://OntoCAPE/upper_level/system.owl#Model"/>
            </owl:Restriction>
        </rdfs:subClassOf>
        <rdfs:subClassOf>
            <owl:Restriction>
                <owl:onProperty rdf:resource="http://OntoCAPE/upper_level/system.owl#isRelatedTo"/>
                <owl:allValuesFrom rdf:resource="http://OntoCAPE/upper_level/system.owl#System"/>
            </owl:Restriction>
        </rdfs:subClassOf>
        <owl:disjointWith rdf:resource="http://OntoCAPE/upper_level/system.owl#Value"/>
        <rdfs:comment>The System class denotes all kind of systems, which may be physical or abstract</rdfs:comment>
    </owl:Class>
    


    <!-- http://OntoCAPE/upper_level/system.owl#SystemEnvironment -->

    <owl:Class rdf:about="http://OntoCAPE/upper_level/system.owl#SystemEnvironment">
        <owl:equivalentClass>
            <owl:Class>
                <owl:intersectionOf rdf:parseType="Collection">
                    <rdf:Description rdf:about="http://OntoCAPE/upper_level/system.owl#System"/>
                    <owl:Class>
                        <owl:complementOf>
                            <owl:Class>
                                <owl:oneOf rdf:parseType="Collection">
                                    <rdf:Description rdf:about="http://OntoCAPE/upper_level/system.owl#S"/>
                                </owl:oneOf>
                            </owl:Class>
                        </owl:complementOf>
                    </owl:Class>
                    <owl:Class>
                        <owl:complementOf>
                            <owl:Restriction>
                                <owl:onProperty rdf:resource="http://OntoCAPE/upper_level/system.owl#hasSubsystem"/>
                                <owl:hasValue rdf:resource="http://OntoCAPE/upper_level/system.owl#S"/>
                            </owl:Restriction>
                        </owl:complementOf>
                    </owl:Class>
                    <owl:Class>
                        <owl:complementOf>
                            <owl:Restriction>
                                <owl:onProperty rdf:resource="http://OntoCAPE/upper_level/system.owl#isSubsystemOf"/>
                                <owl:hasValue rdf:resource="http://OntoCAPE/upper_level/system.owl#S"/>
                            </owl:Restriction>
                        </owl:complementOf>
                    </owl:Class>
                    <owl:Restriction>
                        <owl:onProperty rdf:resource="http://OntoCAPE/upper_level/system.owl#isDirectlyRelatedTo"/>
                        <owl:hasValue rdf:resource="http://OntoCAPE/upper_level/system.owl#S"/>
                    </owl:Restriction>
                </owl:intersectionOf>
            </owl:Class>
        </owl:equivalentClass>
        <owl:disjointWith>
            <owl:Class>
                <owl:oneOf rdf:parseType="Collection">
                    <rdf:Description rdf:about="http://OntoCAPE/upper_level/system.owl#S"/>
                </owl:oneOf>
            </owl:Class>
        </owl:disjointWith>
        <rdfs:comment>The ImmediateEnvironment of a given System S consists of all Systems that are directly related to S. It can be specified by means of a query class. As the environment concept is relative, such a query class must be defined individually for each System instance. The query class SystemEnvironment exemplarily demonstrates the approach for sample System S.</rdfs:comment>
    </owl:Class>
    


    <!-- http://OntoCAPE/upper_level/system.owl#SystemInterface -->

    <owl:Class rdf:about="http://OntoCAPE/upper_level/system.owl#SystemInterface">
        <rdfs:subClassOf rdf:resource="http://OntoCAPE/upper_level/system.owl#ExclusiveSubsystem"/>
        <rdfs:subClassOf>
            <owl:Restriction>
                <owl:onProperty rdf:resource="http://OntoCAPE/upper_level/system.owl#isDirectlyConnectedTo"/>
                <owl:allValuesFrom rdf:resource="http://OntoCAPE/upper_level/system.owl#SystemInterface"/>
            </owl:Restriction>
        </rdfs:subClassOf>
        <rdfs:subClassOf>
            <owl:Restriction>
                <owl:onProperty rdf:resource="http://OntoCAPE/upper_level/system.owl#isDirectlyConnectedTo"/>
                <owl:maxCardinality rdf:datatype="http://www.w3.org/2001/XMLSchema#nonNegativeInteger">1</owl:maxCardinality>
            </owl:Restriction>
        </rdfs:subClassOf>
        <rdfs:comment>The class SystemInterface represents the interface through which a System can be connected to another System.</rdfs:comment>
    </owl:Class>
    


    <!-- http://OntoCAPE/upper_level/system.owl#TopLevelSystem -->

    <owl:Class rdf:about="http://OntoCAPE/upper_level/system.owl#TopLevelSystem">
        <owl:equivalentClass>
            <owl:Class>
                <owl:intersectionOf rdf:parseType="Collection">
                    <rdf:Description rdf:about="http://OntoCAPE/upper_level/system.owl#Supersystem"/>
                    <owl:Class>
                        <owl:complementOf rdf:resource="http://OntoCAPE/upper_level/system.owl#Subsystem"/>
                    </owl:Class>
                </owl:intersectionOf>
            </owl:Class>
        </owl:equivalentClass>
        <rdfs:subClassOf>
            <owl:Restriction>
                <owl:onProperty rdf:resource="http://OntoCAPE/upper_level/system.owl#isDirectlyConnectedTo"/>
                <owl:allValuesFrom rdf:resource="http://OntoCAPE/upper_level/system.owl#TopLevelSystem"/>
            </owl:Restriction>
        </rdfs:subClassOf>
        <rdfs:subClassOf>
            <owl:Restriction>
                <owl:onProperty rdf:resource="http://OntoCAPE/upper_level/system.owl#isDirectSubsystemOf"/>
                <owl:cardinality rdf:datatype="http://www.w3.org/2001/XMLSchema#nonNegativeInteger">0</owl:cardinality>
            </owl:Restriction>
        </rdfs:subClassOf>
        <rdfs:comment>A TopLevelSystem is a Supersystem that is not a constituent of some other System.</rdfs:comment>
    </owl:Class>
    


    <!-- http://OntoCAPE/upper_level/system.owl#UnitOfMeasure -->

    <owl:Class rdf:about="http://OntoCAPE/upper_level/system.owl#UnitOfMeasure">
        <rdfs:subClassOf rdf:resource="http://meta_model/fundamental_concepts/fundamental_concepts.owl#NonExhaustiveValueSet"/>
        <rdfs:subClassOf>
            <owl:Restriction>
                <owl:onProperty rdf:resource="http://OntoCAPE/upper_level/system.owl#hasDimension"/>
                <owl:someValuesFrom rdf:resource="http://OntoCAPE/upper_level/system.owl#PhysicalDimension"/>
            </owl:Restriction>
        </rdfs:subClassOf>
        <rdfs:subClassOf>
            <owl:Restriction>
                <owl:onProperty rdf:resource="http://OntoCAPE/upper_level/system.owl#hasDimension"/>
                <owl:allValuesFrom rdf:resource="http://OntoCAPE/upper_level/system.owl#PhysicalDimension"/>
            </owl:Restriction>
        </rdfs:subClassOf>
        <rdfs:subClassOf>
            <owl:Restriction>
                <owl:onProperty rdf:resource="http://OntoCAPE/upper_level/system.owl#hasDimension"/>
                <owl:cardinality rdf:datatype="http://www.w3.org/2001/XMLSchema#nonNegativeInteger">1</owl:cardinality>
            </owl:Restriction>
        </rdfs:subClassOf>
        <rdfs:comment>A UnitOfMeasure is a standard measure for the ScalarValue of a of PhysicalQuantity.</rdfs:comment>
    </owl:Class>
    


    <!-- http://OntoCAPE/upper_level/system.owl#Value -->

    <owl:Class rdf:about="http://OntoCAPE/upper_level/system.owl#Value">
        <rdfs:subClassOf rdf:resource="http://meta_model/fundamental_concepts/fundamental_concepts.owl#Object"/>
        <rdfs:subClassOf>
            <owl:Restriction>
                <owl:onProperty rdf:resource="http://OntoCAPE/upper_level/system.owl#isBackdropOf"/>
                <owl:allValuesFrom rdf:resource="http://OntoCAPE/upper_level/system.owl#Value"/>
            </owl:Restriction>
        </rdfs:subClassOf>
        <rdfs:subClassOf>
            <owl:Restriction>
                <owl:onProperty rdf:resource="http://OntoCAPE/upper_level/system.owl#isObservedAgainstBackdrop"/>
                <owl:allValuesFrom rdf:resource="http://OntoCAPE/upper_level/system.owl#Value"/>
            </owl:Restriction>
        </rdfs:subClassOf>
        <rdfs:subClassOf>
            <owl:Restriction>
                <owl:onProperty rdf:resource="http://OntoCAPE/upper_level/system.owl#isValueOf"/>
                <owl:allValuesFrom rdf:resource="http://OntoCAPE/upper_level/system.owl#Property"/>
            </owl:Restriction>
        </rdfs:subClassOf>
        <rdfs:subClassOf>
            <owl:Restriction>
                <owl:onProperty rdf:resource="http://OntoCAPE/upper_level/system.owl#isValueOf"/>
                <owl:maxCardinality rdf:datatype="http://www.w3.org/2001/XMLSchema#nonNegativeInteger">1</owl:maxCardinality>
            </owl:Restriction>
        </rdfs:subClassOf>
        <rdfs:comment>The Value class denotes the different values of a Property.</rdfs:comment>
    </owl:Class>
    


    <!-- http://OntoCAPE/upper_level/system.owl#ValueEnumeration -->

    <owl:Class rdf:about="http://OntoCAPE/upper_level/system.owl#ValueEnumeration">
        <owl:equivalentClass>
            <owl:Class>
                <owl:unionOf rdf:parseType="Collection">
                    <rdf:Description rdf:about="http://OntoCAPE/upper_level/system.owl#ExtensibleValueSet"/>
                    <rdf:Description rdf:about="http://OntoCAPE/upper_level/system.owl#FixedValueSet"/>
                </owl:unionOf>
            </owl:Class>
        </owl:equivalentClass>
        <rdfs:subClassOf rdf:resource="http://meta_model/fundamental_concepts/fundamental_concepts.owl#FeatureSpace"/>
        <rdfs:comment>A ValueEnumeration specifies a (finite) set of possible values of a QualitativeValue.</rdfs:comment>
    </owl:Class>
    


    <!-- http://meta_model/fundamental_concepts/fundamental_concepts.owl#FeatureSpace -->

    <owl:Class rdf:about="http://meta_model/fundamental_concepts/fundamental_concepts.owl#FeatureSpace"/>
    


    <!-- http://meta_model/fundamental_concepts/fundamental_concepts.owl#NonExhaustiveValueSet -->

    <owl:Class rdf:about="http://meta_model/fundamental_concepts/fundamental_concepts.owl#NonExhaustiveValueSet"/>
    


    <!-- http://meta_model/fundamental_concepts/fundamental_concepts.owl#Object -->

    <owl:Class rdf:about="http://meta_model/fundamental_concepts/fundamental_concepts.owl#Object"/>
    


    <!-- 
    ///////////////////////////////////////////////////////////////////////////////////////
    //
    // Individuals
    //
    ///////////////////////////////////////////////////////////////////////////////////////
     -->

    


    <!-- http://OntoCAPE/chemical_process_system/CPS_function/process.owl#Batch -->

    <owl:NamedIndividual rdf:about="http://OntoCAPE/chemical_process_system/CPS_function/process.owl#Batch">
        <rdf:type rdf:resource="http://OntoCAPE/chemical_process_system/CPS_function/process.owl#ModeOfOperation"/>
    </owl:NamedIndividual>
    


    <!-- http://OntoCAPE/chemical_process_system/CPS_function/process.owl#Continuous -->

    <owl:NamedIndividual rdf:about="http://OntoCAPE/chemical_process_system/CPS_function/process.owl#Continuous">
        <rdf:type rdf:resource="http://OntoCAPE/chemical_process_system/CPS_function/process.owl#ModeOfOperation"/>
    </owl:NamedIndividual>
    


    <!-- http://OntoCAPE/supporting_concepts/physical_dimension/derived_dimensions.owl#pressure -->

    <owl:NamedIndividual rdf:about="http://OntoCAPE/supporting_concepts/physical_dimension/derived_dimensions.owl#pressure"/>
    


    <!-- http://OntoCAPE/supporting_concepts/physical_dimension/physical_dimension.owl#identity_dimension -->

    <owl:NamedIndividual rdf:about="http://OntoCAPE/supporting_concepts/physical_dimension/physical_dimension.owl#identity_dimension"/>
    


    <!-- http://OntoCAPE/upper_level/system.owl#S -->

    <owl:NamedIndividual rdf:about="http://OntoCAPE/upper_level/system.owl#S">
        <rdf:type rdf:resource="http://OntoCAPE/upper_level/system.owl#System"/>
        <rdfs:comment>Sample system; used for the construction of the query classes SystemEnvironment and InternalProperties.</rdfs:comment>
    </owl:NamedIndividual>
</rdf:RDF>



<!-- Generated by the OWL API (version 4.5.29) https://github.com/owlcs/owlapi -->

